update the generated files
git-svn-id: https://projects.brucker.ch/hol-testgen/svn/HOL-TestGen/trunk/hol-testgen@10340 3260e6d1-4efc-4170-b0a7-36055960796d

doc/Employee_DesignModel_UMLPart_generated.thy
@@ -12,7 +12,7 @@ section{* Introduction *}
 
 (* 4 ************************************ 3 + 1 *)
 text{* 
-  
+
   For certain concepts like classes and class-types, only a generic
   definition for its resulting semantics can be given. Generic means,
   there is a function outside HOL that ``compiles'' a concrete,
@@ -47,7 +47,7 @@ text{*  *}
 
 (* 9 ************************************ 8 + 1 *)
 text{* 
-  
+
 \begin{figure}
   \centering\scalebox{.3}{\includegraphics{figures/person.png}}%
   \caption{A simple UML class model drawn from Figure 7.3,
@@ -269,10 +269,10 @@ definition "OclAsType\<^sub>G\<^sub>a\<^sub>l\<^sub>a\<^sub>x\<^sub>y_\<AA> = (\
     | (in\<^sub>P\<^sub>l\<^sub>a\<^sub>n\<^sub>e\<^sub>t (Planet)) \<Rightarrow> \<lfloor>(mkoid\<^sub>G\<^sub>a\<^sub>l\<^sub>a\<^sub>x\<^sub>y ((mk\<^sub>G\<^sub>a\<^sub>l\<^sub>a\<^sub>x\<^sub>y_\<^sub>P\<^sub>l\<^sub>a\<^sub>n\<^sub>e\<^sub>t (Planet))) (None) (None))\<rfloor>
     | (in\<^sub>P\<^sub>e\<^sub>r\<^sub>s\<^sub>o\<^sub>n (Person)) \<Rightarrow> \<lfloor>(mkoid\<^sub>G\<^sub>a\<^sub>l\<^sub>a\<^sub>x\<^sub>y ((mk\<^sub>G\<^sub>a\<^sub>l\<^sub>a\<^sub>x\<^sub>y_\<^sub>P\<^sub>e\<^sub>r\<^sub>s\<^sub>o\<^sub>n (Person))) (None) (None))\<rfloor>
     | _ \<Rightarrow> None)"
-definition "OclAsType\<^sub>O\<^sub>c\<^sub>l\<^sub>A\<^sub>n\<^sub>y_\<AA> = \<lfloor>\<lambda> (in\<^sub>O\<^sub>c\<^sub>l\<^sub>A\<^sub>n\<^sub>y (OclAny)) \<Rightarrow> OclAny
+definition "OclAsType\<^sub>O\<^sub>c\<^sub>l\<^sub>A\<^sub>n\<^sub>y_\<AA> = Some o (\<lambda> (in\<^sub>O\<^sub>c\<^sub>l\<^sub>A\<^sub>n\<^sub>y (OclAny)) \<Rightarrow> OclAny
     | (in\<^sub>G\<^sub>a\<^sub>l\<^sub>a\<^sub>x\<^sub>y (Galaxy)) \<Rightarrow> (mkoid\<^sub>O\<^sub>c\<^sub>l\<^sub>A\<^sub>n\<^sub>y ((mk\<^sub>O\<^sub>c\<^sub>l\<^sub>A\<^sub>n\<^sub>y_\<^sub>G\<^sub>a\<^sub>l\<^sub>a\<^sub>x\<^sub>y (Galaxy))))
     | (in\<^sub>P\<^sub>l\<^sub>a\<^sub>n\<^sub>e\<^sub>t (Planet)) \<Rightarrow> (mkoid\<^sub>O\<^sub>c\<^sub>l\<^sub>A\<^sub>n\<^sub>y ((mk\<^sub>O\<^sub>c\<^sub>l\<^sub>A\<^sub>n\<^sub>y_\<^sub>P\<^sub>l\<^sub>a\<^sub>n\<^sub>e\<^sub>t (Planet))))
-    | (in\<^sub>P\<^sub>e\<^sub>r\<^sub>s\<^sub>o\<^sub>n (Person)) \<Rightarrow> (mkoid\<^sub>O\<^sub>c\<^sub>l\<^sub>A\<^sub>n\<^sub>y ((mk\<^sub>O\<^sub>c\<^sub>l\<^sub>A\<^sub>n\<^sub>y_\<^sub>P\<^sub>e\<^sub>r\<^sub>s\<^sub>o\<^sub>n (Person))))\<rfloor>"
+    | (in\<^sub>P\<^sub>e\<^sub>r\<^sub>s\<^sub>o\<^sub>n (Person)) \<Rightarrow> (mkoid\<^sub>O\<^sub>c\<^sub>l\<^sub>A\<^sub>n\<^sub>y ((mk\<^sub>O\<^sub>c\<^sub>l\<^sub>A\<^sub>n\<^sub>y_\<^sub>P\<^sub>e\<^sub>r\<^sub>s\<^sub>o\<^sub>n (Person)))))"
 
 (* 33 ************************************ 70 + 1 *)
 lemmas [simp,code_unfold] = OclAsType\<^sub>P\<^sub>e\<^sub>r\<^sub>s\<^sub>o\<^sub>n_Person
@@ -590,32 +590,32 @@ lemma OclAsType\<^sub>P\<^sub>l\<^sub>a\<^sub>n\<^sub>e\<^sub>t_Person_defined :
 assumes isdef: "\<tau> \<Turnstile> (\<delta> (X))"
 shows "\<tau> \<Turnstile> (\<delta> ((X::Person) .oclAsType(Planet)))"
   using isdef
-by(auto simp: OclAsType\<^sub>P\<^sub>l\<^sub>a\<^sub>n\<^sub>e\<^sub>t_Person foundation16 null_option_def bot_option_def)
+by(auto simp: OclAsType\<^sub>P\<^sub>l\<^sub>a\<^sub>n\<^sub>e\<^sub>t_Person foundation16 null_option_def bot_option_def) 
 lemma OclAsType\<^sub>G\<^sub>a\<^sub>l\<^sub>a\<^sub>x\<^sub>y_Planet_defined : 
 assumes isdef: "\<tau> \<Turnstile> (\<delta> (X))"
 shows "\<tau> \<Turnstile> (\<delta> ((X::Planet) .oclAsType(Galaxy)))"
   using isdef
-by(auto simp: OclAsType\<^sub>G\<^sub>a\<^sub>l\<^sub>a\<^sub>x\<^sub>y_Planet foundation16 null_option_def bot_option_def)
+by(auto simp: OclAsType\<^sub>G\<^sub>a\<^sub>l\<^sub>a\<^sub>x\<^sub>y_Planet foundation16 null_option_def bot_option_def) 
 lemma OclAsType\<^sub>G\<^sub>a\<^sub>l\<^sub>a\<^sub>x\<^sub>y_Person_defined : 
 assumes isdef: "\<tau> \<Turnstile> (\<delta> (X))"
 shows "\<tau> \<Turnstile> (\<delta> ((X::Person) .oclAsType(Galaxy)))"
   using isdef
-by(auto simp: OclAsType\<^sub>G\<^sub>a\<^sub>l\<^sub>a\<^sub>x\<^sub>y_Person foundation16 null_option_def bot_option_def)
+by(auto simp: OclAsType\<^sub>G\<^sub>a\<^sub>l\<^sub>a\<^sub>x\<^sub>y_Person foundation16 null_option_def bot_option_def) 
 lemma OclAsType\<^sub>O\<^sub>c\<^sub>l\<^sub>A\<^sub>n\<^sub>y_Galaxy_defined : 
 assumes isdef: "\<tau> \<Turnstile> (\<delta> (X))"
 shows "\<tau> \<Turnstile> (\<delta> ((X::Galaxy) .oclAsType(OclAny)))"
   using isdef
-by(auto simp: OclAsType\<^sub>O\<^sub>c\<^sub>l\<^sub>A\<^sub>n\<^sub>y_Galaxy foundation16 null_option_def bot_option_def)
+by(auto simp: OclAsType\<^sub>O\<^sub>c\<^sub>l\<^sub>A\<^sub>n\<^sub>y_Galaxy foundation16 null_option_def bot_option_def) 
 lemma OclAsType\<^sub>O\<^sub>c\<^sub>l\<^sub>A\<^sub>n\<^sub>y_Planet_defined : 
 assumes isdef: "\<tau> \<Turnstile> (\<delta> (X))"
 shows "\<tau> \<Turnstile> (\<delta> ((X::Planet) .oclAsType(OclAny)))"
   using isdef
-by(auto simp: OclAsType\<^sub>O\<^sub>c\<^sub>l\<^sub>A\<^sub>n\<^sub>y_Planet foundation16 null_option_def bot_option_def)
+by(auto simp: OclAsType\<^sub>O\<^sub>c\<^sub>l\<^sub>A\<^sub>n\<^sub>y_Planet foundation16 null_option_def bot_option_def) 
 lemma OclAsType\<^sub>O\<^sub>c\<^sub>l\<^sub>A\<^sub>n\<^sub>y_Person_defined : 
 assumes isdef: "\<tau> \<Turnstile> (\<delta> (X))"
 shows "\<tau> \<Turnstile> (\<delta> ((X::Person) .oclAsType(OclAny)))"
   using isdef
-by(auto simp: OclAsType\<^sub>O\<^sub>c\<^sub>l\<^sub>A\<^sub>n\<^sub>y_Person foundation16 null_option_def bot_option_def)
+by(auto simp: OclAsType\<^sub>O\<^sub>c\<^sub>l\<^sub>A\<^sub>n\<^sub>y_Person foundation16 null_option_def bot_option_def) 
 
 (* 42 ************************************ 178 + 1 *)
 subsection{* Up Down Casting *}
@@ -625,32 +625,32 @@ lemma up\<^sub>P\<^sub>l\<^sub>a\<^sub>n\<^sub>e\<^sub>t_down\<^sub>P\<^sub>e\<^
 assumes isdef: "\<tau> \<Turnstile> (\<delta> (X))"
 shows "\<tau> \<Turnstile> (((X::Person) .oclAsType(Planet)) .oclAsType(Person)) \<triangleq> X"
   using isdef
-by(auto simp: OclAsType\<^sub>P\<^sub>l\<^sub>a\<^sub>n\<^sub>e\<^sub>t_Person OclAsType\<^sub>P\<^sub>e\<^sub>r\<^sub>s\<^sub>o\<^sub>n_Planet foundation22 foundation16 null_option_def bot_option_def split: type\<^sub>P\<^sub>e\<^sub>r\<^sub>s\<^sub>o\<^sub>n.split typeoid\<^sub>P\<^sub>e\<^sub>r\<^sub>s\<^sub>o\<^sub>n.split)
+by(auto simp: OclAsType\<^sub>P\<^sub>l\<^sub>a\<^sub>n\<^sub>e\<^sub>t_Person OclAsType\<^sub>P\<^sub>e\<^sub>r\<^sub>s\<^sub>o\<^sub>n_Planet foundation22 foundation16 null_option_def bot_option_def split: type\<^sub>P\<^sub>e\<^sub>r\<^sub>s\<^sub>o\<^sub>n.split typeoid\<^sub>P\<^sub>e\<^sub>r\<^sub>s\<^sub>o\<^sub>n.split) 
 lemma up\<^sub>G\<^sub>a\<^sub>l\<^sub>a\<^sub>x\<^sub>y_down\<^sub>P\<^sub>e\<^sub>r\<^sub>s\<^sub>o\<^sub>n_cast0 : 
 assumes isdef: "\<tau> \<Turnstile> (\<delta> (X))"
 shows "\<tau> \<Turnstile> (((X::Person) .oclAsType(Galaxy)) .oclAsType(Person)) \<triangleq> X"
   using isdef
-by(auto simp: OclAsType\<^sub>G\<^sub>a\<^sub>l\<^sub>a\<^sub>x\<^sub>y_Person OclAsType\<^sub>P\<^sub>e\<^sub>r\<^sub>s\<^sub>o\<^sub>n_Galaxy foundation22 foundation16 null_option_def bot_option_def split: type\<^sub>P\<^sub>e\<^sub>r\<^sub>s\<^sub>o\<^sub>n.split typeoid\<^sub>P\<^sub>e\<^sub>r\<^sub>s\<^sub>o\<^sub>n.split)
+by(auto simp: OclAsType\<^sub>G\<^sub>a\<^sub>l\<^sub>a\<^sub>x\<^sub>y_Person OclAsType\<^sub>P\<^sub>e\<^sub>r\<^sub>s\<^sub>o\<^sub>n_Galaxy foundation22 foundation16 null_option_def bot_option_def split: type\<^sub>P\<^sub>e\<^sub>r\<^sub>s\<^sub>o\<^sub>n.split typeoid\<^sub>P\<^sub>e\<^sub>r\<^sub>s\<^sub>o\<^sub>n.split) 
 lemma up\<^sub>O\<^sub>c\<^sub>l\<^sub>A\<^sub>n\<^sub>y_down\<^sub>P\<^sub>e\<^sub>r\<^sub>s\<^sub>o\<^sub>n_cast0 : 
 assumes isdef: "\<tau> \<Turnstile> (\<delta> (X))"
 shows "\<tau> \<Turnstile> (((X::Person) .oclAsType(OclAny)) .oclAsType(Person)) \<triangleq> X"
   using isdef
-by(auto simp: OclAsType\<^sub>O\<^sub>c\<^sub>l\<^sub>A\<^sub>n\<^sub>y_Person OclAsType\<^sub>P\<^sub>e\<^sub>r\<^sub>s\<^sub>o\<^sub>n_OclAny foundation22 foundation16 null_option_def bot_option_def split: type\<^sub>P\<^sub>e\<^sub>r\<^sub>s\<^sub>o\<^sub>n.split typeoid\<^sub>P\<^sub>e\<^sub>r\<^sub>s\<^sub>o\<^sub>n.split)
+by(auto simp: OclAsType\<^sub>O\<^sub>c\<^sub>l\<^sub>A\<^sub>n\<^sub>y_Person OclAsType\<^sub>P\<^sub>e\<^sub>r\<^sub>s\<^sub>o\<^sub>n_OclAny foundation22 foundation16 null_option_def bot_option_def split: type\<^sub>P\<^sub>e\<^sub>r\<^sub>s\<^sub>o\<^sub>n.split typeoid\<^sub>P\<^sub>e\<^sub>r\<^sub>s\<^sub>o\<^sub>n.split) 
 lemma up\<^sub>G\<^sub>a\<^sub>l\<^sub>a\<^sub>x\<^sub>y_down\<^sub>P\<^sub>l\<^sub>a\<^sub>n\<^sub>e\<^sub>t_cast0 : 
 assumes isdef: "\<tau> \<Turnstile> (\<delta> (X))"
 shows "\<tau> \<Turnstile> (((X::Planet) .oclAsType(Galaxy)) .oclAsType(Planet)) \<triangleq> X"
   using isdef
-by(auto simp: OclAsType\<^sub>G\<^sub>a\<^sub>l\<^sub>a\<^sub>x\<^sub>y_Planet OclAsType\<^sub>P\<^sub>l\<^sub>a\<^sub>n\<^sub>e\<^sub>t_Galaxy foundation22 foundation16 null_option_def bot_option_def split: type\<^sub>P\<^sub>l\<^sub>a\<^sub>n\<^sub>e\<^sub>t.split typeoid\<^sub>P\<^sub>l\<^sub>a\<^sub>n\<^sub>e\<^sub>t.split)
+by(auto simp: OclAsType\<^sub>G\<^sub>a\<^sub>l\<^sub>a\<^sub>x\<^sub>y_Planet OclAsType\<^sub>P\<^sub>l\<^sub>a\<^sub>n\<^sub>e\<^sub>t_Galaxy foundation22 foundation16 null_option_def bot_option_def split: type\<^sub>P\<^sub>l\<^sub>a\<^sub>n\<^sub>e\<^sub>t.split typeoid\<^sub>P\<^sub>l\<^sub>a\<^sub>n\<^sub>e\<^sub>t.split) 
 lemma up\<^sub>O\<^sub>c\<^sub>l\<^sub>A\<^sub>n\<^sub>y_down\<^sub>P\<^sub>l\<^sub>a\<^sub>n\<^sub>e\<^sub>t_cast0 : 
 assumes isdef: "\<tau> \<Turnstile> (\<delta> (X))"
 shows "\<tau> \<Turnstile> (((X::Planet) .oclAsType(OclAny)) .oclAsType(Planet)) \<triangleq> X"
   using isdef
-by(auto simp: OclAsType\<^sub>O\<^sub>c\<^sub>l\<^sub>A\<^sub>n\<^sub>y_Planet OclAsType\<^sub>P\<^sub>l\<^sub>a\<^sub>n\<^sub>e\<^sub>t_OclAny foundation22 foundation16 null_option_def bot_option_def split: type\<^sub>P\<^sub>l\<^sub>a\<^sub>n\<^sub>e\<^sub>t.split typeoid\<^sub>P\<^sub>l\<^sub>a\<^sub>n\<^sub>e\<^sub>t.split)
+by(auto simp: OclAsType\<^sub>O\<^sub>c\<^sub>l\<^sub>A\<^sub>n\<^sub>y_Planet OclAsType\<^sub>P\<^sub>l\<^sub>a\<^sub>n\<^sub>e\<^sub>t_OclAny foundation22 foundation16 null_option_def bot_option_def split: type\<^sub>P\<^sub>l\<^sub>a\<^sub>n\<^sub>e\<^sub>t.split typeoid\<^sub>P\<^sub>l\<^sub>a\<^sub>n\<^sub>e\<^sub>t.split) 
 lemma up\<^sub>O\<^sub>c\<^sub>l\<^sub>A\<^sub>n\<^sub>y_down\<^sub>G\<^sub>a\<^sub>l\<^sub>a\<^sub>x\<^sub>y_cast0 : 
 assumes isdef: "\<tau> \<Turnstile> (\<delta> (X))"
 shows "\<tau> \<Turnstile> (((X::Galaxy) .oclAsType(OclAny)) .oclAsType(Galaxy)) \<triangleq> X"
   using isdef
-by(auto simp: OclAsType\<^sub>O\<^sub>c\<^sub>l\<^sub>A\<^sub>n\<^sub>y_Galaxy OclAsType\<^sub>G\<^sub>a\<^sub>l\<^sub>a\<^sub>x\<^sub>y_OclAny foundation22 foundation16 null_option_def bot_option_def split: type\<^sub>G\<^sub>a\<^sub>l\<^sub>a\<^sub>x\<^sub>y.split typeoid\<^sub>G\<^sub>a\<^sub>l\<^sub>a\<^sub>x\<^sub>y.split)
+by(auto simp: OclAsType\<^sub>O\<^sub>c\<^sub>l\<^sub>A\<^sub>n\<^sub>y_Galaxy OclAsType\<^sub>G\<^sub>a\<^sub>l\<^sub>a\<^sub>x\<^sub>y_OclAny foundation22 foundation16 null_option_def bot_option_def split: type\<^sub>G\<^sub>a\<^sub>l\<^sub>a\<^sub>x\<^sub>y.split typeoid\<^sub>G\<^sub>a\<^sub>l\<^sub>a\<^sub>x\<^sub>y.split) 
 
 (* 44 ************************************ 185 + 6 *)
 lemma up\<^sub>P\<^sub>l\<^sub>a\<^sub>n\<^sub>e\<^sub>t_down\<^sub>P\<^sub>e\<^sub>r\<^sub>s\<^sub>o\<^sub>n_cast : 
@@ -660,7 +660,7 @@ shows "(((X::Person) .oclAsType(Planet)) .oclAsType(Person)) = X"
   apply(case_tac "\<tau> \<Turnstile> (\<delta> (X))", simp add: up\<^sub>P\<^sub>l\<^sub>a\<^sub>n\<^sub>e\<^sub>t_down\<^sub>P\<^sub>e\<^sub>r\<^sub>s\<^sub>o\<^sub>n_cast0)
   apply(simp add: def_split_local, elim disjE)
   apply((erule StrongEq_L_subst2_rev, simp, simp)+)
-done
+done 
 lemma up\<^sub>G\<^sub>a\<^sub>l\<^sub>a\<^sub>x\<^sub>y_down\<^sub>P\<^sub>e\<^sub>r\<^sub>s\<^sub>o\<^sub>n_cast : 
 shows "(((X::Person) .oclAsType(Galaxy)) .oclAsType(Person)) = X"
   apply(rule ext, rename_tac \<tau>)
@@ -668,7 +668,7 @@ shows "(((X::Person) .oclAsType(Galaxy)) .oclAsType(Person)) = X"
   apply(case_tac "\<tau> \<Turnstile> (\<delta> (X))", simp add: up\<^sub>G\<^sub>a\<^sub>l\<^sub>a\<^sub>x\<^sub>y_down\<^sub>P\<^sub>e\<^sub>r\<^sub>s\<^sub>o\<^sub>n_cast0)
   apply(simp add: def_split_local, elim disjE)
   apply((erule StrongEq_L_subst2_rev, simp, simp)+)
-done
+done 
 lemma up\<^sub>O\<^sub>c\<^sub>l\<^sub>A\<^sub>n\<^sub>y_down\<^sub>P\<^sub>e\<^sub>r\<^sub>s\<^sub>o\<^sub>n_cast : 
 shows "(((X::Person) .oclAsType(OclAny)) .oclAsType(Person)) = X"
   apply(rule ext, rename_tac \<tau>)
@@ -676,7 +676,7 @@ shows "(((X::Person) .oclAsType(OclAny)) .oclAsType(Person)) = X"
   apply(case_tac "\<tau> \<Turnstile> (\<delta> (X))", simp add: up\<^sub>O\<^sub>c\<^sub>l\<^sub>A\<^sub>n\<^sub>y_down\<^sub>P\<^sub>e\<^sub>r\<^sub>s\<^sub>o\<^sub>n_cast0)
   apply(simp add: def_split_local, elim disjE)
   apply((erule StrongEq_L_subst2_rev, simp, simp)+)
-done
+done 
 lemma up\<^sub>G\<^sub>a\<^sub>l\<^sub>a\<^sub>x\<^sub>y_down\<^sub>P\<^sub>l\<^sub>a\<^sub>n\<^sub>e\<^sub>t_cast : 
 shows "(((X::Planet) .oclAsType(Galaxy)) .oclAsType(Planet)) = X"
   apply(rule ext, rename_tac \<tau>)
@@ -684,7 +684,7 @@ shows "(((X::Planet) .oclAsType(Galaxy)) .oclAsType(Planet)) = X"
   apply(case_tac "\<tau> \<Turnstile> (\<delta> (X))", simp add: up\<^sub>G\<^sub>a\<^sub>l\<^sub>a\<^sub>x\<^sub>y_down\<^sub>P\<^sub>l\<^sub>a\<^sub>n\<^sub>e\<^sub>t_cast0)
   apply(simp add: def_split_local, elim disjE)
   apply((erule StrongEq_L_subst2_rev, simp, simp)+)
-done
+done 
 lemma up\<^sub>O\<^sub>c\<^sub>l\<^sub>A\<^sub>n\<^sub>y_down\<^sub>P\<^sub>l\<^sub>a\<^sub>n\<^sub>e\<^sub>t_cast : 
 shows "(((X::Planet) .oclAsType(OclAny)) .oclAsType(Planet)) = X"
   apply(rule ext, rename_tac \<tau>)
@@ -692,7 +692,7 @@ shows "(((X::Planet) .oclAsType(OclAny)) .oclAsType(Planet)) = X"
   apply(case_tac "\<tau> \<Turnstile> (\<delta> (X))", simp add: up\<^sub>O\<^sub>c\<^sub>l\<^sub>A\<^sub>n\<^sub>y_down\<^sub>P\<^sub>l\<^sub>a\<^sub>n\<^sub>e\<^sub>t_cast0)
   apply(simp add: def_split_local, elim disjE)
   apply((erule StrongEq_L_subst2_rev, simp, simp)+)
-done
+done 
 lemma up\<^sub>O\<^sub>c\<^sub>l\<^sub>A\<^sub>n\<^sub>y_down\<^sub>G\<^sub>a\<^sub>l\<^sub>a\<^sub>x\<^sub>y_cast : 
 shows "(((X::Galaxy) .oclAsType(OclAny)) .oclAsType(Galaxy)) = X"
   apply(rule ext, rename_tac \<tau>)
@@ -700,7 +700,7 @@ shows "(((X::Galaxy) .oclAsType(OclAny)) .oclAsType(Galaxy)) = X"
   apply(case_tac "\<tau> \<Turnstile> (\<delta> (X))", simp add: up\<^sub>O\<^sub>c\<^sub>l\<^sub>A\<^sub>n\<^sub>y_down\<^sub>G\<^sub>a\<^sub>l\<^sub>a\<^sub>x\<^sub>y_cast0)
   apply(simp add: def_split_local, elim disjE)
   apply((erule StrongEq_L_subst2_rev, simp, simp)+)
-done
+done 
 
 (* 45 ************************************ 191 + 1 *)
 section{* OclIsTypeOf *}
@@ -1107,148 +1107,148 @@ lemma OclIsTypeOf\<^sub>P\<^sub>e\<^sub>r\<^sub>s\<^sub>o\<^sub>n_OclAny_defined
 assumes isdef: "\<tau> \<Turnstile> (\<upsilon> (X))"
 shows "\<tau> \<Turnstile> (\<delta> ((X::OclAny) .oclIsTypeOf(Person)))"
   apply(insert isdef[simplified foundation18'], simp only: OclValid_def, subst cp_defined)
-by(auto simp: cp_defined[symmetric ] bot_option_def OclIsTypeOf\<^sub>P\<^sub>e\<^sub>r\<^sub>s\<^sub>o\<^sub>n_OclAny split: option.split type\<^sub>O\<^sub>c\<^sub>l\<^sub>A\<^sub>n\<^sub>y.split typeoid\<^sub>O\<^sub>c\<^sub>l\<^sub>A\<^sub>n\<^sub>y.split)
+by(auto simp: cp_defined[symmetric ] bot_option_def OclIsTypeOf\<^sub>P\<^sub>e\<^sub>r\<^sub>s\<^sub>o\<^sub>n_OclAny split: option.split type\<^sub>O\<^sub>c\<^sub>l\<^sub>A\<^sub>n\<^sub>y.split typeoid\<^sub>O\<^sub>c\<^sub>l\<^sub>A\<^sub>n\<^sub>y.split) 
 lemma OclIsTypeOf\<^sub>P\<^sub>e\<^sub>r\<^sub>s\<^sub>o\<^sub>n_Galaxy_defined : 
 assumes isdef: "\<tau> \<Turnstile> (\<upsilon> (X))"
 shows "\<tau> \<Turnstile> (\<delta> ((X::Galaxy) .oclIsTypeOf(Person)))"
   apply(insert isdef[simplified foundation18'], simp only: OclValid_def, subst cp_defined)
-by(auto simp: cp_defined[symmetric ] bot_option_def OclIsTypeOf\<^sub>P\<^sub>e\<^sub>r\<^sub>s\<^sub>o\<^sub>n_Galaxy split: option.split type\<^sub>G\<^sub>a\<^sub>l\<^sub>a\<^sub>x\<^sub>y.split typeoid\<^sub>G\<^sub>a\<^sub>l\<^sub>a\<^sub>x\<^sub>y.split)
+by(auto simp: cp_defined[symmetric ] bot_option_def OclIsTypeOf\<^sub>P\<^sub>e\<^sub>r\<^sub>s\<^sub>o\<^sub>n_Galaxy split: option.split type\<^sub>G\<^sub>a\<^sub>l\<^sub>a\<^sub>x\<^sub>y.split typeoid\<^sub>G\<^sub>a\<^sub>l\<^sub>a\<^sub>x\<^sub>y.split) 
 lemma OclIsTypeOf\<^sub>P\<^sub>e\<^sub>r\<^sub>s\<^sub>o\<^sub>n_Planet_defined : 
 assumes isdef: "\<tau> \<Turnstile> (\<upsilon> (X))"
 shows "\<tau> \<Turnstile> (\<delta> ((X::Planet) .oclIsTypeOf(Person)))"
   apply(insert isdef[simplified foundation18'], simp only: OclValid_def, subst cp_defined)
-by(auto simp: cp_defined[symmetric ] bot_option_def OclIsTypeOf\<^sub>P\<^sub>e\<^sub>r\<^sub>s\<^sub>o\<^sub>n_Planet split: option.split type\<^sub>P\<^sub>l\<^sub>a\<^sub>n\<^sub>e\<^sub>t.split typeoid\<^sub>P\<^sub>l\<^sub>a\<^sub>n\<^sub>e\<^sub>t.split)
+by(auto simp: cp_defined[symmetric ] bot_option_def OclIsTypeOf\<^sub>P\<^sub>e\<^sub>r\<^sub>s\<^sub>o\<^sub>n_Planet split: option.split type\<^sub>P\<^sub>l\<^sub>a\<^sub>n\<^sub>e\<^sub>t.split typeoid\<^sub>P\<^sub>l\<^sub>a\<^sub>n\<^sub>e\<^sub>t.split) 
 lemma OclIsTypeOf\<^sub>P\<^sub>e\<^sub>r\<^sub>s\<^sub>o\<^sub>n_Person_defined : 
 assumes isdef: "\<tau> \<Turnstile> (\<upsilon> (X))"
 shows "\<tau> \<Turnstile> (\<delta> ((X::Person) .oclIsTypeOf(Person)))"
   apply(insert isdef[simplified foundation18'], simp only: OclValid_def, subst cp_defined)
-by(auto simp: cp_defined[symmetric ] bot_option_def OclIsTypeOf\<^sub>P\<^sub>e\<^sub>r\<^sub>s\<^sub>o\<^sub>n_Person split: option.split type\<^sub>P\<^sub>e\<^sub>r\<^sub>s\<^sub>o\<^sub>n.split typeoid\<^sub>P\<^sub>e\<^sub>r\<^sub>s\<^sub>o\<^sub>n.split)
+by(auto simp: cp_defined[symmetric ] bot_option_def OclIsTypeOf\<^sub>P\<^sub>e\<^sub>r\<^sub>s\<^sub>o\<^sub>n_Person split: option.split type\<^sub>P\<^sub>e\<^sub>r\<^sub>s\<^sub>o\<^sub>n.split typeoid\<^sub>P\<^sub>e\<^sub>r\<^sub>s\<^sub>o\<^sub>n.split) 
 lemma OclIsTypeOf\<^sub>P\<^sub>l\<^sub>a\<^sub>n\<^sub>e\<^sub>t_OclAny_defined : 
 assumes isdef: "\<tau> \<Turnstile> (\<upsilon> (X))"
 shows "\<tau> \<Turnstile> (\<delta> ((X::OclAny) .oclIsTypeOf(Planet)))"
   apply(insert isdef[simplified foundation18'], simp only: OclValid_def, subst cp_defined)
-by(auto simp: cp_defined[symmetric ] bot_option_def OclIsTypeOf\<^sub>P\<^sub>l\<^sub>a\<^sub>n\<^sub>e\<^sub>t_OclAny split: option.split type\<^sub>O\<^sub>c\<^sub>l\<^sub>A\<^sub>n\<^sub>y.split typeoid\<^sub>O\<^sub>c\<^sub>l\<^sub>A\<^sub>n\<^sub>y.split)
+by(auto simp: cp_defined[symmetric ] bot_option_def OclIsTypeOf\<^sub>P\<^sub>l\<^sub>a\<^sub>n\<^sub>e\<^sub>t_OclAny split: option.split type\<^sub>O\<^sub>c\<^sub>l\<^sub>A\<^sub>n\<^sub>y.split typeoid\<^sub>O\<^sub>c\<^sub>l\<^sub>A\<^sub>n\<^sub>y.split) 
 lemma OclIsTypeOf\<^sub>P\<^sub>l\<^sub>a\<^sub>n\<^sub>e\<^sub>t_Galaxy_defined : 
 assumes isdef: "\<tau> \<Turnstile> (\<upsilon> (X))"
 shows "\<tau> \<Turnstile> (\<delta> ((X::Galaxy) .oclIsTypeOf(Planet)))"
   apply(insert isdef[simplified foundation18'], simp only: OclValid_def, subst cp_defined)
-by(auto simp: cp_defined[symmetric ] bot_option_def OclIsTypeOf\<^sub>P\<^sub>l\<^sub>a\<^sub>n\<^sub>e\<^sub>t_Galaxy split: option.split type\<^sub>G\<^sub>a\<^sub>l\<^sub>a\<^sub>x\<^sub>y.split typeoid\<^sub>G\<^sub>a\<^sub>l\<^sub>a\<^sub>x\<^sub>y.split)
+by(auto simp: cp_defined[symmetric ] bot_option_def OclIsTypeOf\<^sub>P\<^sub>l\<^sub>a\<^sub>n\<^sub>e\<^sub>t_Galaxy split: option.split type\<^sub>G\<^sub>a\<^sub>l\<^sub>a\<^sub>x\<^sub>y.split typeoid\<^sub>G\<^sub>a\<^sub>l\<^sub>a\<^sub>x\<^sub>y.split) 
 lemma OclIsTypeOf\<^sub>P\<^sub>l\<^sub>a\<^sub>n\<^sub>e\<^sub>t_Planet_defined : 
 assumes isdef: "\<tau> \<Turnstile> (\<upsilon> (X))"
 shows "\<tau> \<Turnstile> (\<delta> ((X::Planet) .oclIsTypeOf(Planet)))"
   apply(insert isdef[simplified foundation18'], simp only: OclValid_def, subst cp_defined)
-by(auto simp: cp_defined[symmetric ] bot_option_def OclIsTypeOf\<^sub>P\<^sub>l\<^sub>a\<^sub>n\<^sub>e\<^sub>t_Planet split: option.split type\<^sub>P\<^sub>l\<^sub>a\<^sub>n\<^sub>e\<^sub>t.split typeoid\<^sub>P\<^sub>l\<^sub>a\<^sub>n\<^sub>e\<^sub>t.split)
+by(auto simp: cp_defined[symmetric ] bot_option_def OclIsTypeOf\<^sub>P\<^sub>l\<^sub>a\<^sub>n\<^sub>e\<^sub>t_Planet split: option.split type\<^sub>P\<^sub>l\<^sub>a\<^sub>n\<^sub>e\<^sub>t.split typeoid\<^sub>P\<^sub>l\<^sub>a\<^sub>n\<^sub>e\<^sub>t.split) 
 lemma OclIsTypeOf\<^sub>P\<^sub>l\<^sub>a\<^sub>n\<^sub>e\<^sub>t_Person_defined : 
 assumes isdef: "\<tau> \<Turnstile> (\<upsilon> (X))"
 shows "\<tau> \<Turnstile> (\<delta> ((X::Person) .oclIsTypeOf(Planet)))"
   apply(insert isdef[simplified foundation18'], simp only: OclValid_def, subst cp_defined)
-by(auto simp: cp_defined[symmetric ] bot_option_def OclIsTypeOf\<^sub>P\<^sub>l\<^sub>a\<^sub>n\<^sub>e\<^sub>t_Person split: option.split type\<^sub>P\<^sub>e\<^sub>r\<^sub>s\<^sub>o\<^sub>n.split typeoid\<^sub>P\<^sub>e\<^sub>r\<^sub>s\<^sub>o\<^sub>n.split)
+by(auto simp: cp_defined[symmetric ] bot_option_def OclIsTypeOf\<^sub>P\<^sub>l\<^sub>a\<^sub>n\<^sub>e\<^sub>t_Person split: option.split type\<^sub>P\<^sub>e\<^sub>r\<^sub>s\<^sub>o\<^sub>n.split typeoid\<^sub>P\<^sub>e\<^sub>r\<^sub>s\<^sub>o\<^sub>n.split) 
 lemma OclIsTypeOf\<^sub>G\<^sub>a\<^sub>l\<^sub>a\<^sub>x\<^sub>y_OclAny_defined : 
 assumes isdef: "\<tau> \<Turnstile> (\<upsilon> (X))"
 shows "\<tau> \<Turnstile> (\<delta> ((X::OclAny) .oclIsTypeOf(Galaxy)))"
   apply(insert isdef[simplified foundation18'], simp only: OclValid_def, subst cp_defined)
-by(auto simp: cp_defined[symmetric ] bot_option_def OclIsTypeOf\<^sub>G\<^sub>a\<^sub>l\<^sub>a\<^sub>x\<^sub>y_OclAny split: option.split type\<^sub>O\<^sub>c\<^sub>l\<^sub>A\<^sub>n\<^sub>y.split typeoid\<^sub>O\<^sub>c\<^sub>l\<^sub>A\<^sub>n\<^sub>y.split)
+by(auto simp: cp_defined[symmetric ] bot_option_def OclIsTypeOf\<^sub>G\<^sub>a\<^sub>l\<^sub>a\<^sub>x\<^sub>y_OclAny split: option.split type\<^sub>O\<^sub>c\<^sub>l\<^sub>A\<^sub>n\<^sub>y.split typeoid\<^sub>O\<^sub>c\<^sub>l\<^sub>A\<^sub>n\<^sub>y.split) 
 lemma OclIsTypeOf\<^sub>G\<^sub>a\<^sub>l\<^sub>a\<^sub>x\<^sub>y_Galaxy_defined : 
 assumes isdef: "\<tau> \<Turnstile> (\<upsilon> (X))"
 shows "\<tau> \<Turnstile> (\<delta> ((X::Galaxy) .oclIsTypeOf(Galaxy)))"
   apply(insert isdef[simplified foundation18'], simp only: OclValid_def, subst cp_defined)
-by(auto simp: cp_defined[symmetric ] bot_option_def OclIsTypeOf\<^sub>G\<^sub>a\<^sub>l\<^sub>a\<^sub>x\<^sub>y_Galaxy split: option.split type\<^sub>G\<^sub>a\<^sub>l\<^sub>a\<^sub>x\<^sub>y.split typeoid\<^sub>G\<^sub>a\<^sub>l\<^sub>a\<^sub>x\<^sub>y.split)
+by(auto simp: cp_defined[symmetric ] bot_option_def OclIsTypeOf\<^sub>G\<^sub>a\<^sub>l\<^sub>a\<^sub>x\<^sub>y_Galaxy split: option.split type\<^sub>G\<^sub>a\<^sub>l\<^sub>a\<^sub>x\<^sub>y.split typeoid\<^sub>G\<^sub>a\<^sub>l\<^sub>a\<^sub>x\<^sub>y.split) 
 lemma OclIsTypeOf\<^sub>G\<^sub>a\<^sub>l\<^sub>a\<^sub>x\<^sub>y_Planet_defined : 
 assumes isdef: "\<tau> \<Turnstile> (\<upsilon> (X))"
 shows "\<tau> \<Turnstile> (\<delta> ((X::Planet) .oclIsTypeOf(Galaxy)))"
   apply(insert isdef[simplified foundation18'], simp only: OclValid_def, subst cp_defined)
-by(auto simp: cp_defined[symmetric ] bot_option_def OclIsTypeOf\<^sub>G\<^sub>a\<^sub>l\<^sub>a\<^sub>x\<^sub>y_Planet split: option.split type\<^sub>P\<^sub>l\<^sub>a\<^sub>n\<^sub>e\<^sub>t.split typeoid\<^sub>P\<^sub>l\<^sub>a\<^sub>n\<^sub>e\<^sub>t.split)
+by(auto simp: cp_defined[symmetric ] bot_option_def OclIsTypeOf\<^sub>G\<^sub>a\<^sub>l\<^sub>a\<^sub>x\<^sub>y_Planet split: option.split type\<^sub>P\<^sub>l\<^sub>a\<^sub>n\<^sub>e\<^sub>t.split typeoid\<^sub>P\<^sub>l\<^sub>a\<^sub>n\<^sub>e\<^sub>t.split) 
 lemma OclIsTypeOf\<^sub>G\<^sub>a\<^sub>l\<^sub>a\<^sub>x\<^sub>y_Person_defined : 
 assumes isdef: "\<tau> \<Turnstile> (\<upsilon> (X))"
 shows "\<tau> \<Turnstile> (\<delta> ((X::Person) .oclIsTypeOf(Galaxy)))"
   apply(insert isdef[simplified foundation18'], simp only: OclValid_def, subst cp_defined)
-by(auto simp: cp_defined[symmetric ] bot_option_def OclIsTypeOf\<^sub>G\<^sub>a\<^sub>l\<^sub>a\<^sub>x\<^sub>y_Person split: option.split type\<^sub>P\<^sub>e\<^sub>r\<^sub>s\<^sub>o\<^sub>n.split typeoid\<^sub>P\<^sub>e\<^sub>r\<^sub>s\<^sub>o\<^sub>n.split)
+by(auto simp: cp_defined[symmetric ] bot_option_def OclIsTypeOf\<^sub>G\<^sub>a\<^sub>l\<^sub>a\<^sub>x\<^sub>y_Person split: option.split type\<^sub>P\<^sub>e\<^sub>r\<^sub>s\<^sub>o\<^sub>n.split typeoid\<^sub>P\<^sub>e\<^sub>r\<^sub>s\<^sub>o\<^sub>n.split) 
 lemma OclIsTypeOf\<^sub>O\<^sub>c\<^sub>l\<^sub>A\<^sub>n\<^sub>y_OclAny_defined : 
 assumes isdef: "\<tau> \<Turnstile> (\<upsilon> (X))"
 shows "\<tau> \<Turnstile> (\<delta> ((X::OclAny) .oclIsTypeOf(OclAny)))"
   apply(insert isdef[simplified foundation18'], simp only: OclValid_def, subst cp_defined)
-by(auto simp: cp_defined[symmetric ] bot_option_def OclIsTypeOf\<^sub>O\<^sub>c\<^sub>l\<^sub>A\<^sub>n\<^sub>y_OclAny split: option.split type\<^sub>O\<^sub>c\<^sub>l\<^sub>A\<^sub>n\<^sub>y.split typeoid\<^sub>O\<^sub>c\<^sub>l\<^sub>A\<^sub>n\<^sub>y.split)
+by(auto simp: cp_defined[symmetric ] bot_option_def OclIsTypeOf\<^sub>O\<^sub>c\<^sub>l\<^sub>A\<^sub>n\<^sub>y_OclAny split: option.split type\<^sub>O\<^sub>c\<^sub>l\<^sub>A\<^sub>n\<^sub>y.split typeoid\<^sub>O\<^sub>c\<^sub>l\<^sub>A\<^sub>n\<^sub>y.split) 
 lemma OclIsTypeOf\<^sub>O\<^sub>c\<^sub>l\<^sub>A\<^sub>n\<^sub>y_Galaxy_defined : 
 assumes isdef: "\<tau> \<Turnstile> (\<upsilon> (X))"
 shows "\<tau> \<Turnstile> (\<delta> ((X::Galaxy) .oclIsTypeOf(OclAny)))"
   apply(insert isdef[simplified foundation18'], simp only: OclValid_def, subst cp_defined)
-by(auto simp: cp_defined[symmetric ] bot_option_def OclIsTypeOf\<^sub>O\<^sub>c\<^sub>l\<^sub>A\<^sub>n\<^sub>y_Galaxy split: option.split type\<^sub>G\<^sub>a\<^sub>l\<^sub>a\<^sub>x\<^sub>y.split typeoid\<^sub>G\<^sub>a\<^sub>l\<^sub>a\<^sub>x\<^sub>y.split)
+by(auto simp: cp_defined[symmetric ] bot_option_def OclIsTypeOf\<^sub>O\<^sub>c\<^sub>l\<^sub>A\<^sub>n\<^sub>y_Galaxy split: option.split type\<^sub>G\<^sub>a\<^sub>l\<^sub>a\<^sub>x\<^sub>y.split typeoid\<^sub>G\<^sub>a\<^sub>l\<^sub>a\<^sub>x\<^sub>y.split) 
 lemma OclIsTypeOf\<^sub>O\<^sub>c\<^sub>l\<^sub>A\<^sub>n\<^sub>y_Planet_defined : 
 assumes isdef: "\<tau> \<Turnstile> (\<upsilon> (X))"
 shows "\<tau> \<Turnstile> (\<delta> ((X::Planet) .oclIsTypeOf(OclAny)))"
   apply(insert isdef[simplified foundation18'], simp only: OclValid_def, subst cp_defined)
-by(auto simp: cp_defined[symmetric ] bot_option_def OclIsTypeOf\<^sub>O\<^sub>c\<^sub>l\<^sub>A\<^sub>n\<^sub>y_Planet split: option.split type\<^sub>P\<^sub>l\<^sub>a\<^sub>n\<^sub>e\<^sub>t.split typeoid\<^sub>P\<^sub>l\<^sub>a\<^sub>n\<^sub>e\<^sub>t.split)
+by(auto simp: cp_defined[symmetric ] bot_option_def OclIsTypeOf\<^sub>O\<^sub>c\<^sub>l\<^sub>A\<^sub>n\<^sub>y_Planet split: option.split type\<^sub>P\<^sub>l\<^sub>a\<^sub>n\<^sub>e\<^sub>t.split typeoid\<^sub>P\<^sub>l\<^sub>a\<^sub>n\<^sub>e\<^sub>t.split) 
 lemma OclIsTypeOf\<^sub>O\<^sub>c\<^sub>l\<^sub>A\<^sub>n\<^sub>y_Person_defined : 
 assumes isdef: "\<tau> \<Turnstile> (\<upsilon> (X))"
 shows "\<tau> \<Turnstile> (\<delta> ((X::Person) .oclIsTypeOf(OclAny)))"
   apply(insert isdef[simplified foundation18'], simp only: OclValid_def, subst cp_defined)
-by(auto simp: cp_defined[symmetric ] bot_option_def OclIsTypeOf\<^sub>O\<^sub>c\<^sub>l\<^sub>A\<^sub>n\<^sub>y_Person split: option.split type\<^sub>P\<^sub>e\<^sub>r\<^sub>s\<^sub>o\<^sub>n.split typeoid\<^sub>P\<^sub>e\<^sub>r\<^sub>s\<^sub>o\<^sub>n.split)
+by(auto simp: cp_defined[symmetric ] bot_option_def OclIsTypeOf\<^sub>O\<^sub>c\<^sub>l\<^sub>A\<^sub>n\<^sub>y_Person split: option.split type\<^sub>P\<^sub>e\<^sub>r\<^sub>s\<^sub>o\<^sub>n.split typeoid\<^sub>P\<^sub>e\<^sub>r\<^sub>s\<^sub>o\<^sub>n.split) 
 
 (* 59 ************************************ 335 + 16 *)
 lemma OclIsTypeOf\<^sub>P\<^sub>e\<^sub>r\<^sub>s\<^sub>o\<^sub>n_OclAny_defined' : 
 assumes isdef: "\<tau> \<Turnstile> (\<delta> (X))"
 shows "\<tau> \<Turnstile> (\<delta> ((X::OclAny) .oclIsTypeOf(Person)))"
-by(rule OclIsTypeOf\<^sub>P\<^sub>e\<^sub>r\<^sub>s\<^sub>o\<^sub>n_OclAny_defined[OF isdef[THEN foundation20]])
+by(rule OclIsTypeOf\<^sub>P\<^sub>e\<^sub>r\<^sub>s\<^sub>o\<^sub>n_OclAny_defined[OF isdef[THEN foundation20]]) 
 lemma OclIsTypeOf\<^sub>P\<^sub>e\<^sub>r\<^sub>s\<^sub>o\<^sub>n_Galaxy_defined' : 
 assumes isdef: "\<tau> \<Turnstile> (\<delta> (X))"
 shows "\<tau> \<Turnstile> (\<delta> ((X::Galaxy) .oclIsTypeOf(Person)))"
-by(rule OclIsTypeOf\<^sub>P\<^sub>e\<^sub>r\<^sub>s\<^sub>o\<^sub>n_Galaxy_defined[OF isdef[THEN foundation20]])
+by(rule OclIsTypeOf\<^sub>P\<^sub>e\<^sub>r\<^sub>s\<^sub>o\<^sub>n_Galaxy_defined[OF isdef[THEN foundation20]]) 
 lemma OclIsTypeOf\<^sub>P\<^sub>e\<^sub>r\<^sub>s\<^sub>o\<^sub>n_Planet_defined' : 
 assumes isdef: "\<tau> \<Turnstile> (\<delta> (X))"
 shows "\<tau> \<Turnstile> (\<delta> ((X::Planet) .oclIsTypeOf(Person)))"
-by(rule OclIsTypeOf\<^sub>P\<^sub>e\<^sub>r\<^sub>s\<^sub>o\<^sub>n_Planet_defined[OF isdef[THEN foundation20]])
+by(rule OclIsTypeOf\<^sub>P\<^sub>e\<^sub>r\<^sub>s\<^sub>o\<^sub>n_Planet_defined[OF isdef[THEN foundation20]]) 
 lemma OclIsTypeOf\<^sub>P\<^sub>e\<^sub>r\<^sub>s\<^sub>o\<^sub>n_Person_defined' : 
 assumes isdef: "\<tau> \<Turnstile> (\<delta> (X))"
 shows "\<tau> \<Turnstile> (\<delta> ((X::Person) .oclIsTypeOf(Person)))"
-by(rule OclIsTypeOf\<^sub>P\<^sub>e\<^sub>r\<^sub>s\<^sub>o\<^sub>n_Person_defined[OF isdef[THEN foundation20]])
+by(rule OclIsTypeOf\<^sub>P\<^sub>e\<^sub>r\<^sub>s\<^sub>o\<^sub>n_Person_defined[OF isdef[THEN foundation20]]) 
 lemma OclIsTypeOf\<^sub>P\<^sub>l\<^sub>a\<^sub>n\<^sub>e\<^sub>t_OclAny_defined' : 
 assumes isdef: "\<tau> \<Turnstile> (\<delta> (X))"
 shows "\<tau> \<Turnstile> (\<delta> ((X::OclAny) .oclIsTypeOf(Planet)))"
-by(rule OclIsTypeOf\<^sub>P\<^sub>l\<^sub>a\<^sub>n\<^sub>e\<^sub>t_OclAny_defined[OF isdef[THEN foundation20]])
+by(rule OclIsTypeOf\<^sub>P\<^sub>l\<^sub>a\<^sub>n\<^sub>e\<^sub>t_OclAny_defined[OF isdef[THEN foundation20]]) 
 lemma OclIsTypeOf\<^sub>P\<^sub>l\<^sub>a\<^sub>n\<^sub>e\<^sub>t_Galaxy_defined' : 
 assumes isdef: "\<tau> \<Turnstile> (\<delta> (X))"
 shows "\<tau> \<Turnstile> (\<delta> ((X::Galaxy) .oclIsTypeOf(Planet)))"
-by(rule OclIsTypeOf\<^sub>P\<^sub>l\<^sub>a\<^sub>n\<^sub>e\<^sub>t_Galaxy_defined[OF isdef[THEN foundation20]])
+by(rule OclIsTypeOf\<^sub>P\<^sub>l\<^sub>a\<^sub>n\<^sub>e\<^sub>t_Galaxy_defined[OF isdef[THEN foundation20]]) 
 lemma OclIsTypeOf\<^sub>P\<^sub>l\<^sub>a\<^sub>n\<^sub>e\<^sub>t_Planet_defined' : 
 assumes isdef: "\<tau> \<Turnstile> (\<delta> (X))"
 shows "\<tau> \<Turnstile> (\<delta> ((X::Planet) .oclIsTypeOf(Planet)))"
-by(rule OclIsTypeOf\<^sub>P\<^sub>l\<^sub>a\<^sub>n\<^sub>e\<^sub>t_Planet_defined[OF isdef[THEN foundation20]])
+by(rule OclIsTypeOf\<^sub>P\<^sub>l\<^sub>a\<^sub>n\<^sub>e\<^sub>t_Planet_defined[OF isdef[THEN foundation20]]) 
 lemma OclIsTypeOf\<^sub>P\<^sub>l\<^sub>a\<^sub>n\<^sub>e\<^sub>t_Person_defined' : 
 assumes isdef: "\<tau> \<Turnstile> (\<delta> (X))"
 shows "\<tau> \<Turnstile> (\<delta> ((X::Person) .oclIsTypeOf(Planet)))"
-by(rule OclIsTypeOf\<^sub>P\<^sub>l\<^sub>a\<^sub>n\<^sub>e\<^sub>t_Person_defined[OF isdef[THEN foundation20]])
+by(rule OclIsTypeOf\<^sub>P\<^sub>l\<^sub>a\<^sub>n\<^sub>e\<^sub>t_Person_defined[OF isdef[THEN foundation20]]) 
 lemma OclIsTypeOf\<^sub>G\<^sub>a\<^sub>l\<^sub>a\<^sub>x\<^sub>y_OclAny_defined' : 
 assumes isdef: "\<tau> \<Turnstile> (\<delta> (X))"
 shows "\<tau> \<Turnstile> (\<delta> ((X::OclAny) .oclIsTypeOf(Galaxy)))"
-by(rule OclIsTypeOf\<^sub>G\<^sub>a\<^sub>l\<^sub>a\<^sub>x\<^sub>y_OclAny_defined[OF isdef[THEN foundation20]])
+by(rule OclIsTypeOf\<^sub>G\<^sub>a\<^sub>l\<^sub>a\<^sub>x\<^sub>y_OclAny_defined[OF isdef[THEN foundation20]]) 
 lemma OclIsTypeOf\<^sub>G\<^sub>a\<^sub>l\<^sub>a\<^sub>x\<^sub>y_Galaxy_defined' : 
 assumes isdef: "\<tau> \<Turnstile> (\<delta> (X))"
 shows "\<tau> \<Turnstile> (\<delta> ((X::Galaxy) .oclIsTypeOf(Galaxy)))"
-by(rule OclIsTypeOf\<^sub>G\<^sub>a\<^sub>l\<^sub>a\<^sub>x\<^sub>y_Galaxy_defined[OF isdef[THEN foundation20]])
+by(rule OclIsTypeOf\<^sub>G\<^sub>a\<^sub>l\<^sub>a\<^sub>x\<^sub>y_Galaxy_defined[OF isdef[THEN foundation20]]) 
 lemma OclIsTypeOf\<^sub>G\<^sub>a\<^sub>l\<^sub>a\<^sub>x\<^sub>y_Planet_defined' : 
 assumes isdef: "\<tau> \<Turnstile> (\<delta> (X))"
 shows "\<tau> \<Turnstile> (\<delta> ((X::Planet) .oclIsTypeOf(Galaxy)))"
-by(rule OclIsTypeOf\<^sub>G\<^sub>a\<^sub>l\<^sub>a\<^sub>x\<^sub>y_Planet_defined[OF isdef[THEN foundation20]])
+by(rule OclIsTypeOf\<^sub>G\<^sub>a\<^sub>l\<^sub>a\<^sub>x\<^sub>y_Planet_defined[OF isdef[THEN foundation20]]) 
 lemma OclIsTypeOf\<^sub>G\<^sub>a\<^sub>l\<^sub>a\<^sub>x\<^sub>y_Person_defined' : 
 assumes isdef: "\<tau> \<Turnstile> (\<delta> (X))"
 shows "\<tau> \<Turnstile> (\<delta> ((X::Person) .oclIsTypeOf(Galaxy)))"
-by(rule OclIsTypeOf\<^sub>G\<^sub>a\<^sub>l\<^sub>a\<^sub>x\<^sub>y_Person_defined[OF isdef[THEN foundation20]])
+by(rule OclIsTypeOf\<^sub>G\<^sub>a\<^sub>l\<^sub>a\<^sub>x\<^sub>y_Person_defined[OF isdef[THEN foundation20]]) 
 lemma OclIsTypeOf\<^sub>O\<^sub>c\<^sub>l\<^sub>A\<^sub>n\<^sub>y_OclAny_defined' : 
 assumes isdef: "\<tau> \<Turnstile> (\<delta> (X))"
 shows "\<tau> \<Turnstile> (\<delta> ((X::OclAny) .oclIsTypeOf(OclAny)))"
-by(rule OclIsTypeOf\<^sub>O\<^sub>c\<^sub>l\<^sub>A\<^sub>n\<^sub>y_OclAny_defined[OF isdef[THEN foundation20]])
+by(rule OclIsTypeOf\<^sub>O\<^sub>c\<^sub>l\<^sub>A\<^sub>n\<^sub>y_OclAny_defined[OF isdef[THEN foundation20]]) 
 lemma OclIsTypeOf\<^sub>O\<^sub>c\<^sub>l\<^sub>A\<^sub>n\<^sub>y_Galaxy_defined' : 
 assumes isdef: "\<tau> \<Turnstile> (\<delta> (X))"
 shows "\<tau> \<Turnstile> (\<delta> ((X::Galaxy) .oclIsTypeOf(OclAny)))"
-by(rule OclIsTypeOf\<^sub>O\<^sub>c\<^sub>l\<^sub>A\<^sub>n\<^sub>y_Galaxy_defined[OF isdef[THEN foundation20]])
+by(rule OclIsTypeOf\<^sub>O\<^sub>c\<^sub>l\<^sub>A\<^sub>n\<^sub>y_Galaxy_defined[OF isdef[THEN foundation20]]) 
 lemma OclIsTypeOf\<^sub>O\<^sub>c\<^sub>l\<^sub>A\<^sub>n\<^sub>y_Planet_defined' : 
 assumes isdef: "\<tau> \<Turnstile> (\<delta> (X))"
 shows "\<tau> \<Turnstile> (\<delta> ((X::Planet) .oclIsTypeOf(OclAny)))"
-by(rule OclIsTypeOf\<^sub>O\<^sub>c\<^sub>l\<^sub>A\<^sub>n\<^sub>y_Planet_defined[OF isdef[THEN foundation20]])
+by(rule OclIsTypeOf\<^sub>O\<^sub>c\<^sub>l\<^sub>A\<^sub>n\<^sub>y_Planet_defined[OF isdef[THEN foundation20]]) 
 lemma OclIsTypeOf\<^sub>O\<^sub>c\<^sub>l\<^sub>A\<^sub>n\<^sub>y_Person_defined' : 
 assumes isdef: "\<tau> \<Turnstile> (\<delta> (X))"
 shows "\<tau> \<Turnstile> (\<delta> ((X::Person) .oclIsTypeOf(OclAny)))"
-by(rule OclIsTypeOf\<^sub>O\<^sub>c\<^sub>l\<^sub>A\<^sub>n\<^sub>y_Person_defined[OF isdef[THEN foundation20]])
+by(rule OclIsTypeOf\<^sub>O\<^sub>c\<^sub>l\<^sub>A\<^sub>n\<^sub>y_Person_defined[OF isdef[THEN foundation20]]) 
 
 (* 60 ************************************ 351 + 1 *)
 subsection{* Up Down Casting *}
@@ -1258,32 +1258,32 @@ lemma actualType\<^sub>P\<^sub>e\<^sub>r\<^sub>s\<^sub>o\<^sub>n_larger_staticTy
 assumes isdef: "\<tau> \<Turnstile> (\<delta> (X))"
 shows "\<tau> \<Turnstile> ((X::Person) .oclIsTypeOf(Planet)) \<triangleq> false"
   using isdef
-by(auto simp: OclIsTypeOf\<^sub>P\<^sub>l\<^sub>a\<^sub>n\<^sub>e\<^sub>t_Person foundation22 foundation16 null_option_def bot_option_def)
+by(auto simp: OclIsTypeOf\<^sub>P\<^sub>l\<^sub>a\<^sub>n\<^sub>e\<^sub>t_Person foundation22 foundation16 null_option_def bot_option_def) 
 lemma actualType\<^sub>P\<^sub>e\<^sub>r\<^sub>s\<^sub>o\<^sub>n_larger_staticType\<^sub>G\<^sub>a\<^sub>l\<^sub>a\<^sub>x\<^sub>y : 
 assumes isdef: "\<tau> \<Turnstile> (\<delta> (X))"
 shows "\<tau> \<Turnstile> ((X::Person) .oclIsTypeOf(Galaxy)) \<triangleq> false"
   using isdef
-by(auto simp: OclIsTypeOf\<^sub>G\<^sub>a\<^sub>l\<^sub>a\<^sub>x\<^sub>y_Person foundation22 foundation16 null_option_def bot_option_def)
+by(auto simp: OclIsTypeOf\<^sub>G\<^sub>a\<^sub>l\<^sub>a\<^sub>x\<^sub>y_Person foundation22 foundation16 null_option_def bot_option_def) 
 lemma actualType\<^sub>P\<^sub>e\<^sub>r\<^sub>s\<^sub>o\<^sub>n_larger_staticType\<^sub>O\<^sub>c\<^sub>l\<^sub>A\<^sub>n\<^sub>y : 
 assumes isdef: "\<tau> \<Turnstile> (\<delta> (X))"
 shows "\<tau> \<Turnstile> ((X::Person) .oclIsTypeOf(OclAny)) \<triangleq> false"
   using isdef
-by(auto simp: OclIsTypeOf\<^sub>O\<^sub>c\<^sub>l\<^sub>A\<^sub>n\<^sub>y_Person foundation22 foundation16 null_option_def bot_option_def)
+by(auto simp: OclIsTypeOf\<^sub>O\<^sub>c\<^sub>l\<^sub>A\<^sub>n\<^sub>y_Person foundation22 foundation16 null_option_def bot_option_def) 
 lemma actualType\<^sub>P\<^sub>l\<^sub>a\<^sub>n\<^sub>e\<^sub>t_larger_staticType\<^sub>G\<^sub>a\<^sub>l\<^sub>a\<^sub>x\<^sub>y : 
 assumes isdef: "\<tau> \<Turnstile> (\<delta> (X))"
 shows "\<tau> \<Turnstile> ((X::Planet) .oclIsTypeOf(Galaxy)) \<triangleq> false"
   using isdef
-by(auto simp: OclIsTypeOf\<^sub>G\<^sub>a\<^sub>l\<^sub>a\<^sub>x\<^sub>y_Planet foundation22 foundation16 null_option_def bot_option_def)
+by(auto simp: OclIsTypeOf\<^sub>G\<^sub>a\<^sub>l\<^sub>a\<^sub>x\<^sub>y_Planet foundation22 foundation16 null_option_def bot_option_def) 
 lemma actualType\<^sub>P\<^sub>l\<^sub>a\<^sub>n\<^sub>e\<^sub>t_larger_staticType\<^sub>O\<^sub>c\<^sub>l\<^sub>A\<^sub>n\<^sub>y : 
 assumes isdef: "\<tau> \<Turnstile> (\<delta> (X))"
 shows "\<tau> \<Turnstile> ((X::Planet) .oclIsTypeOf(OclAny)) \<triangleq> false"
   using isdef
-by(auto simp: OclIsTypeOf\<^sub>O\<^sub>c\<^sub>l\<^sub>A\<^sub>n\<^sub>y_Planet foundation22 foundation16 null_option_def bot_option_def)
+by(auto simp: OclIsTypeOf\<^sub>O\<^sub>c\<^sub>l\<^sub>A\<^sub>n\<^sub>y_Planet foundation22 foundation16 null_option_def bot_option_def) 
 lemma actualType\<^sub>G\<^sub>a\<^sub>l\<^sub>a\<^sub>x\<^sub>y_larger_staticType\<^sub>O\<^sub>c\<^sub>l\<^sub>A\<^sub>n\<^sub>y : 
 assumes isdef: "\<tau> \<Turnstile> (\<delta> (X))"
 shows "\<tau> \<Turnstile> ((X::Galaxy) .oclIsTypeOf(OclAny)) \<triangleq> false"
   using isdef
-by(auto simp: OclIsTypeOf\<^sub>O\<^sub>c\<^sub>l\<^sub>A\<^sub>n\<^sub>y_Galaxy foundation22 foundation16 null_option_def bot_option_def)
+by(auto simp: OclIsTypeOf\<^sub>O\<^sub>c\<^sub>l\<^sub>A\<^sub>n\<^sub>y_Galaxy foundation22 foundation16 null_option_def bot_option_def) 
 
 (* 62 ************************************ 358 + 10 *)
 lemma down_cast_type\<^sub>P\<^sub>l\<^sub>a\<^sub>n\<^sub>e\<^sub>t_from_Planet_to_Person : 
@@ -1292,70 +1292,70 @@ assumes isdef: "\<tau> \<Turnstile> (\<delta> (X))"
 shows "\<tau> \<Turnstile> (X .oclAsType(Person)) \<triangleq> invalid"
   using istyp isdef
   apply(auto simp: OclAsType\<^sub>P\<^sub>e\<^sub>r\<^sub>s\<^sub>o\<^sub>n_Planet foundation22 foundation16 null_option_def bot_option_def split: type\<^sub>P\<^sub>l\<^sub>a\<^sub>n\<^sub>e\<^sub>t.split typeoid\<^sub>P\<^sub>l\<^sub>a\<^sub>n\<^sub>e\<^sub>t.split)
-by(simp add: OclValid_def false_def true_def)
+by(simp add: OclValid_def false_def true_def) 
 lemma down_cast_type\<^sub>G\<^sub>a\<^sub>l\<^sub>a\<^sub>x\<^sub>y_from_Galaxy_to_Person : 
 assumes istyp: "\<tau> \<Turnstile> ((X::Galaxy) .oclIsTypeOf(Galaxy))"
 assumes isdef: "\<tau> \<Turnstile> (\<delta> (X))"
 shows "\<tau> \<Turnstile> (X .oclAsType(Person)) \<triangleq> invalid"
   using istyp isdef
   apply(auto simp: OclAsType\<^sub>P\<^sub>e\<^sub>r\<^sub>s\<^sub>o\<^sub>n_Galaxy foundation22 foundation16 null_option_def bot_option_def split: type\<^sub>G\<^sub>a\<^sub>l\<^sub>a\<^sub>x\<^sub>y.split typeoid\<^sub>G\<^sub>a\<^sub>l\<^sub>a\<^sub>x\<^sub>y.split)
-by(simp add: OclValid_def false_def true_def)
+by(simp add: OclValid_def false_def true_def) 
 lemma down_cast_type\<^sub>O\<^sub>c\<^sub>l\<^sub>A\<^sub>n\<^sub>y_from_OclAny_to_Person : 
 assumes istyp: "\<tau> \<Turnstile> ((X::OclAny) .oclIsTypeOf(OclAny))"
 assumes isdef: "\<tau> \<Turnstile> (\<delta> (X))"
 shows "\<tau> \<Turnstile> (X .oclAsType(Person)) \<triangleq> invalid"
   using istyp isdef
   apply(auto simp: OclAsType\<^sub>P\<^sub>e\<^sub>r\<^sub>s\<^sub>o\<^sub>n_OclAny foundation22 foundation16 null_option_def bot_option_def split: type\<^sub>O\<^sub>c\<^sub>l\<^sub>A\<^sub>n\<^sub>y.split typeoid\<^sub>O\<^sub>c\<^sub>l\<^sub>A\<^sub>n\<^sub>y.split)
-by(simp add: OclValid_def false_def true_def)
+by(simp add: OclValid_def false_def true_def) 
 lemma down_cast_type\<^sub>G\<^sub>a\<^sub>l\<^sub>a\<^sub>x\<^sub>y_from_Galaxy_to_Planet : 
 assumes istyp: "\<tau> \<Turnstile> ((X::Galaxy) .oclIsTypeOf(Galaxy))"
 assumes isdef: "\<tau> \<Turnstile> (\<delta> (X))"
 shows "\<tau> \<Turnstile> (X .oclAsType(Planet)) \<triangleq> invalid"
   using istyp isdef
   apply(auto simp: OclAsType\<^sub>P\<^sub>l\<^sub>a\<^sub>n\<^sub>e\<^sub>t_Galaxy foundation22 foundation16 null_option_def bot_option_def split: type\<^sub>G\<^sub>a\<^sub>l\<^sub>a\<^sub>x\<^sub>y.split typeoid\<^sub>G\<^sub>a\<^sub>l\<^sub>a\<^sub>x\<^sub>y.split)
-by(simp add: OclValid_def false_def true_def)
+by(simp add: OclValid_def false_def true_def) 
 lemma down_cast_type\<^sub>O\<^sub>c\<^sub>l\<^sub>A\<^sub>n\<^sub>y_from_OclAny_to_Planet : 
 assumes istyp: "\<tau> \<Turnstile> ((X::OclAny) .oclIsTypeOf(OclAny))"
 assumes isdef: "\<tau> \<Turnstile> (\<delta> (X))"
 shows "\<tau> \<Turnstile> (X .oclAsType(Planet)) \<triangleq> invalid"
   using istyp isdef
   apply(auto simp: OclAsType\<^sub>P\<^sub>l\<^sub>a\<^sub>n\<^sub>e\<^sub>t_OclAny foundation22 foundation16 null_option_def bot_option_def split: type\<^sub>O\<^sub>c\<^sub>l\<^sub>A\<^sub>n\<^sub>y.split typeoid\<^sub>O\<^sub>c\<^sub>l\<^sub>A\<^sub>n\<^sub>y.split)
-by(simp add: OclValid_def false_def true_def)
+by(simp add: OclValid_def false_def true_def) 
 lemma down_cast_type\<^sub>O\<^sub>c\<^sub>l\<^sub>A\<^sub>n\<^sub>y_from_OclAny_to_Galaxy : 
 assumes istyp: "\<tau> \<Turnstile> ((X::OclAny) .oclIsTypeOf(OclAny))"
 assumes isdef: "\<tau> \<Turnstile> (\<delta> (X))"
 shows "\<tau> \<Turnstile> (X .oclAsType(Galaxy)) \<triangleq> invalid"
   using istyp isdef
   apply(auto simp: OclAsType\<^sub>G\<^sub>a\<^sub>l\<^sub>a\<^sub>x\<^sub>y_OclAny foundation22 foundation16 null_option_def bot_option_def split: type\<^sub>O\<^sub>c\<^sub>l\<^sub>A\<^sub>n\<^sub>y.split typeoid\<^sub>O\<^sub>c\<^sub>l\<^sub>A\<^sub>n\<^sub>y.split)
-by(simp add: OclValid_def false_def true_def)
+by(simp add: OclValid_def false_def true_def) 
 lemma down_cast_type\<^sub>P\<^sub>l\<^sub>a\<^sub>n\<^sub>e\<^sub>t_from_Galaxy_to_Person : 
 assumes istyp: "\<tau> \<Turnstile> ((X::Galaxy) .oclIsTypeOf(Planet))"
 assumes isdef: "\<tau> \<Turnstile> (\<delta> (X))"
 shows "\<tau> \<Turnstile> (X .oclAsType(Person)) \<triangleq> invalid"
   using istyp isdef
   apply(auto simp: OclAsType\<^sub>P\<^sub>e\<^sub>r\<^sub>s\<^sub>o\<^sub>n_Galaxy foundation22 foundation16 null_option_def bot_option_def split: type\<^sub>G\<^sub>a\<^sub>l\<^sub>a\<^sub>x\<^sub>y.split typeoid\<^sub>G\<^sub>a\<^sub>l\<^sub>a\<^sub>x\<^sub>y.split)
-by(simp add: OclIsTypeOf\<^sub>P\<^sub>l\<^sub>a\<^sub>n\<^sub>e\<^sub>t_Galaxy OclValid_def false_def true_def)
+by(simp add: OclIsTypeOf\<^sub>P\<^sub>l\<^sub>a\<^sub>n\<^sub>e\<^sub>t_Galaxy OclValid_def false_def true_def) 
 lemma down_cast_type\<^sub>P\<^sub>l\<^sub>a\<^sub>n\<^sub>e\<^sub>t_from_OclAny_to_Person : 
 assumes istyp: "\<tau> \<Turnstile> ((X::OclAny) .oclIsTypeOf(Planet))"
 assumes isdef: "\<tau> \<Turnstile> (\<delta> (X))"
 shows "\<tau> \<Turnstile> (X .oclAsType(Person)) \<triangleq> invalid"
   using istyp isdef
   apply(auto simp: OclAsType\<^sub>P\<^sub>e\<^sub>r\<^sub>s\<^sub>o\<^sub>n_OclAny foundation22 foundation16 null_option_def bot_option_def split: type\<^sub>O\<^sub>c\<^sub>l\<^sub>A\<^sub>n\<^sub>y.split typeoid\<^sub>O\<^sub>c\<^sub>l\<^sub>A\<^sub>n\<^sub>y.split)
-by(simp add: OclIsTypeOf\<^sub>P\<^sub>l\<^sub>a\<^sub>n\<^sub>e\<^sub>t_OclAny OclValid_def false_def true_def)
+by(simp add: OclIsTypeOf\<^sub>P\<^sub>l\<^sub>a\<^sub>n\<^sub>e\<^sub>t_OclAny OclValid_def false_def true_def) 
 lemma down_cast_type\<^sub>G\<^sub>a\<^sub>l\<^sub>a\<^sub>x\<^sub>y_from_OclAny_to_Person : 
 assumes istyp: "\<tau> \<Turnstile> ((X::OclAny) .oclIsTypeOf(Galaxy))"
 assumes isdef: "\<tau> \<Turnstile> (\<delta> (X))"
 shows "\<tau> \<Turnstile> (X .oclAsType(Person)) \<triangleq> invalid"
   using istyp isdef
   apply(auto simp: OclAsType\<^sub>P\<^sub>e\<^sub>r\<^sub>s\<^sub>o\<^sub>n_OclAny foundation22 foundation16 null_option_def bot_option_def split: type\<^sub>O\<^sub>c\<^sub>l\<^sub>A\<^sub>n\<^sub>y.split typeoid\<^sub>O\<^sub>c\<^sub>l\<^sub>A\<^sub>n\<^sub>y.split)
-by(simp add: OclIsTypeOf\<^sub>G\<^sub>a\<^sub>l\<^sub>a\<^sub>x\<^sub>y_OclAny OclValid_def false_def true_def)
+by(simp add: OclIsTypeOf\<^sub>G\<^sub>a\<^sub>l\<^sub>a\<^sub>x\<^sub>y_OclAny OclValid_def false_def true_def) 
 lemma down_cast_type\<^sub>G\<^sub>a\<^sub>l\<^sub>a\<^sub>x\<^sub>y_from_OclAny_to_Planet : 
 assumes istyp: "\<tau> \<Turnstile> ((X::OclAny) .oclIsTypeOf(Galaxy))"
 assumes isdef: "\<tau> \<Turnstile> (\<delta> (X))"
 shows "\<tau> \<Turnstile> (X .oclAsType(Planet)) \<triangleq> invalid"
   using istyp isdef
   apply(auto simp: OclAsType\<^sub>P\<^sub>l\<^sub>a\<^sub>n\<^sub>e\<^sub>t_OclAny foundation22 foundation16 null_option_def bot_option_def split: type\<^sub>O\<^sub>c\<^sub>l\<^sub>A\<^sub>n\<^sub>y.split typeoid\<^sub>O\<^sub>c\<^sub>l\<^sub>A\<^sub>n\<^sub>y.split)
-by(simp add: OclIsTypeOf\<^sub>G\<^sub>a\<^sub>l\<^sub>a\<^sub>x\<^sub>y_OclAny OclValid_def false_def true_def)
+by(simp add: OclIsTypeOf\<^sub>G\<^sub>a\<^sub>l\<^sub>a\<^sub>x\<^sub>y_OclAny OclValid_def false_def true_def) 
 
 (* 63 ************************************ 368 + 1 *)
 section{* OclIsKindOf *}
@@ -1816,133 +1816,133 @@ subsection{* Validity and Definedness Properties *}
 lemma OclIsKindOf\<^sub>P\<^sub>e\<^sub>r\<^sub>s\<^sub>o\<^sub>n_OclAny_defined : 
 assumes isdef: "\<tau> \<Turnstile> (\<upsilon> (X))"
 shows "\<tau> \<Turnstile> (\<delta> ((X::OclAny) .oclIsKindOf(Person)))"
-by(simp only: OclIsKindOf\<^sub>P\<^sub>e\<^sub>r\<^sub>s\<^sub>o\<^sub>n_OclAny, rule OclIsTypeOf\<^sub>P\<^sub>e\<^sub>r\<^sub>s\<^sub>o\<^sub>n_OclAny_defined[OF isdef])
+by(simp only: OclIsKindOf\<^sub>P\<^sub>e\<^sub>r\<^sub>s\<^sub>o\<^sub>n_OclAny, rule OclIsTypeOf\<^sub>P\<^sub>e\<^sub>r\<^sub>s\<^sub>o\<^sub>n_OclAny_defined[OF isdef]) 
 lemma OclIsKindOf\<^sub>P\<^sub>e\<^sub>r\<^sub>s\<^sub>o\<^sub>n_Galaxy_defined : 
 assumes isdef: "\<tau> \<Turnstile> (\<upsilon> (X))"
 shows "\<tau> \<Turnstile> (\<delta> ((X::Galaxy) .oclIsKindOf(Person)))"
-by(simp only: OclIsKindOf\<^sub>P\<^sub>e\<^sub>r\<^sub>s\<^sub>o\<^sub>n_Galaxy, rule OclIsTypeOf\<^sub>P\<^sub>e\<^sub>r\<^sub>s\<^sub>o\<^sub>n_Galaxy_defined[OF isdef])
+by(simp only: OclIsKindOf\<^sub>P\<^sub>e\<^sub>r\<^sub>s\<^sub>o\<^sub>n_Galaxy, rule OclIsTypeOf\<^sub>P\<^sub>e\<^sub>r\<^sub>s\<^sub>o\<^sub>n_Galaxy_defined[OF isdef]) 
 lemma OclIsKindOf\<^sub>P\<^sub>e\<^sub>r\<^sub>s\<^sub>o\<^sub>n_Planet_defined : 
 assumes isdef: "\<tau> \<Turnstile> (\<upsilon> (X))"
 shows "\<tau> \<Turnstile> (\<delta> ((X::Planet) .oclIsKindOf(Person)))"
-by(simp only: OclIsKindOf\<^sub>P\<^sub>e\<^sub>r\<^sub>s\<^sub>o\<^sub>n_Planet, rule OclIsTypeOf\<^sub>P\<^sub>e\<^sub>r\<^sub>s\<^sub>o\<^sub>n_Planet_defined[OF isdef])
+by(simp only: OclIsKindOf\<^sub>P\<^sub>e\<^sub>r\<^sub>s\<^sub>o\<^sub>n_Planet, rule OclIsTypeOf\<^sub>P\<^sub>e\<^sub>r\<^sub>s\<^sub>o\<^sub>n_Planet_defined[OF isdef]) 
 lemma OclIsKindOf\<^sub>P\<^sub>e\<^sub>r\<^sub>s\<^sub>o\<^sub>n_Person_defined : 
 assumes isdef: "\<tau> \<Turnstile> (\<upsilon> (X))"
 shows "\<tau> \<Turnstile> (\<delta> ((X::Person) .oclIsKindOf(Person)))"
-by(simp only: OclIsKindOf\<^sub>P\<^sub>e\<^sub>r\<^sub>s\<^sub>o\<^sub>n_Person, rule OclIsTypeOf\<^sub>P\<^sub>e\<^sub>r\<^sub>s\<^sub>o\<^sub>n_Person_defined[OF isdef])
+by(simp only: OclIsKindOf\<^sub>P\<^sub>e\<^sub>r\<^sub>s\<^sub>o\<^sub>n_Person, rule OclIsTypeOf\<^sub>P\<^sub>e\<^sub>r\<^sub>s\<^sub>o\<^sub>n_Person_defined[OF isdef]) 
 lemma OclIsKindOf\<^sub>P\<^sub>l\<^sub>a\<^sub>n\<^sub>e\<^sub>t_OclAny_defined : 
 assumes isdef: "\<tau> \<Turnstile> (\<upsilon> (X))"
 shows "\<tau> \<Turnstile> (\<delta> ((X::OclAny) .oclIsKindOf(Planet)))"
-by(simp only: OclIsKindOf\<^sub>P\<^sub>l\<^sub>a\<^sub>n\<^sub>e\<^sub>t_OclAny, rule defined_or_I[OF OclIsTypeOf\<^sub>P\<^sub>l\<^sub>a\<^sub>n\<^sub>e\<^sub>t_OclAny_defined[OF isdef], OF OclIsKindOf\<^sub>P\<^sub>e\<^sub>r\<^sub>s\<^sub>o\<^sub>n_OclAny_defined[OF isdef]])
+by(simp only: OclIsKindOf\<^sub>P\<^sub>l\<^sub>a\<^sub>n\<^sub>e\<^sub>t_OclAny, rule defined_or_I[OF OclIsTypeOf\<^sub>P\<^sub>l\<^sub>a\<^sub>n\<^sub>e\<^sub>t_OclAny_defined[OF isdef], OF OclIsKindOf\<^sub>P\<^sub>e\<^sub>r\<^sub>s\<^sub>o\<^sub>n_OclAny_defined[OF isdef]]) 
 lemma OclIsKindOf\<^sub>P\<^sub>l\<^sub>a\<^sub>n\<^sub>e\<^sub>t_Galaxy_defined : 
 assumes isdef: "\<tau> \<Turnstile> (\<upsilon> (X))"
 shows "\<tau> \<Turnstile> (\<delta> ((X::Galaxy) .oclIsKindOf(Planet)))"
-by(simp only: OclIsKindOf\<^sub>P\<^sub>l\<^sub>a\<^sub>n\<^sub>e\<^sub>t_Galaxy, rule defined_or_I[OF OclIsTypeOf\<^sub>P\<^sub>l\<^sub>a\<^sub>n\<^sub>e\<^sub>t_Galaxy_defined[OF isdef], OF OclIsKindOf\<^sub>P\<^sub>e\<^sub>r\<^sub>s\<^sub>o\<^sub>n_Galaxy_defined[OF isdef]])
+by(simp only: OclIsKindOf\<^sub>P\<^sub>l\<^sub>a\<^sub>n\<^sub>e\<^sub>t_Galaxy, rule defined_or_I[OF OclIsTypeOf\<^sub>P\<^sub>l\<^sub>a\<^sub>n\<^sub>e\<^sub>t_Galaxy_defined[OF isdef], OF OclIsKindOf\<^sub>P\<^sub>e\<^sub>r\<^sub>s\<^sub>o\<^sub>n_Galaxy_defined[OF isdef]]) 
 lemma OclIsKindOf\<^sub>P\<^sub>l\<^sub>a\<^sub>n\<^sub>e\<^sub>t_Planet_defined : 
 assumes isdef: "\<tau> \<Turnstile> (\<upsilon> (X))"
 shows "\<tau> \<Turnstile> (\<delta> ((X::Planet) .oclIsKindOf(Planet)))"
-by(simp only: OclIsKindOf\<^sub>P\<^sub>l\<^sub>a\<^sub>n\<^sub>e\<^sub>t_Planet, rule defined_or_I[OF OclIsTypeOf\<^sub>P\<^sub>l\<^sub>a\<^sub>n\<^sub>e\<^sub>t_Planet_defined[OF isdef], OF OclIsKindOf\<^sub>P\<^sub>e\<^sub>r\<^sub>s\<^sub>o\<^sub>n_Planet_defined[OF isdef]])
+by(simp only: OclIsKindOf\<^sub>P\<^sub>l\<^sub>a\<^sub>n\<^sub>e\<^sub>t_Planet, rule defined_or_I[OF OclIsTypeOf\<^sub>P\<^sub>l\<^sub>a\<^sub>n\<^sub>e\<^sub>t_Planet_defined[OF isdef], OF OclIsKindOf\<^sub>P\<^sub>e\<^sub>r\<^sub>s\<^sub>o\<^sub>n_Planet_defined[OF isdef]]) 
 lemma OclIsKindOf\<^sub>P\<^sub>l\<^sub>a\<^sub>n\<^sub>e\<^sub>t_Person_defined : 
 assumes isdef: "\<tau> \<Turnstile> (\<upsilon> (X))"
 shows "\<tau> \<Turnstile> (\<delta> ((X::Person) .oclIsKindOf(Planet)))"
-by(simp only: OclIsKindOf\<^sub>P\<^sub>l\<^sub>a\<^sub>n\<^sub>e\<^sub>t_Person, rule defined_or_I[OF OclIsTypeOf\<^sub>P\<^sub>l\<^sub>a\<^sub>n\<^sub>e\<^sub>t_Person_defined[OF isdef], OF OclIsKindOf\<^sub>P\<^sub>e\<^sub>r\<^sub>s\<^sub>o\<^sub>n_Person_defined[OF isdef]])
+by(simp only: OclIsKindOf\<^sub>P\<^sub>l\<^sub>a\<^sub>n\<^sub>e\<^sub>t_Person, rule defined_or_I[OF OclIsTypeOf\<^sub>P\<^sub>l\<^sub>a\<^sub>n\<^sub>e\<^sub>t_Person_defined[OF isdef], OF OclIsKindOf\<^sub>P\<^sub>e\<^sub>r\<^sub>s\<^sub>o\<^sub>n_Person_defined[OF isdef]]) 
 lemma OclIsKindOf\<^sub>G\<^sub>a\<^sub>l\<^sub>a\<^sub>x\<^sub>y_OclAny_defined : 
 assumes isdef: "\<tau> \<Turnstile> (\<upsilon> (X))"
 shows "\<tau> \<Turnstile> (\<delta> ((X::OclAny) .oclIsKindOf(Galaxy)))"
-by(simp only: OclIsKindOf\<^sub>G\<^sub>a\<^sub>l\<^sub>a\<^sub>x\<^sub>y_OclAny, rule defined_or_I[OF OclIsTypeOf\<^sub>G\<^sub>a\<^sub>l\<^sub>a\<^sub>x\<^sub>y_OclAny_defined[OF isdef], OF OclIsKindOf\<^sub>P\<^sub>l\<^sub>a\<^sub>n\<^sub>e\<^sub>t_OclAny_defined[OF isdef]])
+by(simp only: OclIsKindOf\<^sub>G\<^sub>a\<^sub>l\<^sub>a\<^sub>x\<^sub>y_OclAny, rule defined_or_I[OF OclIsTypeOf\<^sub>G\<^sub>a\<^sub>l\<^sub>a\<^sub>x\<^sub>y_OclAny_defined[OF isdef], OF OclIsKindOf\<^sub>P\<^sub>l\<^sub>a\<^sub>n\<^sub>e\<^sub>t_OclAny_defined[OF isdef]]) 
 lemma OclIsKindOf\<^sub>G\<^sub>a\<^sub>l\<^sub>a\<^sub>x\<^sub>y_Galaxy_defined : 
 assumes isdef: "\<tau> \<Turnstile> (\<upsilon> (X))"
 shows "\<tau> \<Turnstile> (\<delta> ((X::Galaxy) .oclIsKindOf(Galaxy)))"
-by(simp only: OclIsKindOf\<^sub>G\<^sub>a\<^sub>l\<^sub>a\<^sub>x\<^sub>y_Galaxy, rule defined_or_I[OF OclIsTypeOf\<^sub>G\<^sub>a\<^sub>l\<^sub>a\<^sub>x\<^sub>y_Galaxy_defined[OF isdef], OF OclIsKindOf\<^sub>P\<^sub>l\<^sub>a\<^sub>n\<^sub>e\<^sub>t_Galaxy_defined[OF isdef]])
+by(simp only: OclIsKindOf\<^sub>G\<^sub>a\<^sub>l\<^sub>a\<^sub>x\<^sub>y_Galaxy, rule defined_or_I[OF OclIsTypeOf\<^sub>G\<^sub>a\<^sub>l\<^sub>a\<^sub>x\<^sub>y_Galaxy_defined[OF isdef], OF OclIsKindOf\<^sub>P\<^sub>l\<^sub>a\<^sub>n\<^sub>e\<^sub>t_Galaxy_defined[OF isdef]]) 
 lemma OclIsKindOf\<^sub>G\<^sub>a\<^sub>l\<^sub>a\<^sub>x\<^sub>y_Planet_defined : 
 assumes isdef: "\<tau> \<Turnstile> (\<upsilon> (X))"
 shows "\<tau> \<Turnstile> (\<delta> ((X::Planet) .oclIsKindOf(Galaxy)))"
-by(simp only: OclIsKindOf\<^sub>G\<^sub>a\<^sub>l\<^sub>a\<^sub>x\<^sub>y_Planet, rule defined_or_I[OF OclIsTypeOf\<^sub>G\<^sub>a\<^sub>l\<^sub>a\<^sub>x\<^sub>y_Planet_defined[OF isdef], OF OclIsKindOf\<^sub>P\<^sub>l\<^sub>a\<^sub>n\<^sub>e\<^sub>t_Planet_defined[OF isdef]])
+by(simp only: OclIsKindOf\<^sub>G\<^sub>a\<^sub>l\<^sub>a\<^sub>x\<^sub>y_Planet, rule defined_or_I[OF OclIsTypeOf\<^sub>G\<^sub>a\<^sub>l\<^sub>a\<^sub>x\<^sub>y_Planet_defined[OF isdef], OF OclIsKindOf\<^sub>P\<^sub>l\<^sub>a\<^sub>n\<^sub>e\<^sub>t_Planet_defined[OF isdef]]) 
 lemma OclIsKindOf\<^sub>G\<^sub>a\<^sub>l\<^sub>a\<^sub>x\<^sub>y_Person_defined : 
 assumes isdef: "\<tau> \<Turnstile> (\<upsilon> (X))"
 shows "\<tau> \<Turnstile> (\<delta> ((X::Person) .oclIsKindOf(Galaxy)))"
-by(simp only: OclIsKindOf\<^sub>G\<^sub>a\<^sub>l\<^sub>a\<^sub>x\<^sub>y_Person, rule defined_or_I[OF OclIsTypeOf\<^sub>G\<^sub>a\<^sub>l\<^sub>a\<^sub>x\<^sub>y_Person_defined[OF isdef], OF OclIsKindOf\<^sub>P\<^sub>l\<^sub>a\<^sub>n\<^sub>e\<^sub>t_Person_defined[OF isdef]])
+by(simp only: OclIsKindOf\<^sub>G\<^sub>a\<^sub>l\<^sub>a\<^sub>x\<^sub>y_Person, rule defined_or_I[OF OclIsTypeOf\<^sub>G\<^sub>a\<^sub>l\<^sub>a\<^sub>x\<^sub>y_Person_defined[OF isdef], OF OclIsKindOf\<^sub>P\<^sub>l\<^sub>a\<^sub>n\<^sub>e\<^sub>t_Person_defined[OF isdef]]) 
 lemma OclIsKindOf\<^sub>O\<^sub>c\<^sub>l\<^sub>A\<^sub>n\<^sub>y_OclAny_defined : 
 assumes isdef: "\<tau> \<Turnstile> (\<upsilon> (X))"
 shows "\<tau> \<Turnstile> (\<delta> ((X::OclAny) .oclIsKindOf(OclAny)))"
-by(simp only: OclIsKindOf\<^sub>O\<^sub>c\<^sub>l\<^sub>A\<^sub>n\<^sub>y_OclAny, rule defined_or_I[OF OclIsTypeOf\<^sub>O\<^sub>c\<^sub>l\<^sub>A\<^sub>n\<^sub>y_OclAny_defined[OF isdef], OF OclIsKindOf\<^sub>G\<^sub>a\<^sub>l\<^sub>a\<^sub>x\<^sub>y_OclAny_defined[OF isdef]])
+by(simp only: OclIsKindOf\<^sub>O\<^sub>c\<^sub>l\<^sub>A\<^sub>n\<^sub>y_OclAny, rule defined_or_I[OF OclIsTypeOf\<^sub>O\<^sub>c\<^sub>l\<^sub>A\<^sub>n\<^sub>y_OclAny_defined[OF isdef], OF OclIsKindOf\<^sub>G\<^sub>a\<^sub>l\<^sub>a\<^sub>x\<^sub>y_OclAny_defined[OF isdef]]) 
 lemma OclIsKindOf\<^sub>O\<^sub>c\<^sub>l\<^sub>A\<^sub>n\<^sub>y_Galaxy_defined : 
 assumes isdef: "\<tau> \<Turnstile> (\<upsilon> (X))"
 shows "\<tau> \<Turnstile> (\<delta> ((X::Galaxy) .oclIsKindOf(OclAny)))"
-by(simp only: OclIsKindOf\<^sub>O\<^sub>c\<^sub>l\<^sub>A\<^sub>n\<^sub>y_Galaxy, rule defined_or_I[OF OclIsTypeOf\<^sub>O\<^sub>c\<^sub>l\<^sub>A\<^sub>n\<^sub>y_Galaxy_defined[OF isdef], OF OclIsKindOf\<^sub>G\<^sub>a\<^sub>l\<^sub>a\<^sub>x\<^sub>y_Galaxy_defined[OF isdef]])
+by(simp only: OclIsKindOf\<^sub>O\<^sub>c\<^sub>l\<^sub>A\<^sub>n\<^sub>y_Galaxy, rule defined_or_I[OF OclIsTypeOf\<^sub>O\<^sub>c\<^sub>l\<^sub>A\<^sub>n\<^sub>y_Galaxy_defined[OF isdef], OF OclIsKindOf\<^sub>G\<^sub>a\<^sub>l\<^sub>a\<^sub>x\<^sub>y_Galaxy_defined[OF isdef]]) 
 lemma OclIsKindOf\<^sub>O\<^sub>c\<^sub>l\<^sub>A\<^sub>n\<^sub>y_Planet_defined : 
 assumes isdef: "\<tau> \<Turnstile> (\<upsilon> (X))"
 shows "\<tau> \<Turnstile> (\<delta> ((X::Planet) .oclIsKindOf(OclAny)))"
-by(simp only: OclIsKindOf\<^sub>O\<^sub>c\<^sub>l\<^sub>A\<^sub>n\<^sub>y_Planet, rule defined_or_I[OF OclIsTypeOf\<^sub>O\<^sub>c\<^sub>l\<^sub>A\<^sub>n\<^sub>y_Planet_defined[OF isdef], OF OclIsKindOf\<^sub>G\<^sub>a\<^sub>l\<^sub>a\<^sub>x\<^sub>y_Planet_defined[OF isdef]])
+by(simp only: OclIsKindOf\<^sub>O\<^sub>c\<^sub>l\<^sub>A\<^sub>n\<^sub>y_Planet, rule defined_or_I[OF OclIsTypeOf\<^sub>O\<^sub>c\<^sub>l\<^sub>A\<^sub>n\<^sub>y_Planet_defined[OF isdef], OF OclIsKindOf\<^sub>G\<^sub>a\<^sub>l\<^sub>a\<^sub>x\<^sub>y_Planet_defined[OF isdef]]) 
 lemma OclIsKindOf\<^sub>O\<^sub>c\<^sub>l\<^sub>A\<^sub>n\<^sub>y_Person_defined : 
 assumes isdef: "\<tau> \<Turnstile> (\<upsilon> (X))"
 shows "\<tau> \<Turnstile> (\<delta> ((X::Person) .oclIsKindOf(OclAny)))"
-by(simp only: OclIsKindOf\<^sub>O\<^sub>c\<^sub>l\<^sub>A\<^sub>n\<^sub>y_Person, rule defined_or_I[OF OclIsTypeOf\<^sub>O\<^sub>c\<^sub>l\<^sub>A\<^sub>n\<^sub>y_Person_defined[OF isdef], OF OclIsKindOf\<^sub>G\<^sub>a\<^sub>l\<^sub>a\<^sub>x\<^sub>y_Person_defined[OF isdef]])
+by(simp only: OclIsKindOf\<^sub>O\<^sub>c\<^sub>l\<^sub>A\<^sub>n\<^sub>y_Person, rule defined_or_I[OF OclIsTypeOf\<^sub>O\<^sub>c\<^sub>l\<^sub>A\<^sub>n\<^sub>y_Person_defined[OF isdef], OF OclIsKindOf\<^sub>G\<^sub>a\<^sub>l\<^sub>a\<^sub>x\<^sub>y_Person_defined[OF isdef]]) 
 
 (* 77 ************************************ 512 + 16 *)
 lemma OclIsKindOf\<^sub>P\<^sub>e\<^sub>r\<^sub>s\<^sub>o\<^sub>n_OclAny_defined' : 
 assumes isdef: "\<tau> \<Turnstile> (\<delta> (X))"
 shows "\<tau> \<Turnstile> (\<delta> ((X::OclAny) .oclIsKindOf(Person)))"
-by(rule OclIsKindOf\<^sub>P\<^sub>e\<^sub>r\<^sub>s\<^sub>o\<^sub>n_OclAny_defined[OF isdef[THEN foundation20]])
+by(rule OclIsKindOf\<^sub>P\<^sub>e\<^sub>r\<^sub>s\<^sub>o\<^sub>n_OclAny_defined[OF isdef[THEN foundation20]]) 
 lemma OclIsKindOf\<^sub>P\<^sub>e\<^sub>r\<^sub>s\<^sub>o\<^sub>n_Galaxy_defined' : 
 assumes isdef: "\<tau> \<Turnstile> (\<delta> (X))"
 shows "\<tau> \<Turnstile> (\<delta> ((X::Galaxy) .oclIsKindOf(Person)))"
-by(rule OclIsKindOf\<^sub>P\<^sub>e\<^sub>r\<^sub>s\<^sub>o\<^sub>n_Galaxy_defined[OF isdef[THEN foundation20]])
+by(rule OclIsKindOf\<^sub>P\<^sub>e\<^sub>r\<^sub>s\<^sub>o\<^sub>n_Galaxy_defined[OF isdef[THEN foundation20]]) 
 lemma OclIsKindOf\<^sub>P\<^sub>e\<^sub>r\<^sub>s\<^sub>o\<^sub>n_Planet_defined' : 
 assumes isdef: "\<tau> \<Turnstile> (\<delta> (X))"
 shows "\<tau> \<Turnstile> (\<delta> ((X::Planet) .oclIsKindOf(Person)))"
-by(rule OclIsKindOf\<^sub>P\<^sub>e\<^sub>r\<^sub>s\<^sub>o\<^sub>n_Planet_defined[OF isdef[THEN foundation20]])
+by(rule OclIsKindOf\<^sub>P\<^sub>e\<^sub>r\<^sub>s\<^sub>o\<^sub>n_Planet_defined[OF isdef[THEN foundation20]]) 
 lemma OclIsKindOf\<^sub>P\<^sub>e\<^sub>r\<^sub>s\<^sub>o\<^sub>n_Person_defined' : 
 assumes isdef: "\<tau> \<Turnstile> (\<delta> (X))"
 shows "\<tau> \<Turnstile> (\<delta> ((X::Person) .oclIsKindOf(Person)))"
-by(rule OclIsKindOf\<^sub>P\<^sub>e\<^sub>r\<^sub>s\<^sub>o\<^sub>n_Person_defined[OF isdef[THEN foundation20]])
+by(rule OclIsKindOf\<^sub>P\<^sub>e\<^sub>r\<^sub>s\<^sub>o\<^sub>n_Person_defined[OF isdef[THEN foundation20]]) 
 lemma OclIsKindOf\<^sub>P\<^sub>l\<^sub>a\<^sub>n\<^sub>e\<^sub>t_OclAny_defined' : 
 assumes isdef: "\<tau> \<Turnstile> (\<delta> (X))"
 shows "\<tau> \<Turnstile> (\<delta> ((X::OclAny) .oclIsKindOf(Planet)))"
-by(rule OclIsKindOf\<^sub>P\<^sub>l\<^sub>a\<^sub>n\<^sub>e\<^sub>t_OclAny_defined[OF isdef[THEN foundation20]])
+by(rule OclIsKindOf\<^sub>P\<^sub>l\<^sub>a\<^sub>n\<^sub>e\<^sub>t_OclAny_defined[OF isdef[THEN foundation20]]) 
 lemma OclIsKindOf\<^sub>P\<^sub>l\<^sub>a\<^sub>n\<^sub>e\<^sub>t_Galaxy_defined' : 
 assumes isdef: "\<tau> \<Turnstile> (\<delta> (X))"
 shows "\<tau> \<Turnstile> (\<delta> ((X::Galaxy) .oclIsKindOf(Planet)))"
-by(rule OclIsKindOf\<^sub>P\<^sub>l\<^sub>a\<^sub>n\<^sub>e\<^sub>t_Galaxy_defined[OF isdef[THEN foundation20]])
+by(rule OclIsKindOf\<^sub>P\<^sub>l\<^sub>a\<^sub>n\<^sub>e\<^sub>t_Galaxy_defined[OF isdef[THEN foundation20]]) 
 lemma OclIsKindOf\<^sub>P\<^sub>l\<^sub>a\<^sub>n\<^sub>e\<^sub>t_Planet_defined' : 
 assumes isdef: "\<tau> \<Turnstile> (\<delta> (X))"
 shows "\<tau> \<Turnstile> (\<delta> ((X::Planet) .oclIsKindOf(Planet)))"
-by(rule OclIsKindOf\<^sub>P\<^sub>l\<^sub>a\<^sub>n\<^sub>e\<^sub>t_Planet_defined[OF isdef[THEN foundation20]])
+by(rule OclIsKindOf\<^sub>P\<^sub>l\<^sub>a\<^sub>n\<^sub>e\<^sub>t_Planet_defined[OF isdef[THEN foundation20]]) 
 lemma OclIsKindOf\<^sub>P\<^sub>l\<^sub>a\<^sub>n\<^sub>e\<^sub>t_Person_defined' : 
 assumes isdef: "\<tau> \<Turnstile> (\<delta> (X))"
 shows "\<tau> \<Turnstile> (\<delta> ((X::Person) .oclIsKindOf(Planet)))"
-by(rule OclIsKindOf\<^sub>P\<^sub>l\<^sub>a\<^sub>n\<^sub>e\<^sub>t_Person_defined[OF isdef[THEN foundation20]])
+by(rule OclIsKindOf\<^sub>P\<^sub>l\<^sub>a\<^sub>n\<^sub>e\<^sub>t_Person_defined[OF isdef[THEN foundation20]]) 
 lemma OclIsKindOf\<^sub>G\<^sub>a\<^sub>l\<^sub>a\<^sub>x\<^sub>y_OclAny_defined' : 
 assumes isdef: "\<tau> \<Turnstile> (\<delta> (X))"
 shows "\<tau> \<Turnstile> (\<delta> ((X::OclAny) .oclIsKindOf(Galaxy)))"
-by(rule OclIsKindOf\<^sub>G\<^sub>a\<^sub>l\<^sub>a\<^sub>x\<^sub>y_OclAny_defined[OF isdef[THEN foundation20]])
+by(rule OclIsKindOf\<^sub>G\<^sub>a\<^sub>l\<^sub>a\<^sub>x\<^sub>y_OclAny_defined[OF isdef[THEN foundation20]]) 
 lemma OclIsKindOf\<^sub>G\<^sub>a\<^sub>l\<^sub>a\<^sub>x\<^sub>y_Galaxy_defined' : 
 assumes isdef: "\<tau> \<Turnstile> (\<delta> (X))"
 shows "\<tau> \<Turnstile> (\<delta> ((X::Galaxy) .oclIsKindOf(Galaxy)))"
-by(rule OclIsKindOf\<^sub>G\<^sub>a\<^sub>l\<^sub>a\<^sub>x\<^sub>y_Galaxy_defined[OF isdef[THEN foundation20]])
+by(rule OclIsKindOf\<^sub>G\<^sub>a\<^sub>l\<^sub>a\<^sub>x\<^sub>y_Galaxy_defined[OF isdef[THEN foundation20]]) 
 lemma OclIsKindOf\<^sub>G\<^sub>a\<^sub>l\<^sub>a\<^sub>x\<^sub>y_Planet_defined' : 
 assumes isdef: "\<tau> \<Turnstile> (\<delta> (X))"
 shows "\<tau> \<Turnstile> (\<delta> ((X::Planet) .oclIsKindOf(Galaxy)))"
-by(rule OclIsKindOf\<^sub>G\<^sub>a\<^sub>l\<^sub>a\<^sub>x\<^sub>y_Planet_defined[OF isdef[THEN foundation20]])
+by(rule OclIsKindOf\<^sub>G\<^sub>a\<^sub>l\<^sub>a\<^sub>x\<^sub>y_Planet_defined[OF isdef[THEN foundation20]]) 
 lemma OclIsKindOf\<^sub>G\<^sub>a\<^sub>l\<^sub>a\<^sub>x\<^sub>y_Person_defined' : 
 assumes isdef: "\<tau> \<Turnstile> (\<delta> (X))"
 shows "\<tau> \<Turnstile> (\<delta> ((X::Person) .oclIsKindOf(Galaxy)))"
-by(rule OclIsKindOf\<^sub>G\<^sub>a\<^sub>l\<^sub>a\<^sub>x\<^sub>y_Person_defined[OF isdef[THEN foundation20]])
+by(rule OclIsKindOf\<^sub>G\<^sub>a\<^sub>l\<^sub>a\<^sub>x\<^sub>y_Person_defined[OF isdef[THEN foundation20]]) 
 lemma OclIsKindOf\<^sub>O\<^sub>c\<^sub>l\<^sub>A\<^sub>n\<^sub>y_OclAny_defined' : 
 assumes isdef: "\<tau> \<Turnstile> (\<delta> (X))"
 shows "\<tau> \<Turnstile> (\<delta> ((X::OclAny) .oclIsKindOf(OclAny)))"
-by(rule OclIsKindOf\<^sub>O\<^sub>c\<^sub>l\<^sub>A\<^sub>n\<^sub>y_OclAny_defined[OF isdef[THEN foundation20]])
+by(rule OclIsKindOf\<^sub>O\<^sub>c\<^sub>l\<^sub>A\<^sub>n\<^sub>y_OclAny_defined[OF isdef[THEN foundation20]]) 
 lemma OclIsKindOf\<^sub>O\<^sub>c\<^sub>l\<^sub>A\<^sub>n\<^sub>y_Galaxy_defined' : 
 assumes isdef: "\<tau> \<Turnstile> (\<delta> (X))"
 shows "\<tau> \<Turnstile> (\<delta> ((X::Galaxy) .oclIsKindOf(OclAny)))"
-by(rule OclIsKindOf\<^sub>O\<^sub>c\<^sub>l\<^sub>A\<^sub>n\<^sub>y_Galaxy_defined[OF isdef[THEN foundation20]])
+by(rule OclIsKindOf\<^sub>O\<^sub>c\<^sub>l\<^sub>A\<^sub>n\<^sub>y_Galaxy_defined[OF isdef[THEN foundation20]]) 
 lemma OclIsKindOf\<^sub>O\<^sub>c\<^sub>l\<^sub>A\<^sub>n\<^sub>y_Planet_defined' : 
 assumes isdef: "\<tau> \<Turnstile> (\<delta> (X))"
 shows "\<tau> \<Turnstile> (\<delta> ((X::Planet) .oclIsKindOf(OclAny)))"
-by(rule OclIsKindOf\<^sub>O\<^sub>c\<^sub>l\<^sub>A\<^sub>n\<^sub>y_Planet_defined[OF isdef[THEN foundation20]])
+by(rule OclIsKindOf\<^sub>O\<^sub>c\<^sub>l\<^sub>A\<^sub>n\<^sub>y_Planet_defined[OF isdef[THEN foundation20]]) 
 lemma OclIsKindOf\<^sub>O\<^sub>c\<^sub>l\<^sub>A\<^sub>n\<^sub>y_Person_defined' : 
 assumes isdef: "\<tau> \<Turnstile> (\<delta> (X))"
 shows "\<tau> \<Turnstile> (\<delta> ((X::Person) .oclIsKindOf(OclAny)))"
-by(rule OclIsKindOf\<^sub>O\<^sub>c\<^sub>l\<^sub>A\<^sub>n\<^sub>y_Person_defined[OF isdef[THEN foundation20]])
+by(rule OclIsKindOf\<^sub>O\<^sub>c\<^sub>l\<^sub>A\<^sub>n\<^sub>y_Person_defined[OF isdef[THEN foundation20]]) 
 
 (* 78 ************************************ 528 + 1 *)
 subsection{* Up Down Casting *}
@@ -1952,22 +1952,22 @@ lemma actual_eq_static\<^sub>P\<^sub>e\<^sub>r\<^sub>s\<^sub>o\<^sub>n :
 assumes isdef: "\<tau> \<Turnstile> (\<delta> (X))"
 shows "\<tau> \<Turnstile> ((X::Person) .oclIsKindOf(Person))"
   apply(simp only: OclIsKindOf\<^sub>P\<^sub>e\<^sub>r\<^sub>s\<^sub>o\<^sub>n_Person OclValid_def, insert isdef)
-by(auto simp: foundation16 bot_option_def split: option.split type\<^sub>P\<^sub>e\<^sub>r\<^sub>s\<^sub>o\<^sub>n.split typeoid\<^sub>P\<^sub>e\<^sub>r\<^sub>s\<^sub>o\<^sub>n.split)
+by(auto simp: foundation16 bot_option_def split: option.split type\<^sub>P\<^sub>e\<^sub>r\<^sub>s\<^sub>o\<^sub>n.split typeoid\<^sub>P\<^sub>e\<^sub>r\<^sub>s\<^sub>o\<^sub>n.split) 
 lemma actual_eq_static\<^sub>P\<^sub>l\<^sub>a\<^sub>n\<^sub>e\<^sub>t : 
 assumes isdef: "\<tau> \<Turnstile> (\<delta> (X))"
 shows "\<tau> \<Turnstile> ((X::Planet) .oclIsKindOf(Planet))"
   apply(simp only: OclIsKindOf\<^sub>P\<^sub>l\<^sub>a\<^sub>n\<^sub>e\<^sub>t_Planet OclValid_def, insert isdef)
-by((subst cp_OclOr, auto simp: cp_OclOr[symmetric ] foundation16 bot_option_def OclIsKindOf\<^sub>P\<^sub>e\<^sub>r\<^sub>s\<^sub>o\<^sub>n_Planet OclIsTypeOf\<^sub>P\<^sub>e\<^sub>r\<^sub>s\<^sub>o\<^sub>n_Planet split: option.split type\<^sub>P\<^sub>l\<^sub>a\<^sub>n\<^sub>e\<^sub>t.split typeoid\<^sub>P\<^sub>l\<^sub>a\<^sub>n\<^sub>e\<^sub>t.split type\<^sub>P\<^sub>e\<^sub>r\<^sub>s\<^sub>o\<^sub>n.split typeoid\<^sub>P\<^sub>e\<^sub>r\<^sub>s\<^sub>o\<^sub>n.split)+)
+by((subst cp_OclOr, auto simp: cp_OclOr[symmetric ] foundation16 bot_option_def OclIsKindOf\<^sub>P\<^sub>e\<^sub>r\<^sub>s\<^sub>o\<^sub>n_Planet OclIsTypeOf\<^sub>P\<^sub>e\<^sub>r\<^sub>s\<^sub>o\<^sub>n_Planet split: option.split type\<^sub>P\<^sub>l\<^sub>a\<^sub>n\<^sub>e\<^sub>t.split typeoid\<^sub>P\<^sub>l\<^sub>a\<^sub>n\<^sub>e\<^sub>t.split type\<^sub>P\<^sub>e\<^sub>r\<^sub>s\<^sub>o\<^sub>n.split typeoid\<^sub>P\<^sub>e\<^sub>r\<^sub>s\<^sub>o\<^sub>n.split)+) 
 lemma actual_eq_static\<^sub>G\<^sub>a\<^sub>l\<^sub>a\<^sub>x\<^sub>y : 
 assumes isdef: "\<tau> \<Turnstile> (\<delta> (X))"
 shows "\<tau> \<Turnstile> ((X::Galaxy) .oclIsKindOf(Galaxy))"
   apply(simp only: OclIsKindOf\<^sub>G\<^sub>a\<^sub>l\<^sub>a\<^sub>x\<^sub>y_Galaxy OclValid_def, insert isdef)
-by((subst cp_OclOr, auto simp: cp_OclOr[symmetric ] foundation16 bot_option_def OclIsKindOf\<^sub>P\<^sub>l\<^sub>a\<^sub>n\<^sub>e\<^sub>t_Galaxy OclIsTypeOf\<^sub>P\<^sub>l\<^sub>a\<^sub>n\<^sub>e\<^sub>t_Galaxy OclIsKindOf\<^sub>P\<^sub>e\<^sub>r\<^sub>s\<^sub>o\<^sub>n_Galaxy OclIsTypeOf\<^sub>P\<^sub>e\<^sub>r\<^sub>s\<^sub>o\<^sub>n_Galaxy split: option.split type\<^sub>G\<^sub>a\<^sub>l\<^sub>a\<^sub>x\<^sub>y.split typeoid\<^sub>G\<^sub>a\<^sub>l\<^sub>a\<^sub>x\<^sub>y.split type\<^sub>P\<^sub>l\<^sub>a\<^sub>n\<^sub>e\<^sub>t.split typeoid\<^sub>P\<^sub>l\<^sub>a\<^sub>n\<^sub>e\<^sub>t.split type\<^sub>P\<^sub>e\<^sub>r\<^sub>s\<^sub>o\<^sub>n.split typeoid\<^sub>P\<^sub>e\<^sub>r\<^sub>s\<^sub>o\<^sub>n.split)+)
+by((subst cp_OclOr, auto simp: cp_OclOr[symmetric ] foundation16 bot_option_def OclIsKindOf\<^sub>P\<^sub>l\<^sub>a\<^sub>n\<^sub>e\<^sub>t_Galaxy OclIsTypeOf\<^sub>P\<^sub>l\<^sub>a\<^sub>n\<^sub>e\<^sub>t_Galaxy OclIsKindOf\<^sub>P\<^sub>e\<^sub>r\<^sub>s\<^sub>o\<^sub>n_Galaxy OclIsTypeOf\<^sub>P\<^sub>e\<^sub>r\<^sub>s\<^sub>o\<^sub>n_Galaxy split: option.split type\<^sub>G\<^sub>a\<^sub>l\<^sub>a\<^sub>x\<^sub>y.split typeoid\<^sub>G\<^sub>a\<^sub>l\<^sub>a\<^sub>x\<^sub>y.split type\<^sub>P\<^sub>l\<^sub>a\<^sub>n\<^sub>e\<^sub>t.split typeoid\<^sub>P\<^sub>l\<^sub>a\<^sub>n\<^sub>e\<^sub>t.split type\<^sub>P\<^sub>e\<^sub>r\<^sub>s\<^sub>o\<^sub>n.split typeoid\<^sub>P\<^sub>e\<^sub>r\<^sub>s\<^sub>o\<^sub>n.split)+) 
 lemma actual_eq_static\<^sub>O\<^sub>c\<^sub>l\<^sub>A\<^sub>n\<^sub>y : 
 assumes isdef: "\<tau> \<Turnstile> (\<delta> (X))"
 shows "\<tau> \<Turnstile> ((X::OclAny) .oclIsKindOf(OclAny))"
   apply(simp only: OclIsKindOf\<^sub>O\<^sub>c\<^sub>l\<^sub>A\<^sub>n\<^sub>y_OclAny OclValid_def, insert isdef)
-by((subst cp_OclOr, auto simp: cp_OclOr[symmetric ] foundation16 bot_option_def OclIsKindOf\<^sub>G\<^sub>a\<^sub>l\<^sub>a\<^sub>x\<^sub>y_OclAny OclIsTypeOf\<^sub>G\<^sub>a\<^sub>l\<^sub>a\<^sub>x\<^sub>y_OclAny OclIsKindOf\<^sub>P\<^sub>l\<^sub>a\<^sub>n\<^sub>e\<^sub>t_OclAny OclIsTypeOf\<^sub>P\<^sub>l\<^sub>a\<^sub>n\<^sub>e\<^sub>t_OclAny OclIsKindOf\<^sub>P\<^sub>e\<^sub>r\<^sub>s\<^sub>o\<^sub>n_OclAny OclIsTypeOf\<^sub>P\<^sub>e\<^sub>r\<^sub>s\<^sub>o\<^sub>n_OclAny split: option.split type\<^sub>O\<^sub>c\<^sub>l\<^sub>A\<^sub>n\<^sub>y.split typeoid\<^sub>O\<^sub>c\<^sub>l\<^sub>A\<^sub>n\<^sub>y.split type\<^sub>G\<^sub>a\<^sub>l\<^sub>a\<^sub>x\<^sub>y.split typeoid\<^sub>G\<^sub>a\<^sub>l\<^sub>a\<^sub>x\<^sub>y.split type\<^sub>P\<^sub>l\<^sub>a\<^sub>n\<^sub>e\<^sub>t.split typeoid\<^sub>P\<^sub>l\<^sub>a\<^sub>n\<^sub>e\<^sub>t.split type\<^sub>P\<^sub>e\<^sub>r\<^sub>s\<^sub>o\<^sub>n.split typeoid\<^sub>P\<^sub>e\<^sub>r\<^sub>s\<^sub>o\<^sub>n.split)+)
+by((subst cp_OclOr, auto simp: cp_OclOr[symmetric ] foundation16 bot_option_def OclIsKindOf\<^sub>G\<^sub>a\<^sub>l\<^sub>a\<^sub>x\<^sub>y_OclAny OclIsTypeOf\<^sub>G\<^sub>a\<^sub>l\<^sub>a\<^sub>x\<^sub>y_OclAny OclIsKindOf\<^sub>P\<^sub>l\<^sub>a\<^sub>n\<^sub>e\<^sub>t_OclAny OclIsTypeOf\<^sub>P\<^sub>l\<^sub>a\<^sub>n\<^sub>e\<^sub>t_OclAny OclIsKindOf\<^sub>P\<^sub>e\<^sub>r\<^sub>s\<^sub>o\<^sub>n_OclAny OclIsTypeOf\<^sub>P\<^sub>e\<^sub>r\<^sub>s\<^sub>o\<^sub>n_OclAny split: option.split type\<^sub>O\<^sub>c\<^sub>l\<^sub>A\<^sub>n\<^sub>y.split typeoid\<^sub>O\<^sub>c\<^sub>l\<^sub>A\<^sub>n\<^sub>y.split type\<^sub>G\<^sub>a\<^sub>l\<^sub>a\<^sub>x\<^sub>y.split typeoid\<^sub>G\<^sub>a\<^sub>l\<^sub>a\<^sub>x\<^sub>y.split type\<^sub>P\<^sub>l\<^sub>a\<^sub>n\<^sub>e\<^sub>t.split typeoid\<^sub>P\<^sub>l\<^sub>a\<^sub>n\<^sub>e\<^sub>t.split type\<^sub>P\<^sub>e\<^sub>r\<^sub>s\<^sub>o\<^sub>n.split typeoid\<^sub>P\<^sub>e\<^sub>r\<^sub>s\<^sub>o\<^sub>n.split)+) 
 
 (* 80 ************************************ 533 + 6 *)
 lemma actualKind\<^sub>P\<^sub>e\<^sub>r\<^sub>s\<^sub>o\<^sub>n_larger_staticKind\<^sub>P\<^sub>l\<^sub>a\<^sub>n\<^sub>e\<^sub>t : 
@@ -1976,42 +1976,42 @@ shows "\<tau> \<Turnstile> ((X::Person) .oclIsKindOf(Planet))"
   apply(simp only: OclIsKindOf\<^sub>P\<^sub>l\<^sub>a\<^sub>n\<^sub>e\<^sub>t_Person)
   apply(insert actual_eq_static\<^sub>P\<^sub>e\<^sub>r\<^sub>s\<^sub>o\<^sub>n[OF isdef] actualType\<^sub>P\<^sub>e\<^sub>r\<^sub>s\<^sub>o\<^sub>n_larger_staticType\<^sub>P\<^sub>l\<^sub>a\<^sub>n\<^sub>e\<^sub>t[OF isdef])
   apply(rule foundation11[THEN iffD2])
-by((simp add: OclNot_defargs foundation6 foundation14)+)
+by((simp add: OclNot_defargs foundation6 foundation14)+) 
 lemma actualKind\<^sub>P\<^sub>e\<^sub>r\<^sub>s\<^sub>o\<^sub>n_larger_staticKind\<^sub>G\<^sub>a\<^sub>l\<^sub>a\<^sub>x\<^sub>y : 
 assumes isdef: "\<tau> \<Turnstile> (\<delta> (X))"
 shows "\<tau> \<Turnstile> ((X::Person) .oclIsKindOf(Galaxy))"
   apply(simp only: OclIsKindOf\<^sub>G\<^sub>a\<^sub>l\<^sub>a\<^sub>x\<^sub>y_Person)
   apply(insert actualKind\<^sub>P\<^sub>e\<^sub>r\<^sub>s\<^sub>o\<^sub>n_larger_staticKind\<^sub>P\<^sub>l\<^sub>a\<^sub>n\<^sub>e\<^sub>t[OF isdef] actualType\<^sub>P\<^sub>e\<^sub>r\<^sub>s\<^sub>o\<^sub>n_larger_staticType\<^sub>G\<^sub>a\<^sub>l\<^sub>a\<^sub>x\<^sub>y[OF isdef])
   apply(rule foundation11[THEN iffD2])
-by((simp add: OclNot_defargs foundation6 foundation14)+)
+by((simp add: OclNot_defargs foundation6 foundation14)+) 
 lemma actualKind\<^sub>P\<^sub>e\<^sub>r\<^sub>s\<^sub>o\<^sub>n_larger_staticKind\<^sub>O\<^sub>c\<^sub>l\<^sub>A\<^sub>n\<^sub>y : 
 assumes isdef: "\<tau> \<Turnstile> (\<delta> (X))"
 shows "\<tau> \<Turnstile> ((X::Person) .oclIsKindOf(OclAny))"
   apply(simp only: OclIsKindOf\<^sub>O\<^sub>c\<^sub>l\<^sub>A\<^sub>n\<^sub>y_Person)
   apply(insert actualKind\<^sub>P\<^sub>e\<^sub>r\<^sub>s\<^sub>o\<^sub>n_larger_staticKind\<^sub>G\<^sub>a\<^sub>l\<^sub>a\<^sub>x\<^sub>y[OF isdef] actualType\<^sub>P\<^sub>e\<^sub>r\<^sub>s\<^sub>o\<^sub>n_larger_staticType\<^sub>O\<^sub>c\<^sub>l\<^sub>A\<^sub>n\<^sub>y[OF isdef])
   apply(rule foundation11[THEN iffD2])
-by((simp add: OclNot_defargs foundation6 foundation14)+)
+by((simp add: OclNot_defargs foundation6 foundation14)+) 
 lemma actualKind\<^sub>P\<^sub>l\<^sub>a\<^sub>n\<^sub>e\<^sub>t_larger_staticKind\<^sub>G\<^sub>a\<^sub>l\<^sub>a\<^sub>x\<^sub>y : 
 assumes isdef: "\<tau> \<Turnstile> (\<delta> (X))"
 shows "\<tau> \<Turnstile> ((X::Planet) .oclIsKindOf(Galaxy))"
   apply(simp only: OclIsKindOf\<^sub>G\<^sub>a\<^sub>l\<^sub>a\<^sub>x\<^sub>y_Planet)
   apply(insert actual_eq_static\<^sub>P\<^sub>l\<^sub>a\<^sub>n\<^sub>e\<^sub>t[OF isdef] actualType\<^sub>P\<^sub>l\<^sub>a\<^sub>n\<^sub>e\<^sub>t_larger_staticType\<^sub>G\<^sub>a\<^sub>l\<^sub>a\<^sub>x\<^sub>y[OF isdef])
   apply(rule foundation11[THEN iffD2])
-by((simp add: OclNot_defargs foundation6 foundation14)+)
+by((simp add: OclNot_defargs foundation6 foundation14)+) 
 lemma actualKind\<^sub>P\<^sub>l\<^sub>a\<^sub>n\<^sub>e\<^sub>t_larger_staticKind\<^sub>O\<^sub>c\<^sub>l\<^sub>A\<^sub>n\<^sub>y : 
 assumes isdef: "\<tau> \<Turnstile> (\<delta> (X))"
 shows "\<tau> \<Turnstile> ((X::Planet) .oclIsKindOf(OclAny))"
   apply(simp only: OclIsKindOf\<^sub>O\<^sub>c\<^sub>l\<^sub>A\<^sub>n\<^sub>y_Planet)
   apply(insert actualKind\<^sub>P\<^sub>l\<^sub>a\<^sub>n\<^sub>e\<^sub>t_larger_staticKind\<^sub>G\<^sub>a\<^sub>l\<^sub>a\<^sub>x\<^sub>y[OF isdef] actualType\<^sub>P\<^sub>l\<^sub>a\<^sub>n\<^sub>e\<^sub>t_larger_staticType\<^sub>O\<^sub>c\<^sub>l\<^sub>A\<^sub>n\<^sub>y[OF isdef])
   apply(rule foundation11[THEN iffD2])
-by((simp add: OclNot_defargs foundation6 foundation14)+)
+by((simp add: OclNot_defargs foundation6 foundation14)+) 
 lemma actualKind\<^sub>G\<^sub>a\<^sub>l\<^sub>a\<^sub>x\<^sub>y_larger_staticKind\<^sub>O\<^sub>c\<^sub>l\<^sub>A\<^sub>n\<^sub>y : 
 assumes isdef: "\<tau> \<Turnstile> (\<delta> (X))"
 shows "\<tau> \<Turnstile> ((X::Galaxy) .oclIsKindOf(OclAny))"
   apply(simp only: OclIsKindOf\<^sub>O\<^sub>c\<^sub>l\<^sub>A\<^sub>n\<^sub>y_Galaxy)
   apply(insert actual_eq_static\<^sub>G\<^sub>a\<^sub>l\<^sub>a\<^sub>x\<^sub>y[OF isdef] actualType\<^sub>G\<^sub>a\<^sub>l\<^sub>a\<^sub>x\<^sub>y_larger_staticType\<^sub>O\<^sub>c\<^sub>l\<^sub>A\<^sub>n\<^sub>y[OF isdef])
   apply(rule foundation11[THEN iffD2])
-by((simp add: OclNot_defargs foundation6 foundation14)+)
+by((simp add: OclNot_defargs foundation6 foundation14)+) 
 
 (* 81 ************************************ 539 + 6 *)
 lemma not_OclIsKindOf\<^sub>P\<^sub>e\<^sub>r\<^sub>s\<^sub>o\<^sub>n_then_Planet_OclIsTypeOf_others : 
@@ -2020,7 +2020,7 @@ assumes isdef: "\<tau> \<Turnstile> (\<delta> (X))"
 shows "\<tau> \<Turnstile> ((X::Planet) .oclIsTypeOf(Planet))"
   using actual_eq_static\<^sub>P\<^sub>l\<^sub>a\<^sub>n\<^sub>e\<^sub>t[OF isdef]
   apply(simp only: OclIsKindOf\<^sub>P\<^sub>l\<^sub>a\<^sub>n\<^sub>e\<^sub>t_Planet foundation11[OF OclIsTypeOf\<^sub>P\<^sub>l\<^sub>a\<^sub>n\<^sub>e\<^sub>t_Planet_defined'[OF isdef], OF OclIsKindOf\<^sub>P\<^sub>e\<^sub>r\<^sub>s\<^sub>o\<^sub>n_Planet_defined'[OF isdef]])
-by(simp add: iskin)
+by(simp add: iskin) 
 lemma not_OclIsKindOf\<^sub>P\<^sub>e\<^sub>r\<^sub>s\<^sub>o\<^sub>n_then_Galaxy_OclIsTypeOf_others : 
 assumes iskin: "\<not> \<tau> \<Turnstile> ((X::Galaxy) .oclIsKindOf(Person))"
 assumes isdef: "\<tau> \<Turnstile> (\<delta> (X))"
@@ -2029,7 +2029,7 @@ shows "\<tau> \<Turnstile> ((X::Galaxy) .oclIsTypeOf(Galaxy)) \<or> \<tau> \<Tur
   apply(simp only: OclIsKindOf\<^sub>G\<^sub>a\<^sub>l\<^sub>a\<^sub>x\<^sub>y_Galaxy foundation11[OF OclIsTypeOf\<^sub>G\<^sub>a\<^sub>l\<^sub>a\<^sub>x\<^sub>y_Galaxy_defined'[OF isdef], OF OclIsKindOf\<^sub>P\<^sub>l\<^sub>a\<^sub>n\<^sub>e\<^sub>t_Galaxy_defined'[OF isdef]])
   apply(erule disjE, simp, rule disjI2)
   apply(simp only: OclIsKindOf\<^sub>P\<^sub>l\<^sub>a\<^sub>n\<^sub>e\<^sub>t_Galaxy foundation11[OF OclIsTypeOf\<^sub>P\<^sub>l\<^sub>a\<^sub>n\<^sub>e\<^sub>t_Galaxy_defined'[OF isdef], OF OclIsKindOf\<^sub>P\<^sub>e\<^sub>r\<^sub>s\<^sub>o\<^sub>n_Galaxy_defined'[OF isdef]])
-by(simp add: iskin)
+by(simp add: iskin) 
 lemma not_OclIsKindOf\<^sub>P\<^sub>e\<^sub>r\<^sub>s\<^sub>o\<^sub>n_then_OclAny_OclIsTypeOf_others : 
 assumes iskin: "\<not> \<tau> \<Turnstile> ((X::OclAny) .oclIsKindOf(Person))"
 assumes isdef: "\<tau> \<Turnstile> (\<delta> (X))"
@@ -2040,14 +2040,14 @@ shows "\<tau> \<Turnstile> ((X::OclAny) .oclIsTypeOf(OclAny)) \<or> \<tau> \<Tur
   apply(simp only: OclIsKindOf\<^sub>G\<^sub>a\<^sub>l\<^sub>a\<^sub>x\<^sub>y_OclAny foundation11[OF OclIsTypeOf\<^sub>G\<^sub>a\<^sub>l\<^sub>a\<^sub>x\<^sub>y_OclAny_defined'[OF isdef], OF OclIsKindOf\<^sub>P\<^sub>l\<^sub>a\<^sub>n\<^sub>e\<^sub>t_OclAny_defined'[OF isdef]])
   apply(erule disjE, simp, rule disjI2)
   apply(simp only: OclIsKindOf\<^sub>P\<^sub>l\<^sub>a\<^sub>n\<^sub>e\<^sub>t_OclAny foundation11[OF OclIsTypeOf\<^sub>P\<^sub>l\<^sub>a\<^sub>n\<^sub>e\<^sub>t_OclAny_defined'[OF isdef], OF OclIsKindOf\<^sub>P\<^sub>e\<^sub>r\<^sub>s\<^sub>o\<^sub>n_OclAny_defined'[OF isdef]])
-by(simp add: iskin)
+by(simp add: iskin) 
 lemma not_OclIsKindOf\<^sub>P\<^sub>l\<^sub>a\<^sub>n\<^sub>e\<^sub>t_then_Galaxy_OclIsTypeOf_others : 
 assumes iskin: "\<not> \<tau> \<Turnstile> ((X::Galaxy) .oclIsKindOf(Planet))"
 assumes isdef: "\<tau> \<Turnstile> (\<delta> (X))"
 shows "\<tau> \<Turnstile> ((X::Galaxy) .oclIsTypeOf(Galaxy))"
   using actual_eq_static\<^sub>G\<^sub>a\<^sub>l\<^sub>a\<^sub>x\<^sub>y[OF isdef]
   apply(simp only: OclIsKindOf\<^sub>G\<^sub>a\<^sub>l\<^sub>a\<^sub>x\<^sub>y_Galaxy foundation11[OF OclIsTypeOf\<^sub>G\<^sub>a\<^sub>l\<^sub>a\<^sub>x\<^sub>y_Galaxy_defined'[OF isdef], OF OclIsKindOf\<^sub>P\<^sub>l\<^sub>a\<^sub>n\<^sub>e\<^sub>t_Galaxy_defined'[OF isdef]])
-by(simp add: iskin)
+by(simp add: iskin) 
 lemma not_OclIsKindOf\<^sub>P\<^sub>l\<^sub>a\<^sub>n\<^sub>e\<^sub>t_then_OclAny_OclIsTypeOf_others : 
 assumes iskin: "\<not> \<tau> \<Turnstile> ((X::OclAny) .oclIsKindOf(Planet))"
 assumes isdef: "\<tau> \<Turnstile> (\<delta> (X))"
@@ -2056,14 +2056,14 @@ shows "\<tau> \<Turnstile> ((X::OclAny) .oclIsTypeOf(OclAny)) \<or> \<tau> \<Tur
   apply(simp only: OclIsKindOf\<^sub>O\<^sub>c\<^sub>l\<^sub>A\<^sub>n\<^sub>y_OclAny foundation11[OF OclIsTypeOf\<^sub>O\<^sub>c\<^sub>l\<^sub>A\<^sub>n\<^sub>y_OclAny_defined'[OF isdef], OF OclIsKindOf\<^sub>G\<^sub>a\<^sub>l\<^sub>a\<^sub>x\<^sub>y_OclAny_defined'[OF isdef]])
   apply(erule disjE, simp, rule disjI2)
   apply(simp only: OclIsKindOf\<^sub>G\<^sub>a\<^sub>l\<^sub>a\<^sub>x\<^sub>y_OclAny foundation11[OF OclIsTypeOf\<^sub>G\<^sub>a\<^sub>l\<^sub>a\<^sub>x\<^sub>y_OclAny_defined'[OF isdef], OF OclIsKindOf\<^sub>P\<^sub>l\<^sub>a\<^sub>n\<^sub>e\<^sub>t_OclAny_defined'[OF isdef]])
-by(simp add: iskin)
+by(simp add: iskin) 
 lemma not_OclIsKindOf\<^sub>G\<^sub>a\<^sub>l\<^sub>a\<^sub>x\<^sub>y_then_OclAny_OclIsTypeOf_others : 
 assumes iskin: "\<not> \<tau> \<Turnstile> ((X::OclAny) .oclIsKindOf(Galaxy))"
 assumes isdef: "\<tau> \<Turnstile> (\<delta> (X))"
 shows "\<tau> \<Turnstile> ((X::OclAny) .oclIsTypeOf(OclAny))"
   using actual_eq_static\<^sub>O\<^sub>c\<^sub>l\<^sub>A\<^sub>n\<^sub>y[OF isdef]
   apply(simp only: OclIsKindOf\<^sub>O\<^sub>c\<^sub>l\<^sub>A\<^sub>n\<^sub>y_OclAny foundation11[OF OclIsTypeOf\<^sub>O\<^sub>c\<^sub>l\<^sub>A\<^sub>n\<^sub>y_OclAny_defined'[OF isdef], OF OclIsKindOf\<^sub>G\<^sub>a\<^sub>l\<^sub>a\<^sub>x\<^sub>y_OclAny_defined'[OF isdef]])
-by(simp add: iskin)
+by(simp add: iskin) 
 
 (* 82 ************************************ 545 + 10 *)
 lemma down_cast_kind\<^sub>P\<^sub>e\<^sub>r\<^sub>s\<^sub>o\<^sub>n_from_Planet_to_Person : 
@@ -2072,7 +2072,7 @@ assumes isdef: "\<tau> \<Turnstile> (\<delta> (X))"
 shows "\<tau> \<Turnstile> (X .oclAsType(Person)) \<triangleq> invalid"
   apply(insert not_OclIsKindOf\<^sub>P\<^sub>e\<^sub>r\<^sub>s\<^sub>o\<^sub>n_then_Planet_OclIsTypeOf_others[OF iskin, OF isdef])
   apply(rule down_cast_type\<^sub>P\<^sub>l\<^sub>a\<^sub>n\<^sub>e\<^sub>t_from_Planet_to_Person, simp only: , simp only: isdef)
-done
+done 
 lemma down_cast_kind\<^sub>P\<^sub>e\<^sub>r\<^sub>s\<^sub>o\<^sub>n_from_Galaxy_to_Person : 
 assumes iskin: "\<not> \<tau> \<Turnstile> ((X::Galaxy) .oclIsKindOf(Person))"
 assumes isdef: "\<tau> \<Turnstile> (\<delta> (X))"
@@ -2080,7 +2080,7 @@ shows "\<tau> \<Turnstile> (X .oclAsType(Person)) \<triangleq> invalid"
   apply(insert not_OclIsKindOf\<^sub>P\<^sub>e\<^sub>r\<^sub>s\<^sub>o\<^sub>n_then_Galaxy_OclIsTypeOf_others[OF iskin, OF isdef], elim disjE)
   apply(rule down_cast_type\<^sub>G\<^sub>a\<^sub>l\<^sub>a\<^sub>x\<^sub>y_from_Galaxy_to_Person, simp only: , simp only: isdef)
   apply(rule down_cast_type\<^sub>P\<^sub>l\<^sub>a\<^sub>n\<^sub>e\<^sub>t_from_Galaxy_to_Person, simp only: , simp only: isdef)
-done
+done 
 lemma down_cast_kind\<^sub>P\<^sub>e\<^sub>r\<^sub>s\<^sub>o\<^sub>n_from_OclAny_to_Person : 
 assumes iskin: "\<not> \<tau> \<Turnstile> ((X::OclAny) .oclIsKindOf(Person))"
 assumes isdef: "\<tau> \<Turnstile> (\<delta> (X))"
@@ -2089,14 +2089,14 @@ shows "\<tau> \<Turnstile> (X .oclAsType(Person)) \<triangleq> invalid"
   apply(rule down_cast_type\<^sub>O\<^sub>c\<^sub>l\<^sub>A\<^sub>n\<^sub>y_from_OclAny_to_Person, simp only: , simp only: isdef)
   apply(rule down_cast_type\<^sub>G\<^sub>a\<^sub>l\<^sub>a\<^sub>x\<^sub>y_from_OclAny_to_Person, simp only: , simp only: isdef)
   apply(rule down_cast_type\<^sub>P\<^sub>l\<^sub>a\<^sub>n\<^sub>e\<^sub>t_from_OclAny_to_Person, simp only: , simp only: isdef)
-done
+done 
 lemma down_cast_kind\<^sub>P\<^sub>l\<^sub>a\<^sub>n\<^sub>e\<^sub>t_from_Galaxy_to_Planet : 
 assumes iskin: "\<not> \<tau> \<Turnstile> ((X::Galaxy) .oclIsKindOf(Planet))"
 assumes isdef: "\<tau> \<Turnstile> (\<delta> (X))"
 shows "\<tau> \<Turnstile> (X .oclAsType(Planet)) \<triangleq> invalid"
   apply(insert not_OclIsKindOf\<^sub>P\<^sub>l\<^sub>a\<^sub>n\<^sub>e\<^sub>t_then_Galaxy_OclIsTypeOf_others[OF iskin, OF isdef])
   apply(rule down_cast_type\<^sub>G\<^sub>a\<^sub>l\<^sub>a\<^sub>x\<^sub>y_from_Galaxy_to_Planet, simp only: , simp only: isdef)
-done
+done 
 lemma down_cast_kind\<^sub>P\<^sub>l\<^sub>a\<^sub>n\<^sub>e\<^sub>t_from_OclAny_to_Planet : 
 assumes iskin: "\<not> \<tau> \<Turnstile> ((X::OclAny) .oclIsKindOf(Planet))"
 assumes isdef: "\<tau> \<Turnstile> (\<delta> (X))"
@@ -2104,21 +2104,21 @@ shows "\<tau> \<Turnstile> (X .oclAsType(Planet)) \<triangleq> invalid"
   apply(insert not_OclIsKindOf\<^sub>P\<^sub>l\<^sub>a\<^sub>n\<^sub>e\<^sub>t_then_OclAny_OclIsTypeOf_others[OF iskin, OF isdef], elim disjE)
   apply(rule down_cast_type\<^sub>O\<^sub>c\<^sub>l\<^sub>A\<^sub>n\<^sub>y_from_OclAny_to_Planet, simp only: , simp only: isdef)
   apply(rule down_cast_type\<^sub>G\<^sub>a\<^sub>l\<^sub>a\<^sub>x\<^sub>y_from_OclAny_to_Planet, simp only: , simp only: isdef)
-done
+done 
 lemma down_cast_kind\<^sub>G\<^sub>a\<^sub>l\<^sub>a\<^sub>x\<^sub>y_from_OclAny_to_Galaxy : 
 assumes iskin: "\<not> \<tau> \<Turnstile> ((X::OclAny) .oclIsKindOf(Galaxy))"
 assumes isdef: "\<tau> \<Turnstile> (\<delta> (X))"
 shows "\<tau> \<Turnstile> (X .oclAsType(Galaxy)) \<triangleq> invalid"
   apply(insert not_OclIsKindOf\<^sub>G\<^sub>a\<^sub>l\<^sub>a\<^sub>x\<^sub>y_then_OclAny_OclIsTypeOf_others[OF iskin, OF isdef])
   apply(rule down_cast_type\<^sub>O\<^sub>c\<^sub>l\<^sub>A\<^sub>n\<^sub>y_from_OclAny_to_Galaxy, simp only: , simp only: isdef)
-done
+done 
 lemma down_cast_kind\<^sub>P\<^sub>l\<^sub>a\<^sub>n\<^sub>e\<^sub>t_from_Galaxy_to_Person : 
 assumes iskin: "\<not> \<tau> \<Turnstile> ((X::Galaxy) .oclIsKindOf(Planet))"
 assumes isdef: "\<tau> \<Turnstile> (\<delta> (X))"
 shows "\<tau> \<Turnstile> (X .oclAsType(Person)) \<triangleq> invalid"
   apply(insert not_OclIsKindOf\<^sub>P\<^sub>l\<^sub>a\<^sub>n\<^sub>e\<^sub>t_then_Galaxy_OclIsTypeOf_others[OF iskin, OF isdef])
   apply(rule down_cast_type\<^sub>G\<^sub>a\<^sub>l\<^sub>a\<^sub>x\<^sub>y_from_Galaxy_to_Person, simp only: , simp only: isdef)
-done
+done 
 lemma down_cast_kind\<^sub>P\<^sub>l\<^sub>a\<^sub>n\<^sub>e\<^sub>t_from_OclAny_to_Person : 
 assumes iskin: "\<not> \<tau> \<Turnstile> ((X::OclAny) .oclIsKindOf(Planet))"
 assumes isdef: "\<tau> \<Turnstile> (\<delta> (X))"
@@ -2126,21 +2126,21 @@ shows "\<tau> \<Turnstile> (X .oclAsType(Person)) \<triangleq> invalid"
   apply(insert not_OclIsKindOf\<^sub>P\<^sub>l\<^sub>a\<^sub>n\<^sub>e\<^sub>t_then_OclAny_OclIsTypeOf_others[OF iskin, OF isdef], elim disjE)
   apply(rule down_cast_type\<^sub>O\<^sub>c\<^sub>l\<^sub>A\<^sub>n\<^sub>y_from_OclAny_to_Person, simp only: , simp only: isdef)
   apply(rule down_cast_type\<^sub>G\<^sub>a\<^sub>l\<^sub>a\<^sub>x\<^sub>y_from_OclAny_to_Person, simp only: , simp only: isdef)
-done
+done 
 lemma down_cast_kind\<^sub>G\<^sub>a\<^sub>l\<^sub>a\<^sub>x\<^sub>y_from_OclAny_to_Person : 
 assumes iskin: "\<not> \<tau> \<Turnstile> ((X::OclAny) .oclIsKindOf(Galaxy))"
 assumes isdef: "\<tau> \<Turnstile> (\<delta> (X))"
 shows "\<tau> \<Turnstile> (X .oclAsType(Person)) \<triangleq> invalid"
   apply(insert not_OclIsKindOf\<^sub>G\<^sub>a\<^sub>l\<^sub>a\<^sub>x\<^sub>y_then_OclAny_OclIsTypeOf_others[OF iskin, OF isdef])
   apply(rule down_cast_type\<^sub>O\<^sub>c\<^sub>l\<^sub>A\<^sub>n\<^sub>y_from_OclAny_to_Person, simp only: , simp only: isdef)
-done
+done 
 lemma down_cast_kind\<^sub>G\<^sub>a\<^sub>l\<^sub>a\<^sub>x\<^sub>y_from_OclAny_to_Planet : 
 assumes iskin: "\<not> \<tau> \<Turnstile> ((X::OclAny) .oclIsKindOf(Galaxy))"
 assumes isdef: "\<tau> \<Turnstile> (\<delta> (X))"
 shows "\<tau> \<Turnstile> (X .oclAsType(Planet)) \<triangleq> invalid"
   apply(insert not_OclIsKindOf\<^sub>G\<^sub>a\<^sub>l\<^sub>a\<^sub>x\<^sub>y_then_OclAny_OclIsTypeOf_others[OF iskin, OF isdef])
   apply(rule down_cast_type\<^sub>O\<^sub>c\<^sub>l\<^sub>A\<^sub>n\<^sub>y_from_OclAny_to_Planet, simp only: , simp only: isdef)
-done
+done 
 
 (* 83 ************************************ 555 + 1 *)
 section{* OclAllInstances *}
@@ -2164,45 +2164,368 @@ lemmas [simp,code_unfold] = Person_def
                             OclAny_def
 
 (* 87 ************************************ 562 + 1 *)
+lemma OclAsType\<^sub>O\<^sub>c\<^sub>l\<^sub>A\<^sub>n\<^sub>y_\<AA>_some : "(OclAsType\<^sub>O\<^sub>c\<^sub>l\<^sub>A\<^sub>n\<^sub>y_\<AA> (x)) \<noteq> None"
+by(simp add: OclAsType\<^sub>O\<^sub>c\<^sub>l\<^sub>A\<^sub>n\<^sub>y_\<AA>_def)
+
+(* 88 ************************************ 563 + 3 *)
+lemma OclAllInstances_generic\<^sub>O\<^sub>c\<^sub>l\<^sub>A\<^sub>n\<^sub>y_exec : 
+shows "(OclAllInstances_generic (pre_post) (OclAny)) = (\<lambda>\<tau>. (Abs_Set_0 (\<lfloor>\<lfloor>Some ` OclAny ` (ran ((heap ((pre_post (\<tau>))))))\<rfloor>\<rfloor>)))"
+  proof - let ?S1 = "(\<lambda>\<tau>. OclAny ` (ran ((heap ((pre_post (\<tau>)))))))" show ?thesis
+  proof - let ?S2 = "(\<lambda>\<tau>. ((?S1) (\<tau>)) - {None})" show ?thesis
+  proof - have B: "(\<And>\<tau>. ((?S2) (\<tau>)) \<subseteq> ((?S1) (\<tau>)))" by(auto simp: ) show ?thesis
+  proof - have C: "(\<And>\<tau>. ((?S1) (\<tau>)) \<subseteq> ((?S2) (\<tau>)))" by(auto simp: OclAsType\<^sub>O\<^sub>c\<^sub>l\<^sub>A\<^sub>n\<^sub>y_\<AA>_some) show ?thesis
+  apply(simp add: OclValid_def del: OclAllInstances_generic_def OclIsKindOf\<^sub>O\<^sub>c\<^sub>l\<^sub>A\<^sub>n\<^sub>y_OclAny)
+by(insert equalityI[OF B, OF C], simp) qed qed qed qed
+lemma OclAllInstances_at_post\<^sub>O\<^sub>c\<^sub>l\<^sub>A\<^sub>n\<^sub>y_exec : 
+shows "(OclAllInstances_at_post (OclAny)) = (\<lambda>\<tau>. (Abs_Set_0 (\<lfloor>\<lfloor>Some ` OclAny ` (ran ((heap ((snd (\<tau>))))))\<rfloor>\<rfloor>)))"
+  unfolding OclAllInstances_at_post_def
+by(rule OclAllInstances_generic\<^sub>O\<^sub>c\<^sub>l\<^sub>A\<^sub>n\<^sub>y_exec) 
+lemma OclAllInstances_at_pre\<^sub>O\<^sub>c\<^sub>l\<^sub>A\<^sub>n\<^sub>y_exec : 
+shows "(OclAllInstances_at_pre (OclAny)) = (\<lambda>\<tau>. (Abs_Set_0 (\<lfloor>\<lfloor>Some ` OclAny ` (ran ((heap ((fst (\<tau>))))))\<rfloor>\<rfloor>)))"
+  unfolding OclAllInstances_at_pre_def
+by(rule OclAllInstances_generic\<^sub>O\<^sub>c\<^sub>l\<^sub>A\<^sub>n\<^sub>y_exec) 
+
+(* 89 ************************************ 566 + 1 *)
 subsection{* OclIsTypeOf *}
 
-(* 88 ************************************ 563 + 1 *)
+(* 90 ************************************ 567 + 2 *)
+lemma ex_ssubst : "(\<forall>x \<in> B. (s (x)) = (t (x))) \<Longrightarrow> (\<exists>x \<in> B. (P ((s (x))))) = (\<exists>x \<in> B. (P ((t (x)))))"
+by(simp)
+lemma ex_def : "x \<in> \<lceil>\<lceil>\<lfloor>\<lfloor>Some ` (X - {None})\<rfloor>\<rfloor>\<rceil>\<rceil> \<Longrightarrow> (\<exists>y. x = \<lfloor>\<lfloor>y\<rfloor>\<rfloor>)"
+by(auto simp: )
+
+(* 91 ************************************ 569 + 21 *)
+lemma Person_OclAllInstances_generic_OclIsTypeOf\<^sub>P\<^sub>e\<^sub>r\<^sub>s\<^sub>o\<^sub>n : "\<tau> \<Turnstile> (OclForall ((OclAllInstances_generic (pre_post) (Person))) (OclIsTypeOf\<^sub>P\<^sub>e\<^sub>r\<^sub>s\<^sub>o\<^sub>n))"
+  apply(simp add: OclValid_def del: OclAllInstances_generic_def)
+  apply(simp only: OclForall_def refl if_True OclAllInstances_generic_defined[simplified OclValid_def])
+  apply(simp only: OclAllInstances_generic_def)
+  apply(subst (1 2 3) Abs_Set_0_inverse, simp add: bot_option_def)
+  apply(subst (1 2 3) ex_ssubst[where s = "(\<lambda>x. (((\<lambda>_. x) .oclIsTypeOf(Person)) (\<tau>)))" and t = "(\<lambda>_. (true (\<tau>)))"])
+  apply(intro ballI actual_eq_static\<^sub>P\<^sub>e\<^sub>r\<^sub>s\<^sub>o\<^sub>n[simplified OclValid_def, simplified OclIsKindOf\<^sub>P\<^sub>e\<^sub>r\<^sub>s\<^sub>o\<^sub>n_Person])
+  apply(drule ex_def, erule exE, simp)
+by(simp)
+lemma Person_OclAllInstances_at_post_OclIsTypeOf\<^sub>P\<^sub>e\<^sub>r\<^sub>s\<^sub>o\<^sub>n : 
+shows "\<tau> \<Turnstile> (OclForall ((OclAllInstances_at_post (Person))) (OclIsTypeOf\<^sub>P\<^sub>e\<^sub>r\<^sub>s\<^sub>o\<^sub>n))"
+  unfolding OclAllInstances_at_post_def
+by(rule Person_OclAllInstances_generic_OclIsTypeOf\<^sub>P\<^sub>e\<^sub>r\<^sub>s\<^sub>o\<^sub>n) 
+lemma Person_OclAllInstances_at_pre_OclIsTypeOf\<^sub>P\<^sub>e\<^sub>r\<^sub>s\<^sub>o\<^sub>n : 
+shows "\<tau> \<Turnstile> (OclForall ((OclAllInstances_at_pre (Person))) (OclIsTypeOf\<^sub>P\<^sub>e\<^sub>r\<^sub>s\<^sub>o\<^sub>n))"
+  unfolding OclAllInstances_at_pre_def
+by(rule Person_OclAllInstances_generic_OclIsTypeOf\<^sub>P\<^sub>e\<^sub>r\<^sub>s\<^sub>o\<^sub>n) 
+lemma Planet_OclAllInstances_generic_OclIsTypeOf\<^sub>P\<^sub>l\<^sub>a\<^sub>n\<^sub>e\<^sub>t1 : 
+assumes [simp]: "(\<And>x. (pre_post ((x , x))) = x)"
+shows "(\<exists>\<tau>. \<tau> \<Turnstile> (OclForall ((OclAllInstances_generic (pre_post) (Planet))) (OclIsTypeOf\<^sub>P\<^sub>l\<^sub>a\<^sub>n\<^sub>e\<^sub>t)))"
+  apply(rule exI[where x = "\<tau>\<^sub>0"], simp add: \<tau>\<^sub>0_def OclValid_def del: OclAllInstances_generic_def)
+  apply(simp only: OclForall_def refl if_True OclAllInstances_generic_defined[simplified OclValid_def])
+  apply(simp only: OclAllInstances_generic_def)
+  apply(subst (1 2 3) Abs_Set_0_inverse, simp add: bot_option_def)
+by(simp) 
+lemma Planet_OclAllInstances_at_post_OclIsTypeOf\<^sub>P\<^sub>l\<^sub>a\<^sub>n\<^sub>e\<^sub>t1 : 
+shows "(\<exists>\<tau>. \<tau> \<Turnstile> (OclForall ((OclAllInstances_at_post (Planet))) (OclIsTypeOf\<^sub>P\<^sub>l\<^sub>a\<^sub>n\<^sub>e\<^sub>t)))"
+  unfolding OclAllInstances_at_post_def
+by(rule Planet_OclAllInstances_generic_OclIsTypeOf\<^sub>P\<^sub>l\<^sub>a\<^sub>n\<^sub>e\<^sub>t1, simp) 
+lemma Planet_OclAllInstances_at_pre_OclIsTypeOf\<^sub>P\<^sub>l\<^sub>a\<^sub>n\<^sub>e\<^sub>t1 : 
+shows "(\<exists>\<tau>. \<tau> \<Turnstile> (OclForall ((OclAllInstances_at_pre (Planet))) (OclIsTypeOf\<^sub>P\<^sub>l\<^sub>a\<^sub>n\<^sub>e\<^sub>t)))"
+  unfolding OclAllInstances_at_pre_def
+by(rule Planet_OclAllInstances_generic_OclIsTypeOf\<^sub>P\<^sub>l\<^sub>a\<^sub>n\<^sub>e\<^sub>t1, simp) 
+lemma Planet_OclAllInstances_generic_OclIsTypeOf\<^sub>P\<^sub>l\<^sub>a\<^sub>n\<^sub>e\<^sub>t2 : 
+assumes [simp]: "(\<And>x. (pre_post ((x , x))) = x)"
+shows "(\<exists>\<tau>. \<tau> \<Turnstile> (not ((OclForall ((OclAllInstances_generic (pre_post) (Planet))) (OclIsTypeOf\<^sub>P\<^sub>l\<^sub>a\<^sub>n\<^sub>e\<^sub>t)))))"
+  proof - fix oid a show ?thesis
+  proof - let ?t0 = "(state.make ((Map.empty (oid \<mapsto> (in\<^sub>P\<^sub>l\<^sub>a\<^sub>n\<^sub>e\<^sub>t ((mkoid\<^sub>P\<^sub>l\<^sub>a\<^sub>n\<^sub>e\<^sub>t ((mk\<^sub>P\<^sub>l\<^sub>a\<^sub>n\<^sub>e\<^sub>t_\<^sub>P\<^sub>e\<^sub>r\<^sub>s\<^sub>o\<^sub>n (a))) (None))))))) (Map.empty) (Map.empty))" show ?thesis
+  apply(rule exI[where x = "(?t0 , ?t0)"], simp add: OclValid_def del: OclAllInstances_generic_def)
+  apply(simp only: OclForall_def refl if_True OclAllInstances_generic_defined[simplified OclValid_def])
+  apply(simp only: OclAllInstances_generic_def OclAsType\<^sub>P\<^sub>l\<^sub>a\<^sub>n\<^sub>e\<^sub>t_\<AA>_def)
+  apply(subst (1 2 3) Abs_Set_0_inverse, simp add: bot_option_def)
+by(simp add: state.make_def OclNot_def) qed qed
+lemma Planet_OclAllInstances_at_post_OclIsTypeOf\<^sub>P\<^sub>l\<^sub>a\<^sub>n\<^sub>e\<^sub>t2 : 
+shows "(\<exists>\<tau>. \<tau> \<Turnstile> (not ((OclForall ((OclAllInstances_at_post (Planet))) (OclIsTypeOf\<^sub>P\<^sub>l\<^sub>a\<^sub>n\<^sub>e\<^sub>t)))))"
+  unfolding OclAllInstances_at_post_def
+by(rule Planet_OclAllInstances_generic_OclIsTypeOf\<^sub>P\<^sub>l\<^sub>a\<^sub>n\<^sub>e\<^sub>t2, simp) 
+lemma Planet_OclAllInstances_at_pre_OclIsTypeOf\<^sub>P\<^sub>l\<^sub>a\<^sub>n\<^sub>e\<^sub>t2 : 
+shows "(\<exists>\<tau>. \<tau> \<Turnstile> (not ((OclForall ((OclAllInstances_at_pre (Planet))) (OclIsTypeOf\<^sub>P\<^sub>l\<^sub>a\<^sub>n\<^sub>e\<^sub>t)))))"
+  unfolding OclAllInstances_at_pre_def
+by(rule Planet_OclAllInstances_generic_OclIsTypeOf\<^sub>P\<^sub>l\<^sub>a\<^sub>n\<^sub>e\<^sub>t2, simp) 
+lemma Galaxy_OclAllInstances_generic_OclIsTypeOf\<^sub>G\<^sub>a\<^sub>l\<^sub>a\<^sub>x\<^sub>y1 : 
+assumes [simp]: "(\<And>x. (pre_post ((x , x))) = x)"
+shows "(\<exists>\<tau>. \<tau> \<Turnstile> (OclForall ((OclAllInstances_generic (pre_post) (Galaxy))) (OclIsTypeOf\<^sub>G\<^sub>a\<^sub>l\<^sub>a\<^sub>x\<^sub>y)))"
+  apply(rule exI[where x = "\<tau>\<^sub>0"], simp add: \<tau>\<^sub>0_def OclValid_def del: OclAllInstances_generic_def)
+  apply(simp only: OclForall_def refl if_True OclAllInstances_generic_defined[simplified OclValid_def])
+  apply(simp only: OclAllInstances_generic_def)
+  apply(subst (1 2 3) Abs_Set_0_inverse, simp add: bot_option_def)
+by(simp) 
+lemma Galaxy_OclAllInstances_at_post_OclIsTypeOf\<^sub>G\<^sub>a\<^sub>l\<^sub>a\<^sub>x\<^sub>y1 : 
+shows "(\<exists>\<tau>. \<tau> \<Turnstile> (OclForall ((OclAllInstances_at_post (Galaxy))) (OclIsTypeOf\<^sub>G\<^sub>a\<^sub>l\<^sub>a\<^sub>x\<^sub>y)))"
+  unfolding OclAllInstances_at_post_def
+by(rule Galaxy_OclAllInstances_generic_OclIsTypeOf\<^sub>G\<^sub>a\<^sub>l\<^sub>a\<^sub>x\<^sub>y1, simp) 
+lemma Galaxy_OclAllInstances_at_pre_OclIsTypeOf\<^sub>G\<^sub>a\<^sub>l\<^sub>a\<^sub>x\<^sub>y1 : 
+shows "(\<exists>\<tau>. \<tau> \<Turnstile> (OclForall ((OclAllInstances_at_pre (Galaxy))) (OclIsTypeOf\<^sub>G\<^sub>a\<^sub>l\<^sub>a\<^sub>x\<^sub>y)))"
+  unfolding OclAllInstances_at_pre_def
+by(rule Galaxy_OclAllInstances_generic_OclIsTypeOf\<^sub>G\<^sub>a\<^sub>l\<^sub>a\<^sub>x\<^sub>y1, simp) 
+lemma Galaxy_OclAllInstances_generic_OclIsTypeOf\<^sub>G\<^sub>a\<^sub>l\<^sub>a\<^sub>x\<^sub>y2 : 
+assumes [simp]: "(\<And>x. (pre_post ((x , x))) = x)"
+shows "(\<exists>\<tau>. \<tau> \<Turnstile> (not ((OclForall ((OclAllInstances_generic (pre_post) (Galaxy))) (OclIsTypeOf\<^sub>G\<^sub>a\<^sub>l\<^sub>a\<^sub>x\<^sub>y)))))"
+  proof - fix oid a show ?thesis
+  proof - let ?t0 = "(state.make ((Map.empty (oid \<mapsto> (in\<^sub>G\<^sub>a\<^sub>l\<^sub>a\<^sub>x\<^sub>y ((mkoid\<^sub>G\<^sub>a\<^sub>l\<^sub>a\<^sub>x\<^sub>y ((mk\<^sub>G\<^sub>a\<^sub>l\<^sub>a\<^sub>x\<^sub>y_\<^sub>P\<^sub>l\<^sub>a\<^sub>n\<^sub>e\<^sub>t (a))) (None) (None))))))) (Map.empty) (Map.empty))" show ?thesis
+  apply(rule exI[where x = "(?t0 , ?t0)"], simp add: OclValid_def del: OclAllInstances_generic_def)
+  apply(simp only: OclForall_def refl if_True OclAllInstances_generic_defined[simplified OclValid_def])
+  apply(simp only: OclAllInstances_generic_def OclAsType\<^sub>G\<^sub>a\<^sub>l\<^sub>a\<^sub>x\<^sub>y_\<AA>_def)
+  apply(subst (1 2 3) Abs_Set_0_inverse, simp add: bot_option_def)
+by(simp add: state.make_def OclNot_def) qed qed
+lemma Galaxy_OclAllInstances_at_post_OclIsTypeOf\<^sub>G\<^sub>a\<^sub>l\<^sub>a\<^sub>x\<^sub>y2 : 
+shows "(\<exists>\<tau>. \<tau> \<Turnstile> (not ((OclForall ((OclAllInstances_at_post (Galaxy))) (OclIsTypeOf\<^sub>G\<^sub>a\<^sub>l\<^sub>a\<^sub>x\<^sub>y)))))"
+  unfolding OclAllInstances_at_post_def
+by(rule Galaxy_OclAllInstances_generic_OclIsTypeOf\<^sub>G\<^sub>a\<^sub>l\<^sub>a\<^sub>x\<^sub>y2, simp) 
+lemma Galaxy_OclAllInstances_at_pre_OclIsTypeOf\<^sub>G\<^sub>a\<^sub>l\<^sub>a\<^sub>x\<^sub>y2 : 
+shows "(\<exists>\<tau>. \<tau> \<Turnstile> (not ((OclForall ((OclAllInstances_at_pre (Galaxy))) (OclIsTypeOf\<^sub>G\<^sub>a\<^sub>l\<^sub>a\<^sub>x\<^sub>y)))))"
+  unfolding OclAllInstances_at_pre_def
+by(rule Galaxy_OclAllInstances_generic_OclIsTypeOf\<^sub>G\<^sub>a\<^sub>l\<^sub>a\<^sub>x\<^sub>y2, simp) 
+lemma OclAny_OclAllInstances_generic_OclIsTypeOf\<^sub>O\<^sub>c\<^sub>l\<^sub>A\<^sub>n\<^sub>y1 : 
+assumes [simp]: "(\<And>x. (pre_post ((x , x))) = x)"
+shows "(\<exists>\<tau>. \<tau> \<Turnstile> (OclForall ((OclAllInstances_generic (pre_post) (OclAny))) (OclIsTypeOf\<^sub>O\<^sub>c\<^sub>l\<^sub>A\<^sub>n\<^sub>y)))"
+  apply(rule exI[where x = "\<tau>\<^sub>0"], simp add: \<tau>\<^sub>0_def OclValid_def del: OclAllInstances_generic_def)
+  apply(simp only: OclForall_def refl if_True OclAllInstances_generic_defined[simplified OclValid_def])
+  apply(simp only: OclAllInstances_generic_def)
+  apply(subst (1 2 3) Abs_Set_0_inverse, simp add: bot_option_def)
+by(simp) 
+lemma OclAny_OclAllInstances_at_post_OclIsTypeOf\<^sub>O\<^sub>c\<^sub>l\<^sub>A\<^sub>n\<^sub>y1 : 
+shows "(\<exists>\<tau>. \<tau> \<Turnstile> (OclForall ((OclAllInstances_at_post (OclAny))) (OclIsTypeOf\<^sub>O\<^sub>c\<^sub>l\<^sub>A\<^sub>n\<^sub>y)))"
+  unfolding OclAllInstances_at_post_def
+by(rule OclAny_OclAllInstances_generic_OclIsTypeOf\<^sub>O\<^sub>c\<^sub>l\<^sub>A\<^sub>n\<^sub>y1, simp) 
+lemma OclAny_OclAllInstances_at_pre_OclIsTypeOf\<^sub>O\<^sub>c\<^sub>l\<^sub>A\<^sub>n\<^sub>y1 : 
+shows "(\<exists>\<tau>. \<tau> \<Turnstile> (OclForall ((OclAllInstances_at_pre (OclAny))) (OclIsTypeOf\<^sub>O\<^sub>c\<^sub>l\<^sub>A\<^sub>n\<^sub>y)))"
+  unfolding OclAllInstances_at_pre_def
+by(rule OclAny_OclAllInstances_generic_OclIsTypeOf\<^sub>O\<^sub>c\<^sub>l\<^sub>A\<^sub>n\<^sub>y1, simp) 
+lemma OclAny_OclAllInstances_generic_OclIsTypeOf\<^sub>O\<^sub>c\<^sub>l\<^sub>A\<^sub>n\<^sub>y2 : 
+assumes [simp]: "(\<And>x. (pre_post ((x , x))) = x)"
+shows "(\<exists>\<tau>. \<tau> \<Turnstile> (not ((OclForall ((OclAllInstances_generic (pre_post) (OclAny))) (OclIsTypeOf\<^sub>O\<^sub>c\<^sub>l\<^sub>A\<^sub>n\<^sub>y)))))"
+  proof - fix oid a show ?thesis
+  proof - let ?t0 = "(state.make ((Map.empty (oid \<mapsto> (in\<^sub>O\<^sub>c\<^sub>l\<^sub>A\<^sub>n\<^sub>y ((mkoid\<^sub>O\<^sub>c\<^sub>l\<^sub>A\<^sub>n\<^sub>y ((mk\<^sub>O\<^sub>c\<^sub>l\<^sub>A\<^sub>n\<^sub>y_\<^sub>G\<^sub>a\<^sub>l\<^sub>a\<^sub>x\<^sub>y (a))))))))) (Map.empty) (Map.empty))" show ?thesis
+  apply(rule exI[where x = "(?t0 , ?t0)"], simp add: OclValid_def del: OclAllInstances_generic_def)
+  apply(simp only: OclForall_def refl if_True OclAllInstances_generic_defined[simplified OclValid_def])
+  apply(simp only: OclAllInstances_generic_def OclAsType\<^sub>O\<^sub>c\<^sub>l\<^sub>A\<^sub>n\<^sub>y_\<AA>_def)
+  apply(subst (1 2 3) Abs_Set_0_inverse, simp add: bot_option_def)
+by(simp add: state.make_def OclNot_def) qed qed
+lemma OclAny_OclAllInstances_at_post_OclIsTypeOf\<^sub>O\<^sub>c\<^sub>l\<^sub>A\<^sub>n\<^sub>y2 : 
+shows "(\<exists>\<tau>. \<tau> \<Turnstile> (not ((OclForall ((OclAllInstances_at_post (OclAny))) (OclIsTypeOf\<^sub>O\<^sub>c\<^sub>l\<^sub>A\<^sub>n\<^sub>y)))))"
+  unfolding OclAllInstances_at_post_def
+by(rule OclAny_OclAllInstances_generic_OclIsTypeOf\<^sub>O\<^sub>c\<^sub>l\<^sub>A\<^sub>n\<^sub>y2, simp) 
+lemma OclAny_OclAllInstances_at_pre_OclIsTypeOf\<^sub>O\<^sub>c\<^sub>l\<^sub>A\<^sub>n\<^sub>y2 : 
+shows "(\<exists>\<tau>. \<tau> \<Turnstile> (not ((OclForall ((OclAllInstances_at_pre (OclAny))) (OclIsTypeOf\<^sub>O\<^sub>c\<^sub>l\<^sub>A\<^sub>n\<^sub>y)))))"
+  unfolding OclAllInstances_at_pre_def
+by(rule OclAny_OclAllInstances_generic_OclIsTypeOf\<^sub>O\<^sub>c\<^sub>l\<^sub>A\<^sub>n\<^sub>y2, simp) 
+
+(* 92 ************************************ 590 + 1 *)
 subsection{* OclIsKindOf *}
 
-(* 89 ************************************ 564 + 1 *)
+(* 93 ************************************ 591 + 12 *)
+lemma Person_OclAllInstances_generic_OclIsKindOf\<^sub>P\<^sub>e\<^sub>r\<^sub>s\<^sub>o\<^sub>n : "\<tau> \<Turnstile> (OclForall ((OclAllInstances_generic (pre_post) (Person))) (OclIsKindOf\<^sub>P\<^sub>e\<^sub>r\<^sub>s\<^sub>o\<^sub>n))"
+  apply(simp add: OclValid_def del: OclAllInstances_generic_def OclIsKindOf\<^sub>P\<^sub>e\<^sub>r\<^sub>s\<^sub>o\<^sub>n_Person)
+  apply(simp only: OclForall_def refl if_True OclAllInstances_generic_defined[simplified OclValid_def])
+  apply(simp only: OclAllInstances_generic_def)
+  apply(subst (1 2 3) Abs_Set_0_inverse, simp add: bot_option_def)
+  apply(subst (1 2 3) ex_ssubst[where s = "(\<lambda>x. (((\<lambda>_. x) .oclIsKindOf(Person)) (\<tau>)))" and t = "(\<lambda>_. (true (\<tau>)))"])
+  apply(intro ballI actual_eq_static\<^sub>P\<^sub>e\<^sub>r\<^sub>s\<^sub>o\<^sub>n[simplified OclValid_def])
+  apply(drule ex_def, erule exE, simp)
+by(simp)
+lemma Person_OclAllInstances_at_post_OclIsKindOf\<^sub>P\<^sub>e\<^sub>r\<^sub>s\<^sub>o\<^sub>n : 
+shows "\<tau> \<Turnstile> (OclForall ((OclAllInstances_at_post (Person))) (OclIsKindOf\<^sub>P\<^sub>e\<^sub>r\<^sub>s\<^sub>o\<^sub>n))"
+  unfolding OclAllInstances_at_post_def
+by(rule Person_OclAllInstances_generic_OclIsKindOf\<^sub>P\<^sub>e\<^sub>r\<^sub>s\<^sub>o\<^sub>n) 
+lemma Person_OclAllInstances_at_pre_OclIsKindOf\<^sub>P\<^sub>e\<^sub>r\<^sub>s\<^sub>o\<^sub>n : 
+shows "\<tau> \<Turnstile> (OclForall ((OclAllInstances_at_pre (Person))) (OclIsKindOf\<^sub>P\<^sub>e\<^sub>r\<^sub>s\<^sub>o\<^sub>n))"
+  unfolding OclAllInstances_at_pre_def
+by(rule Person_OclAllInstances_generic_OclIsKindOf\<^sub>P\<^sub>e\<^sub>r\<^sub>s\<^sub>o\<^sub>n) 
+lemma Planet_OclAllInstances_generic_OclIsKindOf\<^sub>P\<^sub>l\<^sub>a\<^sub>n\<^sub>e\<^sub>t : "\<tau> \<Turnstile> (OclForall ((OclAllInstances_generic (pre_post) (Planet))) (OclIsKindOf\<^sub>P\<^sub>l\<^sub>a\<^sub>n\<^sub>e\<^sub>t))"
+  apply(simp add: OclValid_def del: OclAllInstances_generic_def OclIsKindOf\<^sub>P\<^sub>l\<^sub>a\<^sub>n\<^sub>e\<^sub>t_Planet)
+  apply(simp only: OclForall_def refl if_True OclAllInstances_generic_defined[simplified OclValid_def])
+  apply(simp only: OclAllInstances_generic_def)
+  apply(subst (1 2 3) Abs_Set_0_inverse, simp add: bot_option_def)
+  apply(subst (1 2 3) ex_ssubst[where s = "(\<lambda>x. (((\<lambda>_. x) .oclIsKindOf(Planet)) (\<tau>)))" and t = "(\<lambda>_. (true (\<tau>)))"])
+  apply(intro ballI actual_eq_static\<^sub>P\<^sub>l\<^sub>a\<^sub>n\<^sub>e\<^sub>t[simplified OclValid_def])
+  apply(drule ex_def, erule exE, simp)
+by(simp)
+lemma Planet_OclAllInstances_at_post_OclIsKindOf\<^sub>P\<^sub>l\<^sub>a\<^sub>n\<^sub>e\<^sub>t : 
+shows "\<tau> \<Turnstile> (OclForall ((OclAllInstances_at_post (Planet))) (OclIsKindOf\<^sub>P\<^sub>l\<^sub>a\<^sub>n\<^sub>e\<^sub>t))"
+  unfolding OclAllInstances_at_post_def
+by(rule Planet_OclAllInstances_generic_OclIsKindOf\<^sub>P\<^sub>l\<^sub>a\<^sub>n\<^sub>e\<^sub>t) 
+lemma Planet_OclAllInstances_at_pre_OclIsKindOf\<^sub>P\<^sub>l\<^sub>a\<^sub>n\<^sub>e\<^sub>t : 
+shows "\<tau> \<Turnstile> (OclForall ((OclAllInstances_at_pre (Planet))) (OclIsKindOf\<^sub>P\<^sub>l\<^sub>a\<^sub>n\<^sub>e\<^sub>t))"
+  unfolding OclAllInstances_at_pre_def
+by(rule Planet_OclAllInstances_generic_OclIsKindOf\<^sub>P\<^sub>l\<^sub>a\<^sub>n\<^sub>e\<^sub>t) 
+lemma Galaxy_OclAllInstances_generic_OclIsKindOf\<^sub>G\<^sub>a\<^sub>l\<^sub>a\<^sub>x\<^sub>y : "\<tau> \<Turnstile> (OclForall ((OclAllInstances_generic (pre_post) (Galaxy))) (OclIsKindOf\<^sub>G\<^sub>a\<^sub>l\<^sub>a\<^sub>x\<^sub>y))"
+  apply(simp add: OclValid_def del: OclAllInstances_generic_def OclIsKindOf\<^sub>G\<^sub>a\<^sub>l\<^sub>a\<^sub>x\<^sub>y_Galaxy)
+  apply(simp only: OclForall_def refl if_True OclAllInstances_generic_defined[simplified OclValid_def])
+  apply(simp only: OclAllInstances_generic_def)
+  apply(subst (1 2 3) Abs_Set_0_inverse, simp add: bot_option_def)
+  apply(subst (1 2 3) ex_ssubst[where s = "(\<lambda>x. (((\<lambda>_. x) .oclIsKindOf(Galaxy)) (\<tau>)))" and t = "(\<lambda>_. (true (\<tau>)))"])
+  apply(intro ballI actual_eq_static\<^sub>G\<^sub>a\<^sub>l\<^sub>a\<^sub>x\<^sub>y[simplified OclValid_def])
+  apply(drule ex_def, erule exE, simp)
+by(simp)
+lemma Galaxy_OclAllInstances_at_post_OclIsKindOf\<^sub>G\<^sub>a\<^sub>l\<^sub>a\<^sub>x\<^sub>y : 
+shows "\<tau> \<Turnstile> (OclForall ((OclAllInstances_at_post (Galaxy))) (OclIsKindOf\<^sub>G\<^sub>a\<^sub>l\<^sub>a\<^sub>x\<^sub>y))"
+  unfolding OclAllInstances_at_post_def
+by(rule Galaxy_OclAllInstances_generic_OclIsKindOf\<^sub>G\<^sub>a\<^sub>l\<^sub>a\<^sub>x\<^sub>y) 
+lemma Galaxy_OclAllInstances_at_pre_OclIsKindOf\<^sub>G\<^sub>a\<^sub>l\<^sub>a\<^sub>x\<^sub>y : 
+shows "\<tau> \<Turnstile> (OclForall ((OclAllInstances_at_pre (Galaxy))) (OclIsKindOf\<^sub>G\<^sub>a\<^sub>l\<^sub>a\<^sub>x\<^sub>y))"
+  unfolding OclAllInstances_at_pre_def
+by(rule Galaxy_OclAllInstances_generic_OclIsKindOf\<^sub>G\<^sub>a\<^sub>l\<^sub>a\<^sub>x\<^sub>y) 
+lemma OclAny_OclAllInstances_generic_OclIsKindOf\<^sub>O\<^sub>c\<^sub>l\<^sub>A\<^sub>n\<^sub>y : "\<tau> \<Turnstile> (OclForall ((OclAllInstances_generic (pre_post) (OclAny))) (OclIsKindOf\<^sub>O\<^sub>c\<^sub>l\<^sub>A\<^sub>n\<^sub>y))"
+  apply(simp add: OclValid_def del: OclAllInstances_generic_def OclIsKindOf\<^sub>O\<^sub>c\<^sub>l\<^sub>A\<^sub>n\<^sub>y_OclAny)
+  apply(simp only: OclForall_def refl if_True OclAllInstances_generic_defined[simplified OclValid_def])
+  apply(simp only: OclAllInstances_generic_def)
+  apply(subst (1 2 3) Abs_Set_0_inverse, simp add: bot_option_def)
+  apply(subst (1 2 3) ex_ssubst[where s = "(\<lambda>x. (((\<lambda>_. x) .oclIsKindOf(OclAny)) (\<tau>)))" and t = "(\<lambda>_. (true (\<tau>)))"])
+  apply(intro ballI actual_eq_static\<^sub>O\<^sub>c\<^sub>l\<^sub>A\<^sub>n\<^sub>y[simplified OclValid_def])
+  apply(drule ex_def, erule exE, simp)
+by(simp)
+lemma OclAny_OclAllInstances_at_post_OclIsKindOf\<^sub>O\<^sub>c\<^sub>l\<^sub>A\<^sub>n\<^sub>y : 
+shows "\<tau> \<Turnstile> (OclForall ((OclAllInstances_at_post (OclAny))) (OclIsKindOf\<^sub>O\<^sub>c\<^sub>l\<^sub>A\<^sub>n\<^sub>y))"
+  unfolding OclAllInstances_at_post_def
+by(rule OclAny_OclAllInstances_generic_OclIsKindOf\<^sub>O\<^sub>c\<^sub>l\<^sub>A\<^sub>n\<^sub>y) 
+lemma OclAny_OclAllInstances_at_pre_OclIsKindOf\<^sub>O\<^sub>c\<^sub>l\<^sub>A\<^sub>n\<^sub>y : 
+shows "\<tau> \<Turnstile> (OclForall ((OclAllInstances_at_pre (OclAny))) (OclIsKindOf\<^sub>O\<^sub>c\<^sub>l\<^sub>A\<^sub>n\<^sub>y))"
+  unfolding OclAllInstances_at_pre_def
+by(rule OclAny_OclAllInstances_generic_OclIsKindOf\<^sub>O\<^sub>c\<^sub>l\<^sub>A\<^sub>n\<^sub>y) 
+
+(* 94 ************************************ 603 + 18 *)
+lemma Person_OclAllInstances_generic_OclIsKindOf\<^sub>P\<^sub>l\<^sub>a\<^sub>n\<^sub>e\<^sub>t : "\<tau> \<Turnstile> (OclForall ((OclAllInstances_generic (pre_post) (Person))) (OclIsKindOf\<^sub>P\<^sub>l\<^sub>a\<^sub>n\<^sub>e\<^sub>t))"
+  apply(simp add: OclValid_def del: OclAllInstances_generic_def OclIsKindOf\<^sub>P\<^sub>l\<^sub>a\<^sub>n\<^sub>e\<^sub>t_Person)
+  apply(simp only: OclForall_def refl if_True OclAllInstances_generic_defined[simplified OclValid_def])
+  apply(simp only: OclAllInstances_generic_def)
+  apply(subst (1 2 3) Abs_Set_0_inverse, simp add: bot_option_def)
+  apply(subst (1 2 3) ex_ssubst[where s = "(\<lambda>x. (((\<lambda>_. x) .oclIsKindOf(Planet)) (\<tau>)))" and t = "(\<lambda>_. (true (\<tau>)))"])
+  apply(intro ballI actualKind\<^sub>P\<^sub>e\<^sub>r\<^sub>s\<^sub>o\<^sub>n_larger_staticKind\<^sub>P\<^sub>l\<^sub>a\<^sub>n\<^sub>e\<^sub>t[simplified OclValid_def])
+  apply(drule ex_def, erule exE, simp)
+by(simp)
+lemma Person_OclAllInstances_at_post_OclIsKindOf\<^sub>P\<^sub>l\<^sub>a\<^sub>n\<^sub>e\<^sub>t : 
+shows "\<tau> \<Turnstile> (OclForall ((OclAllInstances_at_post (Person))) (OclIsKindOf\<^sub>P\<^sub>l\<^sub>a\<^sub>n\<^sub>e\<^sub>t))"
+  unfolding OclAllInstances_at_post_def
+by(rule Person_OclAllInstances_generic_OclIsKindOf\<^sub>P\<^sub>l\<^sub>a\<^sub>n\<^sub>e\<^sub>t) 
+lemma Person_OclAllInstances_at_pre_OclIsKindOf\<^sub>P\<^sub>l\<^sub>a\<^sub>n\<^sub>e\<^sub>t : 
+shows "\<tau> \<Turnstile> (OclForall ((OclAllInstances_at_pre (Person))) (OclIsKindOf\<^sub>P\<^sub>l\<^sub>a\<^sub>n\<^sub>e\<^sub>t))"
+  unfolding OclAllInstances_at_pre_def
+by(rule Person_OclAllInstances_generic_OclIsKindOf\<^sub>P\<^sub>l\<^sub>a\<^sub>n\<^sub>e\<^sub>t) 
+lemma Person_OclAllInstances_generic_OclIsKindOf\<^sub>G\<^sub>a\<^sub>l\<^sub>a\<^sub>x\<^sub>y : "\<tau> \<Turnstile> (OclForall ((OclAllInstances_generic (pre_post) (Person))) (OclIsKindOf\<^sub>G\<^sub>a\<^sub>l\<^sub>a\<^sub>x\<^sub>y))"
+  apply(simp add: OclValid_def del: OclAllInstances_generic_def OclIsKindOf\<^sub>G\<^sub>a\<^sub>l\<^sub>a\<^sub>x\<^sub>y_Person)
+  apply(simp only: OclForall_def refl if_True OclAllInstances_generic_defined[simplified OclValid_def])
+  apply(simp only: OclAllInstances_generic_def)
+  apply(subst (1 2 3) Abs_Set_0_inverse, simp add: bot_option_def)
+  apply(subst (1 2 3) ex_ssubst[where s = "(\<lambda>x. (((\<lambda>_. x) .oclIsKindOf(Galaxy)) (\<tau>)))" and t = "(\<lambda>_. (true (\<tau>)))"])
+  apply(intro ballI actualKind\<^sub>P\<^sub>e\<^sub>r\<^sub>s\<^sub>o\<^sub>n_larger_staticKind\<^sub>G\<^sub>a\<^sub>l\<^sub>a\<^sub>x\<^sub>y[simplified OclValid_def])
+  apply(drule ex_def, erule exE, simp)
+by(simp)
+lemma Person_OclAllInstances_at_post_OclIsKindOf\<^sub>G\<^sub>a\<^sub>l\<^sub>a\<^sub>x\<^sub>y : 
+shows "\<tau> \<Turnstile> (OclForall ((OclAllInstances_at_post (Person))) (OclIsKindOf\<^sub>G\<^sub>a\<^sub>l\<^sub>a\<^sub>x\<^sub>y))"
+  unfolding OclAllInstances_at_post_def
+by(rule Person_OclAllInstances_generic_OclIsKindOf\<^sub>G\<^sub>a\<^sub>l\<^sub>a\<^sub>x\<^sub>y) 
+lemma Person_OclAllInstances_at_pre_OclIsKindOf\<^sub>G\<^sub>a\<^sub>l\<^sub>a\<^sub>x\<^sub>y : 
+shows "\<tau> \<Turnstile> (OclForall ((OclAllInstances_at_pre (Person))) (OclIsKindOf\<^sub>G\<^sub>a\<^sub>l\<^sub>a\<^sub>x\<^sub>y))"
+  unfolding OclAllInstances_at_pre_def
+by(rule Person_OclAllInstances_generic_OclIsKindOf\<^sub>G\<^sub>a\<^sub>l\<^sub>a\<^sub>x\<^sub>y) 
+lemma Person_OclAllInstances_generic_OclIsKindOf\<^sub>O\<^sub>c\<^sub>l\<^sub>A\<^sub>n\<^sub>y : "\<tau> \<Turnstile> (OclForall ((OclAllInstances_generic (pre_post) (Person))) (OclIsKindOf\<^sub>O\<^sub>c\<^sub>l\<^sub>A\<^sub>n\<^sub>y))"
+  apply(simp add: OclValid_def del: OclAllInstances_generic_def OclIsKindOf\<^sub>O\<^sub>c\<^sub>l\<^sub>A\<^sub>n\<^sub>y_Person)
+  apply(simp only: OclForall_def refl if_True OclAllInstances_generic_defined[simplified OclValid_def])
+  apply(simp only: OclAllInstances_generic_def)
+  apply(subst (1 2 3) Abs_Set_0_inverse, simp add: bot_option_def)
+  apply(subst (1 2 3) ex_ssubst[where s = "(\<lambda>x. (((\<lambda>_. x) .oclIsKindOf(OclAny)) (\<tau>)))" and t = "(\<lambda>_. (true (\<tau>)))"])
+  apply(intro ballI actualKind\<^sub>P\<^sub>e\<^sub>r\<^sub>s\<^sub>o\<^sub>n_larger_staticKind\<^sub>O\<^sub>c\<^sub>l\<^sub>A\<^sub>n\<^sub>y[simplified OclValid_def])
+  apply(drule ex_def, erule exE, simp)
+by(simp)
+lemma Person_OclAllInstances_at_post_OclIsKindOf\<^sub>O\<^sub>c\<^sub>l\<^sub>A\<^sub>n\<^sub>y : 
+shows "\<tau> \<Turnstile> (OclForall ((OclAllInstances_at_post (Person))) (OclIsKindOf\<^sub>O\<^sub>c\<^sub>l\<^sub>A\<^sub>n\<^sub>y))"
+  unfolding OclAllInstances_at_post_def
+by(rule Person_OclAllInstances_generic_OclIsKindOf\<^sub>O\<^sub>c\<^sub>l\<^sub>A\<^sub>n\<^sub>y) 
+lemma Person_OclAllInstances_at_pre_OclIsKindOf\<^sub>O\<^sub>c\<^sub>l\<^sub>A\<^sub>n\<^sub>y : 
+shows "\<tau> \<Turnstile> (OclForall ((OclAllInstances_at_pre (Person))) (OclIsKindOf\<^sub>O\<^sub>c\<^sub>l\<^sub>A\<^sub>n\<^sub>y))"
+  unfolding OclAllInstances_at_pre_def
+by(rule Person_OclAllInstances_generic_OclIsKindOf\<^sub>O\<^sub>c\<^sub>l\<^sub>A\<^sub>n\<^sub>y) 
+lemma Planet_OclAllInstances_generic_OclIsKindOf\<^sub>G\<^sub>a\<^sub>l\<^sub>a\<^sub>x\<^sub>y : "\<tau> \<Turnstile> (OclForall ((OclAllInstances_generic (pre_post) (Planet))) (OclIsKindOf\<^sub>G\<^sub>a\<^sub>l\<^sub>a\<^sub>x\<^sub>y))"
+  apply(simp add: OclValid_def del: OclAllInstances_generic_def OclIsKindOf\<^sub>G\<^sub>a\<^sub>l\<^sub>a\<^sub>x\<^sub>y_Planet)
+  apply(simp only: OclForall_def refl if_True OclAllInstances_generic_defined[simplified OclValid_def])
+  apply(simp only: OclAllInstances_generic_def)
+  apply(subst (1 2 3) Abs_Set_0_inverse, simp add: bot_option_def)
+  apply(subst (1 2 3) ex_ssubst[where s = "(\<lambda>x. (((\<lambda>_. x) .oclIsKindOf(Galaxy)) (\<tau>)))" and t = "(\<lambda>_. (true (\<tau>)))"])
+  apply(intro ballI actualKind\<^sub>P\<^sub>l\<^sub>a\<^sub>n\<^sub>e\<^sub>t_larger_staticKind\<^sub>G\<^sub>a\<^sub>l\<^sub>a\<^sub>x\<^sub>y[simplified OclValid_def])
+  apply(drule ex_def, erule exE, simp)
+by(simp)
+lemma Planet_OclAllInstances_at_post_OclIsKindOf\<^sub>G\<^sub>a\<^sub>l\<^sub>a\<^sub>x\<^sub>y : 
+shows "\<tau> \<Turnstile> (OclForall ((OclAllInstances_at_post (Planet))) (OclIsKindOf\<^sub>G\<^sub>a\<^sub>l\<^sub>a\<^sub>x\<^sub>y))"
+  unfolding OclAllInstances_at_post_def
+by(rule Planet_OclAllInstances_generic_OclIsKindOf\<^sub>G\<^sub>a\<^sub>l\<^sub>a\<^sub>x\<^sub>y) 
+lemma Planet_OclAllInstances_at_pre_OclIsKindOf\<^sub>G\<^sub>a\<^sub>l\<^sub>a\<^sub>x\<^sub>y : 
+shows "\<tau> \<Turnstile> (OclForall ((OclAllInstances_at_pre (Planet))) (OclIsKindOf\<^sub>G\<^sub>a\<^sub>l\<^sub>a\<^sub>x\<^sub>y))"
+  unfolding OclAllInstances_at_pre_def
+by(rule Planet_OclAllInstances_generic_OclIsKindOf\<^sub>G\<^sub>a\<^sub>l\<^sub>a\<^sub>x\<^sub>y) 
+lemma Planet_OclAllInstances_generic_OclIsKindOf\<^sub>O\<^sub>c\<^sub>l\<^sub>A\<^sub>n\<^sub>y : "\<tau> \<Turnstile> (OclForall ((OclAllInstances_generic (pre_post) (Planet))) (OclIsKindOf\<^sub>O\<^sub>c\<^sub>l\<^sub>A\<^sub>n\<^sub>y))"
+  apply(simp add: OclValid_def del: OclAllInstances_generic_def OclIsKindOf\<^sub>O\<^sub>c\<^sub>l\<^sub>A\<^sub>n\<^sub>y_Planet)
+  apply(simp only: OclForall_def refl if_True OclAllInstances_generic_defined[simplified OclValid_def])
+  apply(simp only: OclAllInstances_generic_def)
+  apply(subst (1 2 3) Abs_Set_0_inverse, simp add: bot_option_def)
+  apply(subst (1 2 3) ex_ssubst[where s = "(\<lambda>x. (((\<lambda>_. x) .oclIsKindOf(OclAny)) (\<tau>)))" and t = "(\<lambda>_. (true (\<tau>)))"])
+  apply(intro ballI actualKind\<^sub>P\<^sub>l\<^sub>a\<^sub>n\<^sub>e\<^sub>t_larger_staticKind\<^sub>O\<^sub>c\<^sub>l\<^sub>A\<^sub>n\<^sub>y[simplified OclValid_def])
+  apply(drule ex_def, erule exE, simp)
+by(simp)
+lemma Planet_OclAllInstances_at_post_OclIsKindOf\<^sub>O\<^sub>c\<^sub>l\<^sub>A\<^sub>n\<^sub>y : 
+shows "\<tau> \<Turnstile> (OclForall ((OclAllInstances_at_post (Planet))) (OclIsKindOf\<^sub>O\<^sub>c\<^sub>l\<^sub>A\<^sub>n\<^sub>y))"
+  unfolding OclAllInstances_at_post_def
+by(rule Planet_OclAllInstances_generic_OclIsKindOf\<^sub>O\<^sub>c\<^sub>l\<^sub>A\<^sub>n\<^sub>y) 
+lemma Planet_OclAllInstances_at_pre_OclIsKindOf\<^sub>O\<^sub>c\<^sub>l\<^sub>A\<^sub>n\<^sub>y : 
+shows "\<tau> \<Turnstile> (OclForall ((OclAllInstances_at_pre (Planet))) (OclIsKindOf\<^sub>O\<^sub>c\<^sub>l\<^sub>A\<^sub>n\<^sub>y))"
+  unfolding OclAllInstances_at_pre_def
+by(rule Planet_OclAllInstances_generic_OclIsKindOf\<^sub>O\<^sub>c\<^sub>l\<^sub>A\<^sub>n\<^sub>y) 
+lemma Galaxy_OclAllInstances_generic_OclIsKindOf\<^sub>O\<^sub>c\<^sub>l\<^sub>A\<^sub>n\<^sub>y : "\<tau> \<Turnstile> (OclForall ((OclAllInstances_generic (pre_post) (Galaxy))) (OclIsKindOf\<^sub>O\<^sub>c\<^sub>l\<^sub>A\<^sub>n\<^sub>y))"
+  apply(simp add: OclValid_def del: OclAllInstances_generic_def OclIsKindOf\<^sub>O\<^sub>c\<^sub>l\<^sub>A\<^sub>n\<^sub>y_Galaxy)
+  apply(simp only: OclForall_def refl if_True OclAllInstances_generic_defined[simplified OclValid_def])
+  apply(simp only: OclAllInstances_generic_def)
+  apply(subst (1 2 3) Abs_Set_0_inverse, simp add: bot_option_def)
+  apply(subst (1 2 3) ex_ssubst[where s = "(\<lambda>x. (((\<lambda>_. x) .oclIsKindOf(OclAny)) (\<tau>)))" and t = "(\<lambda>_. (true (\<tau>)))"])
+  apply(intro ballI actualKind\<^sub>G\<^sub>a\<^sub>l\<^sub>a\<^sub>x\<^sub>y_larger_staticKind\<^sub>O\<^sub>c\<^sub>l\<^sub>A\<^sub>n\<^sub>y[simplified OclValid_def])
+  apply(drule ex_def, erule exE, simp)
+by(simp)
+lemma Galaxy_OclAllInstances_at_post_OclIsKindOf\<^sub>O\<^sub>c\<^sub>l\<^sub>A\<^sub>n\<^sub>y : 
+shows "\<tau> \<Turnstile> (OclForall ((OclAllInstances_at_post (Galaxy))) (OclIsKindOf\<^sub>O\<^sub>c\<^sub>l\<^sub>A\<^sub>n\<^sub>y))"
+  unfolding OclAllInstances_at_post_def
+by(rule Galaxy_OclAllInstances_generic_OclIsKindOf\<^sub>O\<^sub>c\<^sub>l\<^sub>A\<^sub>n\<^sub>y) 
+lemma Galaxy_OclAllInstances_at_pre_OclIsKindOf\<^sub>O\<^sub>c\<^sub>l\<^sub>A\<^sub>n\<^sub>y : 
+shows "\<tau> \<Turnstile> (OclForall ((OclAllInstances_at_pre (Galaxy))) (OclIsKindOf\<^sub>O\<^sub>c\<^sub>l\<^sub>A\<^sub>n\<^sub>y))"
+  unfolding OclAllInstances_at_pre_def
+by(rule Galaxy_OclAllInstances_generic_OclIsKindOf\<^sub>O\<^sub>c\<^sub>l\<^sub>A\<^sub>n\<^sub>y) 
+
+(* 95 ************************************ 621 + 1 *)
 section{* The Accessors *}
 
-(* 90 ************************************ 565 + 1 *)
+(* 96 ************************************ 622 + 1 *)
 text{* 
   \label{sec:edm-accessors} *}
 
-(* 91 ************************************ 566 + 1 *)
+(* 97 ************************************ 623 + 1 *)
 text{*  *}
 
-(* 92 ************************************ 567 + 1 *)
+(* 98 ************************************ 624 + 1 *)
 subsection{* Definition *}
 
-(* 93 ************************************ 568 + 1 *)
+(* 99 ************************************ 625 + 1 *)
 text{*  *}
 
-(* 94 ************************************ 569 + 0 *)
+(* 100 ************************************ 626 + 0 *)
 
-(* 95 ************************************ 569 + 1 *)
+(* 101 ************************************ 626 + 1 *)
 text{*  *}
 
-(* 96 ************************************ 570 + 4 *)
+(* 102 ************************************ 627 + 4 *)
 definition "eval_extract x f = (\<lambda>\<tau>. (case x \<tau> of \<lfloor>\<lfloor>obj\<rfloor>\<rfloor> \<Rightarrow> (f ((oid_of (obj))) (\<tau>))
     | _ \<Rightarrow> invalid \<tau>))"
 definition "in_pre_state = fst"
 definition "in_post_state = snd"
 definition "reconst_basetype = id"
 
-(* 97 ************************************ 574 + 1 *)
+(* 103 ************************************ 631 + 1 *)
 text{*  *}
 
-(* 98 ************************************ 575 + 0 *)
+(* 104 ************************************ 632 + 0 *)
 
-(* 99 ************************************ 575 + 4 *)
+(* 105 ************************************ 632 + 4 *)
 definition "deref_oid\<^sub>P\<^sub>e\<^sub>r\<^sub>s\<^sub>o\<^sub>n fst_snd f oid = (\<lambda>\<tau>. (case (heap (fst_snd \<tau>) (oid)) of \<lfloor>in\<^sub>P\<^sub>e\<^sub>r\<^sub>s\<^sub>o\<^sub>n obj\<rfloor> \<Rightarrow> f obj \<tau>
     | _ \<Rightarrow> invalid \<tau>))"
 definition "deref_oid\<^sub>P\<^sub>l\<^sub>a\<^sub>n\<^sub>e\<^sub>t fst_snd f oid = (\<lambda>\<tau>. (case (heap (fst_snd \<tau>) (oid)) of \<lfloor>in\<^sub>P\<^sub>l\<^sub>a\<^sub>n\<^sub>e\<^sub>t obj\<rfloor> \<Rightarrow> f obj \<tau>
@@ -2212,18 +2535,18 @@ definition "deref_oid\<^sub>G\<^sub>a\<^sub>l\<^sub>a\<^sub>x\<^sub>y fst_snd f 
 definition "deref_oid\<^sub>O\<^sub>c\<^sub>l\<^sub>A\<^sub>n\<^sub>y fst_snd f oid = (\<lambda>\<tau>. (case (heap (fst_snd \<tau>) (oid)) of \<lfloor>in\<^sub>O\<^sub>c\<^sub>l\<^sub>A\<^sub>n\<^sub>y obj\<rfloor> \<Rightarrow> f obj \<tau>
     | _ \<Rightarrow> invalid \<tau>))"
 
-(* 100 ************************************ 579 + 0 *)
+(* 106 ************************************ 636 + 0 *)
 
-(* 101 ************************************ 579 + 1 *)
+(* 107 ************************************ 636 + 1 *)
 text{*  *}
 
-(* 102 ************************************ 580 + 0 *)
+(* 108 ************************************ 637 + 0 *)
 
-(* 103 ************************************ 580 + 1 *)
+(* 109 ************************************ 637 + 1 *)
 text{* 
    pointer undefined in state or not referencing a type conform object representation  *}
 
-(* 104 ************************************ 581 + 10 *)
+(* 110 ************************************ 638 + 10 *)
 definition "select\<^sub>P\<^sub>e\<^sub>r\<^sub>s\<^sub>o\<^sub>n\<S>\<A>\<L>\<A>\<R>\<Y> f = (\<lambda> (mkoid\<^sub>P\<^sub>e\<^sub>r\<^sub>s\<^sub>o\<^sub>n (_) (\<bottom>) (_)) \<Rightarrow> null
     | (mkoid\<^sub>P\<^sub>e\<^sub>r\<^sub>s\<^sub>o\<^sub>n (_) (\<lfloor>salary\<rfloor>) (_)) \<Rightarrow> (f ((\<lambda>x _. \<lfloor>\<lfloor>x\<rfloor>\<rfloor>)) (salary)))"
 definition "select\<^sub>P\<^sub>e\<^sub>r\<^sub>s\<^sub>o\<^sub>n\<B>\<O>\<S>\<S> f = (\<lambda> (mkoid\<^sub>P\<^sub>e\<^sub>r\<^sub>s\<^sub>o\<^sub>n (_) (_) (\<bottom>)) \<Rightarrow> null
@@ -2247,9 +2570,9 @@ definition "select\<^sub>P\<^sub>l\<^sub>a\<^sub>n\<^sub>e\<^sub>t\<M>\<O>\<V>\<
     | (mkoid\<^sub>P\<^sub>l\<^sub>a\<^sub>n\<^sub>e\<^sub>t ((mk\<^sub>P\<^sub>l\<^sub>a\<^sub>n\<^sub>e\<^sub>t (_) (_) (\<lfloor>moving\<rfloor>))) (_)) \<Rightarrow> (f ((\<lambda>x _. \<lfloor>\<lfloor>x\<rfloor>\<rfloor>)) (moving))
     | (mkoid\<^sub>P\<^sub>l\<^sub>a\<^sub>n\<^sub>e\<^sub>t ((mk\<^sub>P\<^sub>l\<^sub>a\<^sub>n\<^sub>e\<^sub>t_\<^sub>P\<^sub>e\<^sub>r\<^sub>s\<^sub>o\<^sub>n (person))) (_)) \<Rightarrow> (select\<^sub>P\<^sub>e\<^sub>r\<^sub>s\<^sub>o\<^sub>n\<M>\<O>\<V>\<I>\<N>\<G> (f) (person)))"
 
-(* 105 ************************************ 591 + 0 *)
+(* 111 ************************************ 648 + 0 *)
 
-(* 106 ************************************ 591 + 10 *)
+(* 112 ************************************ 648 + 10 *)
 consts dot\<S>\<A>\<L>\<A>\<R>\<Y> :: "(\<AA>, '\<alpha>) val \<Rightarrow> (\<AA>, int option option) val" ("(_) .salary")
 consts dot\<S>\<A>\<L>\<A>\<R>\<Y>at_pre :: "(\<AA>, '\<alpha>) val \<Rightarrow> (\<AA>, int option option) val" ("(_) .salary@pre")
 consts dot\<B>\<O>\<S>\<S> :: "(\<AA>, '\<alpha>) val \<Rightarrow> Person" ("(_) .boss")
@@ -2261,7 +2584,7 @@ consts dot\<S>\<O>\<U>\<N>\<D>at_pre :: "(\<AA>, '\<alpha>) val \<Rightarrow> (\
 consts dot\<M>\<O>\<V>\<I>\<N>\<G> :: "(\<AA>, '\<alpha>) val \<Rightarrow> (\<AA>, bool option option) val" ("(_) .moving")
 consts dot\<M>\<O>\<V>\<I>\<N>\<G>at_pre :: "(\<AA>, '\<alpha>) val \<Rightarrow> (\<AA>, bool option option) val" ("(_) .moving@pre")
 
-(* 107 ************************************ 601 + 20 *)
+(* 113 ************************************ 658 + 20 *)
 defs(overloaded) dot\<^sub>P\<^sub>e\<^sub>r\<^sub>s\<^sub>o\<^sub>n\<S>\<A>\<L>\<A>\<R>\<Y> : "(x::Person) .salary \<equiv> (eval_extract (x) ((deref_oid\<^sub>P\<^sub>e\<^sub>r\<^sub>s\<^sub>o\<^sub>n (in_post_state) ((select\<^sub>P\<^sub>e\<^sub>r\<^sub>s\<^sub>o\<^sub>n\<S>\<A>\<L>\<A>\<R>\<Y> (reconst_basetype))))))"
 defs(overloaded) dot\<^sub>P\<^sub>e\<^sub>r\<^sub>s\<^sub>o\<^sub>n\<B>\<O>\<S>\<S> : "(x::Person) .boss \<equiv> (eval_extract (x) ((deref_oid\<^sub>P\<^sub>e\<^sub>r\<^sub>s\<^sub>o\<^sub>n (in_post_state) ((select\<^sub>P\<^sub>e\<^sub>r\<^sub>s\<^sub>o\<^sub>n\<B>\<O>\<S>\<S> ((deref_oid\<^sub>P\<^sub>e\<^sub>r\<^sub>s\<^sub>o\<^sub>n (in_post_state))))))))"
 defs(overloaded) dot\<^sub>P\<^sub>e\<^sub>r\<^sub>s\<^sub>o\<^sub>n\<S>\<A>\<L>\<A>\<R>\<Y>at_pre : "(x::Person) .salary@pre \<equiv> (eval_extract (x) ((deref_oid\<^sub>P\<^sub>e\<^sub>r\<^sub>s\<^sub>o\<^sub>n (in_pre_state) ((select\<^sub>P\<^sub>e\<^sub>r\<^sub>s\<^sub>o\<^sub>n\<S>\<A>\<L>\<A>\<R>\<Y> (reconst_basetype))))))"
@@ -2283,7 +2606,7 @@ defs(overloaded) dot\<^sub>P\<^sub>l\<^sub>a\<^sub>n\<^sub>e\<^sub>t\<M>\<O>\<V>
 defs(overloaded) dot\<^sub>P\<^sub>l\<^sub>a\<^sub>n\<^sub>e\<^sub>t\<S>\<O>\<U>\<N>\<D>at_pre : "(x::Planet) .sound@pre \<equiv> (eval_extract (x) ((deref_oid\<^sub>P\<^sub>l\<^sub>a\<^sub>n\<^sub>e\<^sub>t (in_pre_state) ((select\<^sub>P\<^sub>l\<^sub>a\<^sub>n\<^sub>e\<^sub>t\<S>\<O>\<U>\<N>\<D> (reconst_basetype))))))"
 defs(overloaded) dot\<^sub>P\<^sub>l\<^sub>a\<^sub>n\<^sub>e\<^sub>t\<M>\<O>\<V>\<I>\<N>\<G>at_pre : "(x::Planet) .moving@pre \<equiv> (eval_extract (x) ((deref_oid\<^sub>P\<^sub>l\<^sub>a\<^sub>n\<^sub>e\<^sub>t (in_pre_state) ((select\<^sub>P\<^sub>l\<^sub>a\<^sub>n\<^sub>e\<^sub>t\<M>\<O>\<V>\<I>\<N>\<G> (reconst_basetype))))))"
 
-(* 108 ************************************ 621 + 1 *)
+(* 114 ************************************ 678 + 1 *)
 lemmas [simp,code_unfold] = dot\<^sub>P\<^sub>e\<^sub>r\<^sub>s\<^sub>o\<^sub>n\<S>\<A>\<L>\<A>\<R>\<Y>
                             dot\<^sub>P\<^sub>e\<^sub>r\<^sub>s\<^sub>o\<^sub>n\<B>\<O>\<S>\<S>
                             dot\<^sub>P\<^sub>e\<^sub>r\<^sub>s\<^sub>o\<^sub>n\<S>\<A>\<L>\<A>\<R>\<Y>at_pre
@@ -2305,13 +2628,13 @@ lemmas [simp,code_unfold] = dot\<^sub>P\<^sub>e\<^sub>r\<^sub>s\<^sub>o\<^sub>n\
                             dot\<^sub>P\<^sub>l\<^sub>a\<^sub>n\<^sub>e\<^sub>t\<S>\<O>\<U>\<N>\<D>at_pre
                             dot\<^sub>P\<^sub>l\<^sub>a\<^sub>n\<^sub>e\<^sub>t\<M>\<O>\<V>\<I>\<N>\<G>at_pre
 
-(* 109 ************************************ 622 + 1 *)
+(* 115 ************************************ 679 + 1 *)
 subsection{* Context Passing *}
 
-(* 110 ************************************ 623 + 1 *)
+(* 116 ************************************ 680 + 1 *)
 lemmas [simp,code_unfold] = eval_extract_def
 
-(* 111 ************************************ 624 + 20 *)
+(* 117 ************************************ 681 + 20 *)
 lemma cp_dot\<^sub>P\<^sub>e\<^sub>r\<^sub>s\<^sub>o\<^sub>n\<S>\<A>\<L>\<A>\<R>\<Y> : "(cp ((\<lambda>X. (X::Person) .salary)))"
 by(auto simp: cp_def)
 lemma cp_dot\<^sub>P\<^sub>e\<^sub>r\<^sub>s\<^sub>o\<^sub>n\<B>\<O>\<S>\<S> : "(cp ((\<lambda>X. (X::Person) .boss)))"
@@ -2353,7 +2676,7 @@ by(auto simp: cp_def)
 lemma cp_dot\<^sub>P\<^sub>l\<^sub>a\<^sub>n\<^sub>e\<^sub>t\<M>\<O>\<V>\<I>\<N>\<G>at_pre : "(cp ((\<lambda>X. (X::Planet) .moving@pre)))"
 by(auto simp: cp_def)
 
-(* 112 ************************************ 644 + 1 *)
+(* 118 ************************************ 701 + 1 *)
 lemmas [simp,code_unfold] = cp_dot\<^sub>P\<^sub>e\<^sub>r\<^sub>s\<^sub>o\<^sub>n\<S>\<A>\<L>\<A>\<R>\<Y>
                             cp_dot\<^sub>P\<^sub>e\<^sub>r\<^sub>s\<^sub>o\<^sub>n\<B>\<O>\<S>\<S>
                             cp_dot\<^sub>P\<^sub>e\<^sub>r\<^sub>s\<^sub>o\<^sub>n\<S>\<A>\<L>\<A>\<R>\<Y>at_pre
@@ -2375,10 +2698,10 @@ lemmas [simp,code_unfold] = cp_dot\<^sub>P\<^sub>e\<^sub>r\<^sub>s\<^sub>o\<^sub
                             cp_dot\<^sub>P\<^sub>l\<^sub>a\<^sub>n\<^sub>e\<^sub>t\<S>\<O>\<U>\<N>\<D>at_pre
                             cp_dot\<^sub>P\<^sub>l\<^sub>a\<^sub>n\<^sub>e\<^sub>t\<M>\<O>\<V>\<I>\<N>\<G>at_pre
 
-(* 113 ************************************ 645 + 1 *)
+(* 119 ************************************ 702 + 1 *)
 subsection{* Execution with Invalid or Null as Argument *}
 
-(* 114 ************************************ 646 + 40 *)
+(* 120 ************************************ 703 + 40 *)
 lemma dot\<^sub>P\<^sub>e\<^sub>r\<^sub>s\<^sub>o\<^sub>n\<S>\<A>\<L>\<A>\<R>\<Y>_invalid : "(invalid::Person) .salary = invalid"
 by(rule ext, simp add: bot_option_def invalid_def)
 lemma dot\<^sub>P\<^sub>e\<^sub>r\<^sub>s\<^sub>o\<^sub>n\<S>\<A>\<L>\<A>\<R>\<Y>_null : "(null::Person) .salary = invalid"
@@ -2460,12 +2783,12 @@ by(rule ext, simp add: bot_option_def invalid_def)
 lemma dot\<^sub>P\<^sub>l\<^sub>a\<^sub>n\<^sub>e\<^sub>t\<M>\<O>\<V>\<I>\<N>\<G>at_pre_null : "(null::Planet) .moving@pre = invalid"
 by(rule ext, simp add: bot_option_def null_fun_def null_option_def)
 
-(* 115 ************************************ 686 + 1 *)
+(* 121 ************************************ 743 + 1 *)
 section{* A Little Infra-structure on Example States *}
 
-(* 116 ************************************ 687 + 1 *)
+(* 122 ************************************ 744 + 1 *)
 text{* 
-  
+
 The example we are defining in this section comes from the figure~\ref{fig:edm1_system-states}.
 \begin{figure}
 \includegraphics[width=\textwidth]{figures/pre-post.pdf}
@@ -2475,13 +2798,28 @@ The example we are defining in this section comes from the figure~\ref{fig:edm1_
 \end{figure}
  *}
 
-(* 117 ************************************ 688 + 1 *)
+(* 123 ************************************ 745 + 1 *)
 text{*  *}
 
-(* 118 ************************************ 689 + 1 *)
+(* 124 ************************************ 746 + 1 *)
 lemmas [simp,code_unfold] = state.defs
+                            const_ss
 
-(* 119 ************************************ 690 + 8 *)
+(* 125 ************************************ 747 + 1 *)
+lemmas [simp,code_unfold] = OclAsType\<^sub>P\<^sub>e\<^sub>r\<^sub>s\<^sub>o\<^sub>n_Planet
+                            OclAsType\<^sub>P\<^sub>e\<^sub>r\<^sub>s\<^sub>o\<^sub>n_Galaxy
+                            OclAsType\<^sub>P\<^sub>e\<^sub>r\<^sub>s\<^sub>o\<^sub>n_OclAny
+                            OclAsType\<^sub>P\<^sub>l\<^sub>a\<^sub>n\<^sub>e\<^sub>t_Person
+                            OclAsType\<^sub>P\<^sub>l\<^sub>a\<^sub>n\<^sub>e\<^sub>t_Galaxy
+                            OclAsType\<^sub>P\<^sub>l\<^sub>a\<^sub>n\<^sub>e\<^sub>t_OclAny
+                            OclAsType\<^sub>G\<^sub>a\<^sub>l\<^sub>a\<^sub>x\<^sub>y_Person
+                            OclAsType\<^sub>G\<^sub>a\<^sub>l\<^sub>a\<^sub>x\<^sub>y_Planet
+                            OclAsType\<^sub>G\<^sub>a\<^sub>l\<^sub>a\<^sub>x\<^sub>y_OclAny
+                            OclAsType\<^sub>O\<^sub>c\<^sub>l\<^sub>A\<^sub>n\<^sub>y_Person
+                            OclAsType\<^sub>O\<^sub>c\<^sub>l\<^sub>A\<^sub>n\<^sub>y_Planet
+                            OclAsType\<^sub>O\<^sub>c\<^sub>l\<^sub>A\<^sub>n\<^sub>y_Galaxy
+
+(* 126 ************************************ 748 + 8 *)
 definition OclInt1000 ("\<one>\<zero>\<zero>\<zero>")
   where "OclInt1000 = (\<lambda>_. \<lfloor>\<lfloor>1000\<rfloor>\<rfloor>)"
 definition OclInt1200 ("\<one>\<two>\<zero>\<zero>")
@@ -2499,7 +2837,7 @@ definition OclInt3200 ("\<three>\<two>\<zero>\<zero>")
 definition OclInt3500 ("\<three>\<five>\<zero>\<zero>")
   where "OclInt3500 = (\<lambda>_. \<lfloor>\<lfloor>3500\<rfloor>\<rfloor>)"
 
-(* 120 ************************************ 698 + 27 *)
+(* 127 ************************************ 756 + 27 *)
 definition "oid0 = 0"
 definition "oid1 = 1"
 definition "oid2 = 2"
@@ -2528,13 +2866,333 @@ definition "(X\<^sub>P\<^sub>e\<^sub>r\<^sub>s\<^sub>o\<^sub>n7::OclAny) = (\<la
 definition "(X\<^sub>P\<^sub>e\<^sub>r\<^sub>s\<^sub>o\<^sub>n8::OclAny) = (\<lambda>_. \<lfloor>\<lfloor>X\<^sub>P\<^sub>e\<^sub>r\<^sub>s\<^sub>o\<^sub>n8\<^sub>O\<^sub>c\<^sub>l\<^sub>A\<^sub>n\<^sub>y\<rfloor>\<rfloor>)"
 definition "(X\<^sub>P\<^sub>e\<^sub>r\<^sub>s\<^sub>o\<^sub>n9::Person) = (\<lambda>_. \<lfloor>\<lfloor>X\<^sub>P\<^sub>e\<^sub>r\<^sub>s\<^sub>o\<^sub>n9\<^sub>P\<^sub>e\<^sub>r\<^sub>s\<^sub>o\<^sub>n\<rfloor>\<rfloor>)"
 
-(* 121 ************************************ 725 + 1 *)
+(* 128 ************************************ 783 + 1 *)
 definition "\<sigma>\<^sub>1 = (state.make ((Map.empty (oid0 \<mapsto> (in\<^sub>P\<^sub>e\<^sub>r\<^sub>s\<^sub>o\<^sub>n ((mkoid\<^sub>P\<^sub>e\<^sub>r\<^sub>s\<^sub>o\<^sub>n ((mk\<^sub>P\<^sub>e\<^sub>r\<^sub>s\<^sub>o\<^sub>n (oid0) (None) (None) (None))) (\<lfloor>1000\<rfloor>) (\<lfloor>oid1\<rfloor>))))) (oid1 \<mapsto> (in\<^sub>P\<^sub>e\<^sub>r\<^sub>s\<^sub>o\<^sub>n ((mkoid\<^sub>P\<^sub>e\<^sub>r\<^sub>s\<^sub>o\<^sub>n ((mk\<^sub>P\<^sub>e\<^sub>r\<^sub>s\<^sub>o\<^sub>n (oid1) (None) (None) (None))) (\<lfloor>1200\<rfloor>) (None))))) (oid3 \<mapsto> (in\<^sub>P\<^sub>e\<^sub>r\<^sub>s\<^sub>o\<^sub>n ((mkoid\<^sub>P\<^sub>e\<^sub>r\<^sub>s\<^sub>o\<^sub>n ((mk\<^sub>P\<^sub>e\<^sub>r\<^sub>s\<^sub>o\<^sub>n (oid3) (None) (None) (None))) (\<lfloor>2600\<rfloor>) (\<lfloor>oid4\<rfloor>))))) (oid4 \<mapsto> (in\<^sub>P\<^sub>e\<^sub>r\<^sub>s\<^sub>o\<^sub>n (X\<^sub>P\<^sub>e\<^sub>r\<^sub>s\<^sub>o\<^sub>n5\<^sub>P\<^sub>e\<^sub>r\<^sub>s\<^sub>o\<^sub>n))) (oid5 \<mapsto> (in\<^sub>P\<^sub>e\<^sub>r\<^sub>s\<^sub>o\<^sub>n ((mkoid\<^sub>P\<^sub>e\<^sub>r\<^sub>s\<^sub>o\<^sub>n ((mk\<^sub>P\<^sub>e\<^sub>r\<^sub>s\<^sub>o\<^sub>n (oid5) (None) (None) (None))) (\<lfloor>2300\<rfloor>) (\<lfloor>oid3\<rfloor>))))) (oid8 \<mapsto> (in\<^sub>P\<^sub>e\<^sub>r\<^sub>s\<^sub>o\<^sub>n (X\<^sub>P\<^sub>e\<^sub>r\<^sub>s\<^sub>o\<^sub>n9\<^sub>P\<^sub>e\<^sub>r\<^sub>s\<^sub>o\<^sub>n))))) (Map.empty) (Map.empty))"
 
-(* 122 ************************************ 726 + 1 *)
+(* 129 ************************************ 784 + 1 *)
+lemma dom_\<sigma>\<^sub>1 : "(dom ((heap (\<sigma>\<^sub>1)))) = {oid0 , oid1 , oid3 , oid4 , oid5 , oid8}"
+by(auto simp: \<sigma>\<^sub>1_def)
+
+(* 130 ************************************ 785 + 1 *)
+lemmas [simp,code_unfold] = dom_\<sigma>\<^sub>1
+
+(* 131 ************************************ 786 + 1 *)
+lemma perm_\<sigma>\<^sub>1 : "\<sigma>\<^sub>1 = (state.make ((Map.empty (oid8 \<mapsto> (in\<^sub>P\<^sub>e\<^sub>r\<^sub>s\<^sub>o\<^sub>n (X\<^sub>P\<^sub>e\<^sub>r\<^sub>s\<^sub>o\<^sub>n9\<^sub>P\<^sub>e\<^sub>r\<^sub>s\<^sub>o\<^sub>n))) (oid5 \<mapsto> (in\<^sub>P\<^sub>e\<^sub>r\<^sub>s\<^sub>o\<^sub>n ((mkoid\<^sub>P\<^sub>e\<^sub>r\<^sub>s\<^sub>o\<^sub>n ((mk\<^sub>P\<^sub>e\<^sub>r\<^sub>s\<^sub>o\<^sub>n (oid5) (None) (None) (None))) (\<lfloor>2300\<rfloor>) (\<lfloor>oid3\<rfloor>))))) (oid4 \<mapsto> (in\<^sub>P\<^sub>e\<^sub>r\<^sub>s\<^sub>o\<^sub>n (X\<^sub>P\<^sub>e\<^sub>r\<^sub>s\<^sub>o\<^sub>n5\<^sub>P\<^sub>e\<^sub>r\<^sub>s\<^sub>o\<^sub>n))) (oid3 \<mapsto> (in\<^sub>P\<^sub>e\<^sub>r\<^sub>s\<^sub>o\<^sub>n ((mkoid\<^sub>P\<^sub>e\<^sub>r\<^sub>s\<^sub>o\<^sub>n ((mk\<^sub>P\<^sub>e\<^sub>r\<^sub>s\<^sub>o\<^sub>n (oid3) (None) (None) (None))) (\<lfloor>2600\<rfloor>) (\<lfloor>oid4\<rfloor>))))) (oid1 \<mapsto> (in\<^sub>P\<^sub>e\<^sub>r\<^sub>s\<^sub>o\<^sub>n ((mkoid\<^sub>P\<^sub>e\<^sub>r\<^sub>s\<^sub>o\<^sub>n ((mk\<^sub>P\<^sub>e\<^sub>r\<^sub>s\<^sub>o\<^sub>n (oid1) (None) (None) (None))) (\<lfloor>1200\<rfloor>) (None))))) (oid0 \<mapsto> (in\<^sub>P\<^sub>e\<^sub>r\<^sub>s\<^sub>o\<^sub>n ((mkoid\<^sub>P\<^sub>e\<^sub>r\<^sub>s\<^sub>o\<^sub>n ((mk\<^sub>P\<^sub>e\<^sub>r\<^sub>s\<^sub>o\<^sub>n (oid0) (None) (None) (None))) (\<lfloor>1000\<rfloor>) (\<lfloor>oid1\<rfloor>))))))) ((assocs\<^sub>2 (\<sigma>\<^sub>1))) ((assocs\<^sub>3 (\<sigma>\<^sub>1))))"
+  apply(simp add: \<sigma>\<^sub>1_def oid0_def oid1_def oid3_def oid4_def oid5_def oid8_def)
+  apply(subst (1) fun_upd_twist, simp)
+  apply(subst (2) fun_upd_twist, simp)
+  apply(subst (1) fun_upd_twist, simp)
+  apply(subst (3) fun_upd_twist, simp)
+  apply(subst (2) fun_upd_twist, simp)
+  apply(subst (1) fun_upd_twist, simp)
+  apply(subst (4) fun_upd_twist, simp)
+  apply(subst (3) fun_upd_twist, simp)
+  apply(subst (2) fun_upd_twist, simp)
+  apply(subst (1) fun_upd_twist, simp)
+  apply(subst (5) fun_upd_twist, simp)
+  apply(subst (4) fun_upd_twist, simp)
+  apply(subst (3) fun_upd_twist, simp)
+  apply(subst (2) fun_upd_twist, simp)
+  apply(subst (1) fun_upd_twist, simp)
+by(simp)
+
+(* 132 ************************************ 787 + 12 *)
+lemma \<sigma>\<^sub>1_OclAllInstances_generic_exec_Person : 
+assumes [simp]: "(\<And>a. (pre_post ((mk (a)))) = a)"
+shows "(mk (\<sigma>\<^sub>1)) \<Turnstile> (OclAllInstances_generic (pre_post) (Person)) \<doteq> Set{(\<lambda>_. \<lfloor>\<lfloor>(mkoid\<^sub>P\<^sub>e\<^sub>r\<^sub>s\<^sub>o\<^sub>n ((mk\<^sub>P\<^sub>e\<^sub>r\<^sub>s\<^sub>o\<^sub>n (oid0) (None) (None) (None))) (\<lfloor>1000\<rfloor>) (\<lfloor>oid1\<rfloor>))\<rfloor>\<rfloor>) , (\<lambda>_. \<lfloor>\<lfloor>(mkoid\<^sub>P\<^sub>e\<^sub>r\<^sub>s\<^sub>o\<^sub>n ((mk\<^sub>P\<^sub>e\<^sub>r\<^sub>s\<^sub>o\<^sub>n (oid1) (None) (None) (None))) (\<lfloor>1200\<rfloor>) (None))\<rfloor>\<rfloor>) , (\<lambda>_. \<lfloor>\<lfloor>(mkoid\<^sub>P\<^sub>e\<^sub>r\<^sub>s\<^sub>o\<^sub>n ((mk\<^sub>P\<^sub>e\<^sub>r\<^sub>s\<^sub>o\<^sub>n (oid3) (None) (None) (None))) (\<lfloor>2600\<rfloor>) (\<lfloor>oid4\<rfloor>))\<rfloor>\<rfloor>) , X\<^sub>P\<^sub>e\<^sub>r\<^sub>s\<^sub>o\<^sub>n5 , (\<lambda>_. \<lfloor>\<lfloor>(mkoid\<^sub>P\<^sub>e\<^sub>r\<^sub>s\<^sub>o\<^sub>n ((mk\<^sub>P\<^sub>e\<^sub>r\<^sub>s\<^sub>o\<^sub>n (oid5) (None) (None) (None))) (\<lfloor>2300\<rfloor>) (\<lfloor>oid3\<rfloor>))\<rfloor>\<rfloor>) , X\<^sub>P\<^sub>e\<^sub>r\<^sub>s\<^sub>o\<^sub>n9}"
+  apply(subst perm_\<sigma>\<^sub>1)
+  apply(simp only: state.make_def oid0_def oid1_def oid3_def oid4_def oid5_def oid8_def X\<^sub>P\<^sub>e\<^sub>r\<^sub>s\<^sub>o\<^sub>n5_def X\<^sub>P\<^sub>e\<^sub>r\<^sub>s\<^sub>o\<^sub>n9_def)
+  apply(subst state_update_vs_allInstances_generic_tc, simp, simp, simp add: OclAsType\<^sub>P\<^sub>e\<^sub>r\<^sub>s\<^sub>o\<^sub>n_\<AA>_def, simp, rule const_StrictRefEq\<^sub>S\<^sub>e\<^sub>t_including, simp, simp, simp, rule OclIncluding_cong, simp, simp)
+  apply(subst state_update_vs_allInstances_generic_tc, simp, simp, simp add: OclAsType\<^sub>P\<^sub>e\<^sub>r\<^sub>s\<^sub>o\<^sub>n_\<AA>_def, simp, rule const_StrictRefEq\<^sub>S\<^sub>e\<^sub>t_including, simp, simp, simp, rule OclIncluding_cong, simp, simp)
+  apply(subst state_update_vs_allInstances_generic_tc, simp, simp, simp add: OclAsType\<^sub>P\<^sub>e\<^sub>r\<^sub>s\<^sub>o\<^sub>n_\<AA>_def, simp, rule const_StrictRefEq\<^sub>S\<^sub>e\<^sub>t_including, simp, simp, simp, rule OclIncluding_cong, simp, simp)
+  apply(subst state_update_vs_allInstances_generic_tc, simp, simp, simp add: OclAsType\<^sub>P\<^sub>e\<^sub>r\<^sub>s\<^sub>o\<^sub>n_\<AA>_def, simp, rule const_StrictRefEq\<^sub>S\<^sub>e\<^sub>t_including, simp, simp, simp, rule OclIncluding_cong, simp, simp)
+  apply(subst state_update_vs_allInstances_generic_tc, simp, simp, simp add: OclAsType\<^sub>P\<^sub>e\<^sub>r\<^sub>s\<^sub>o\<^sub>n_\<AA>_def, simp, rule const_StrictRefEq\<^sub>S\<^sub>e\<^sub>t_including, simp, simp, simp, rule OclIncluding_cong, simp, simp)
+  apply(subst state_update_vs_allInstances_generic_tc, simp, simp, simp add: OclAsType\<^sub>P\<^sub>e\<^sub>r\<^sub>s\<^sub>o\<^sub>n_\<AA>_def, simp, rule const_StrictRefEq\<^sub>S\<^sub>e\<^sub>t_including, simp, simp, simp, rule OclIncluding_cong, simp, simp)
+  apply(rule state_update_vs_allInstances_generic_empty)
+by((simp add: OclAsType\<^sub>P\<^sub>e\<^sub>r\<^sub>s\<^sub>o\<^sub>n_\<AA>_def)+) 
+lemma \<sigma>\<^sub>1_OclAllInstances_at_post_exec_Person : 
+shows "(st , \<sigma>\<^sub>1) \<Turnstile> (OclAllInstances_at_post (Person)) \<doteq> Set{(\<lambda>_. \<lfloor>\<lfloor>(mkoid\<^sub>P\<^sub>e\<^sub>r\<^sub>s\<^sub>o\<^sub>n ((mk\<^sub>P\<^sub>e\<^sub>r\<^sub>s\<^sub>o\<^sub>n (oid0) (None) (None) (None))) (\<lfloor>1000\<rfloor>) (\<lfloor>oid1\<rfloor>))\<rfloor>\<rfloor>) , (\<lambda>_. \<lfloor>\<lfloor>(mkoid\<^sub>P\<^sub>e\<^sub>r\<^sub>s\<^sub>o\<^sub>n ((mk\<^sub>P\<^sub>e\<^sub>r\<^sub>s\<^sub>o\<^sub>n (oid1) (None) (None) (None))) (\<lfloor>1200\<rfloor>) (None))\<rfloor>\<rfloor>) , (\<lambda>_. \<lfloor>\<lfloor>(mkoid\<^sub>P\<^sub>e\<^sub>r\<^sub>s\<^sub>o\<^sub>n ((mk\<^sub>P\<^sub>e\<^sub>r\<^sub>s\<^sub>o\<^sub>n (oid3) (None) (None) (None))) (\<lfloor>2600\<rfloor>) (\<lfloor>oid4\<rfloor>))\<rfloor>\<rfloor>) , X\<^sub>P\<^sub>e\<^sub>r\<^sub>s\<^sub>o\<^sub>n5 , (\<lambda>_. \<lfloor>\<lfloor>(mkoid\<^sub>P\<^sub>e\<^sub>r\<^sub>s\<^sub>o\<^sub>n ((mk\<^sub>P\<^sub>e\<^sub>r\<^sub>s\<^sub>o\<^sub>n (oid5) (None) (None) (None))) (\<lfloor>2300\<rfloor>) (\<lfloor>oid3\<rfloor>))\<rfloor>\<rfloor>) , X\<^sub>P\<^sub>e\<^sub>r\<^sub>s\<^sub>o\<^sub>n9}"
+  unfolding OclAllInstances_at_post_def
+by(rule \<sigma>\<^sub>1_OclAllInstances_generic_exec_Person, simp) 
+lemma \<sigma>\<^sub>1_OclAllInstances_at_pre_exec_Person : 
+shows "(\<sigma>\<^sub>1 , st) \<Turnstile> (OclAllInstances_at_pre (Person)) \<doteq> Set{(\<lambda>_. \<lfloor>\<lfloor>(mkoid\<^sub>P\<^sub>e\<^sub>r\<^sub>s\<^sub>o\<^sub>n ((mk\<^sub>P\<^sub>e\<^sub>r\<^sub>s\<^sub>o\<^sub>n (oid0) (None) (None) (None))) (\<lfloor>1000\<rfloor>) (\<lfloor>oid1\<rfloor>))\<rfloor>\<rfloor>) , (\<lambda>_. \<lfloor>\<lfloor>(mkoid\<^sub>P\<^sub>e\<^sub>r\<^sub>s\<^sub>o\<^sub>n ((mk\<^sub>P\<^sub>e\<^sub>r\<^sub>s\<^sub>o\<^sub>n (oid1) (None) (None) (None))) (\<lfloor>1200\<rfloor>) (None))\<rfloor>\<rfloor>) , (\<lambda>_. \<lfloor>\<lfloor>(mkoid\<^sub>P\<^sub>e\<^sub>r\<^sub>s\<^sub>o\<^sub>n ((mk\<^sub>P\<^sub>e\<^sub>r\<^sub>s\<^sub>o\<^sub>n (oid3) (None) (None) (None))) (\<lfloor>2600\<rfloor>) (\<lfloor>oid4\<rfloor>))\<rfloor>\<rfloor>) , X\<^sub>P\<^sub>e\<^sub>r\<^sub>s\<^sub>o\<^sub>n5 , (\<lambda>_. \<lfloor>\<lfloor>(mkoid\<^sub>P\<^sub>e\<^sub>r\<^sub>s\<^sub>o\<^sub>n ((mk\<^sub>P\<^sub>e\<^sub>r\<^sub>s\<^sub>o\<^sub>n (oid5) (None) (None) (None))) (\<lfloor>2300\<rfloor>) (\<lfloor>oid3\<rfloor>))\<rfloor>\<rfloor>) , X\<^sub>P\<^sub>e\<^sub>r\<^sub>s\<^sub>o\<^sub>n9}"
+  unfolding OclAllInstances_at_pre_def
+by(rule \<sigma>\<^sub>1_OclAllInstances_generic_exec_Person, simp) 
+lemma \<sigma>\<^sub>1_OclAllInstances_generic_exec_Planet : 
+assumes [simp]: "(\<And>a. (pre_post ((mk (a)))) = a)"
+shows "(mk (\<sigma>\<^sub>1)) \<Turnstile> (OclAllInstances_generic (pre_post) (Planet)) \<doteq> Set{((\<lambda>_. \<lfloor>\<lfloor>(mkoid\<^sub>P\<^sub>e\<^sub>r\<^sub>s\<^sub>o\<^sub>n ((mk\<^sub>P\<^sub>e\<^sub>r\<^sub>s\<^sub>o\<^sub>n (oid0) (None) (None) (None))) (\<lfloor>1000\<rfloor>) (\<lfloor>oid1\<rfloor>))\<rfloor>\<rfloor>)::Person) .oclAsType(Planet) , ((\<lambda>_. \<lfloor>\<lfloor>(mkoid\<^sub>P\<^sub>e\<^sub>r\<^sub>s\<^sub>o\<^sub>n ((mk\<^sub>P\<^sub>e\<^sub>r\<^sub>s\<^sub>o\<^sub>n (oid1) (None) (None) (None))) (\<lfloor>1200\<rfloor>) (None))\<rfloor>\<rfloor>)::Person) .oclAsType(Planet) , ((\<lambda>_. \<lfloor>\<lfloor>(mkoid\<^sub>P\<^sub>e\<^sub>r\<^sub>s\<^sub>o\<^sub>n ((mk\<^sub>P\<^sub>e\<^sub>r\<^sub>s\<^sub>o\<^sub>n (oid3) (None) (None) (None))) (\<lfloor>2600\<rfloor>) (\<lfloor>oid4\<rfloor>))\<rfloor>\<rfloor>)::Person) .oclAsType(Planet) , X\<^sub>P\<^sub>e\<^sub>r\<^sub>s\<^sub>o\<^sub>n5 .oclAsType(Planet) , ((\<lambda>_. \<lfloor>\<lfloor>(mkoid\<^sub>P\<^sub>e\<^sub>r\<^sub>s\<^sub>o\<^sub>n ((mk\<^sub>P\<^sub>e\<^sub>r\<^sub>s\<^sub>o\<^sub>n (oid5) (None) (None) (None))) (\<lfloor>2300\<rfloor>) (\<lfloor>oid3\<rfloor>))\<rfloor>\<rfloor>)::Person) .oclAsType(Planet) , X\<^sub>P\<^sub>e\<^sub>r\<^sub>s\<^sub>o\<^sub>n9 .oclAsType(Planet)}"
+  apply(subst perm_\<sigma>\<^sub>1)
+  apply(simp only: state.make_def oid0_def oid1_def oid3_def oid4_def oid5_def oid8_def X\<^sub>P\<^sub>e\<^sub>r\<^sub>s\<^sub>o\<^sub>n5_def X\<^sub>P\<^sub>e\<^sub>r\<^sub>s\<^sub>o\<^sub>n9_def X\<^sub>P\<^sub>e\<^sub>r\<^sub>s\<^sub>o\<^sub>n5\<^sub>P\<^sub>e\<^sub>r\<^sub>s\<^sub>o\<^sub>n_def X\<^sub>P\<^sub>e\<^sub>r\<^sub>s\<^sub>o\<^sub>n9\<^sub>P\<^sub>e\<^sub>r\<^sub>s\<^sub>o\<^sub>n_def)
+  apply(subst state_update_vs_allInstances_generic_tc, simp, simp, simp add: OclAsType\<^sub>P\<^sub>l\<^sub>a\<^sub>n\<^sub>e\<^sub>t_\<AA>_def, simp, rule const_StrictRefEq\<^sub>S\<^sub>e\<^sub>t_including, simp, simp, simp, rule OclIncluding_cong, simp, simp)
+  apply(subst state_update_vs_allInstances_generic_tc, simp, simp, simp add: OclAsType\<^sub>P\<^sub>l\<^sub>a\<^sub>n\<^sub>e\<^sub>t_\<AA>_def, simp, rule const_StrictRefEq\<^sub>S\<^sub>e\<^sub>t_including, simp, simp, simp, rule OclIncluding_cong, simp, simp)
+  apply(subst state_update_vs_allInstances_generic_tc, simp, simp, simp add: OclAsType\<^sub>P\<^sub>l\<^sub>a\<^sub>n\<^sub>e\<^sub>t_\<AA>_def, simp, rule const_StrictRefEq\<^sub>S\<^sub>e\<^sub>t_including, simp, simp, simp, rule OclIncluding_cong, simp, simp)
+  apply(subst state_update_vs_allInstances_generic_tc, simp, simp, simp add: OclAsType\<^sub>P\<^sub>l\<^sub>a\<^sub>n\<^sub>e\<^sub>t_\<AA>_def, simp, rule const_StrictRefEq\<^sub>S\<^sub>e\<^sub>t_including, simp, simp, simp, rule OclIncluding_cong, simp, simp)
+  apply(subst state_update_vs_allInstances_generic_tc, simp, simp, simp add: OclAsType\<^sub>P\<^sub>l\<^sub>a\<^sub>n\<^sub>e\<^sub>t_\<AA>_def, simp, rule const_StrictRefEq\<^sub>S\<^sub>e\<^sub>t_including, simp, simp, simp, rule OclIncluding_cong, simp, simp)
+  apply(subst state_update_vs_allInstances_generic_tc, simp, simp, simp add: OclAsType\<^sub>P\<^sub>l\<^sub>a\<^sub>n\<^sub>e\<^sub>t_\<AA>_def, simp, rule const_StrictRefEq\<^sub>S\<^sub>e\<^sub>t_including, simp, simp, simp, rule OclIncluding_cong, simp, simp)
+  apply(rule state_update_vs_allInstances_generic_empty)
+by((simp add: OclAsType\<^sub>P\<^sub>l\<^sub>a\<^sub>n\<^sub>e\<^sub>t_\<AA>_def)+) 
+lemma \<sigma>\<^sub>1_OclAllInstances_at_post_exec_Planet : 
+shows "(st , \<sigma>\<^sub>1) \<Turnstile> (OclAllInstances_at_post (Planet)) \<doteq> Set{((\<lambda>_. \<lfloor>\<lfloor>(mkoid\<^sub>P\<^sub>e\<^sub>r\<^sub>s\<^sub>o\<^sub>n ((mk\<^sub>P\<^sub>e\<^sub>r\<^sub>s\<^sub>o\<^sub>n (oid0) (None) (None) (None))) (\<lfloor>1000\<rfloor>) (\<lfloor>oid1\<rfloor>))\<rfloor>\<rfloor>)::Person) .oclAsType(Planet) , ((\<lambda>_. \<lfloor>\<lfloor>(mkoid\<^sub>P\<^sub>e\<^sub>r\<^sub>s\<^sub>o\<^sub>n ((mk\<^sub>P\<^sub>e\<^sub>r\<^sub>s\<^sub>o\<^sub>n (oid1) (None) (None) (None))) (\<lfloor>1200\<rfloor>) (None))\<rfloor>\<rfloor>)::Person) .oclAsType(Planet) , ((\<lambda>_. \<lfloor>\<lfloor>(mkoid\<^sub>P\<^sub>e\<^sub>r\<^sub>s\<^sub>o\<^sub>n ((mk\<^sub>P\<^sub>e\<^sub>r\<^sub>s\<^sub>o\<^sub>n (oid3) (None) (None) (None))) (\<lfloor>2600\<rfloor>) (\<lfloor>oid4\<rfloor>))\<rfloor>\<rfloor>)::Person) .oclAsType(Planet) , X\<^sub>P\<^sub>e\<^sub>r\<^sub>s\<^sub>o\<^sub>n5 .oclAsType(Planet) , ((\<lambda>_. \<lfloor>\<lfloor>(mkoid\<^sub>P\<^sub>e\<^sub>r\<^sub>s\<^sub>o\<^sub>n ((mk\<^sub>P\<^sub>e\<^sub>r\<^sub>s\<^sub>o\<^sub>n (oid5) (None) (None) (None))) (\<lfloor>2300\<rfloor>) (\<lfloor>oid3\<rfloor>))\<rfloor>\<rfloor>)::Person) .oclAsType(Planet) , X\<^sub>P\<^sub>e\<^sub>r\<^sub>s\<^sub>o\<^sub>n9 .oclAsType(Planet)}"
+  unfolding OclAllInstances_at_post_def
+by(rule \<sigma>\<^sub>1_OclAllInstances_generic_exec_Planet, simp) 
+lemma \<sigma>\<^sub>1_OclAllInstances_at_pre_exec_Planet : 
+shows "(\<sigma>\<^sub>1 , st) \<Turnstile> (OclAllInstances_at_pre (Planet)) \<doteq> Set{((\<lambda>_. \<lfloor>\<lfloor>(mkoid\<^sub>P\<^sub>e\<^sub>r\<^sub>s\<^sub>o\<^sub>n ((mk\<^sub>P\<^sub>e\<^sub>r\<^sub>s\<^sub>o\<^sub>n (oid0) (None) (None) (None))) (\<lfloor>1000\<rfloor>) (\<lfloor>oid1\<rfloor>))\<rfloor>\<rfloor>)::Person) .oclAsType(Planet) , ((\<lambda>_. \<lfloor>\<lfloor>(mkoid\<^sub>P\<^sub>e\<^sub>r\<^sub>s\<^sub>o\<^sub>n ((mk\<^sub>P\<^sub>e\<^sub>r\<^sub>s\<^sub>o\<^sub>n (oid1) (None) (None) (None))) (\<lfloor>1200\<rfloor>) (None))\<rfloor>\<rfloor>)::Person) .oclAsType(Planet) , ((\<lambda>_. \<lfloor>\<lfloor>(mkoid\<^sub>P\<^sub>e\<^sub>r\<^sub>s\<^sub>o\<^sub>n ((mk\<^sub>P\<^sub>e\<^sub>r\<^sub>s\<^sub>o\<^sub>n (oid3) (None) (None) (None))) (\<lfloor>2600\<rfloor>) (\<lfloor>oid4\<rfloor>))\<rfloor>\<rfloor>)::Person) .oclAsType(Planet) , X\<^sub>P\<^sub>e\<^sub>r\<^sub>s\<^sub>o\<^sub>n5 .oclAsType(Planet) , ((\<lambda>_. \<lfloor>\<lfloor>(mkoid\<^sub>P\<^sub>e\<^sub>r\<^sub>s\<^sub>o\<^sub>n ((mk\<^sub>P\<^sub>e\<^sub>r\<^sub>s\<^sub>o\<^sub>n (oid5) (None) (None) (None))) (\<lfloor>2300\<rfloor>) (\<lfloor>oid3\<rfloor>))\<rfloor>\<rfloor>)::Person) .oclAsType(Planet) , X\<^sub>P\<^sub>e\<^sub>r\<^sub>s\<^sub>o\<^sub>n9 .oclAsType(Planet)}"
+  unfolding OclAllInstances_at_pre_def
+by(rule \<sigma>\<^sub>1_OclAllInstances_generic_exec_Planet, simp) 
+lemma \<sigma>\<^sub>1_OclAllInstances_generic_exec_Galaxy : 
+assumes [simp]: "(\<And>a. (pre_post ((mk (a)))) = a)"
+shows "(mk (\<sigma>\<^sub>1)) \<Turnstile> (OclAllInstances_generic (pre_post) (Galaxy)) \<doteq> Set{((\<lambda>_. \<lfloor>\<lfloor>(mkoid\<^sub>P\<^sub>e\<^sub>r\<^sub>s\<^sub>o\<^sub>n ((mk\<^sub>P\<^sub>e\<^sub>r\<^sub>s\<^sub>o\<^sub>n (oid0) (None) (None) (None))) (\<lfloor>1000\<rfloor>) (\<lfloor>oid1\<rfloor>))\<rfloor>\<rfloor>)::Person) .oclAsType(Galaxy) , ((\<lambda>_. \<lfloor>\<lfloor>(mkoid\<^sub>P\<^sub>e\<^sub>r\<^sub>s\<^sub>o\<^sub>n ((mk\<^sub>P\<^sub>e\<^sub>r\<^sub>s\<^sub>o\<^sub>n (oid1) (None) (None) (None))) (\<lfloor>1200\<rfloor>) (None))\<rfloor>\<rfloor>)::Person) .oclAsType(Galaxy) , ((\<lambda>_. \<lfloor>\<lfloor>(mkoid\<^sub>P\<^sub>e\<^sub>r\<^sub>s\<^sub>o\<^sub>n ((mk\<^sub>P\<^sub>e\<^sub>r\<^sub>s\<^sub>o\<^sub>n (oid3) (None) (None) (None))) (\<lfloor>2600\<rfloor>) (\<lfloor>oid4\<rfloor>))\<rfloor>\<rfloor>)::Person) .oclAsType(Galaxy) , X\<^sub>P\<^sub>e\<^sub>r\<^sub>s\<^sub>o\<^sub>n5 .oclAsType(Galaxy) , ((\<lambda>_. \<lfloor>\<lfloor>(mkoid\<^sub>P\<^sub>e\<^sub>r\<^sub>s\<^sub>o\<^sub>n ((mk\<^sub>P\<^sub>e\<^sub>r\<^sub>s\<^sub>o\<^sub>n (oid5) (None) (None) (None))) (\<lfloor>2300\<rfloor>) (\<lfloor>oid3\<rfloor>))\<rfloor>\<rfloor>)::Person) .oclAsType(Galaxy) , X\<^sub>P\<^sub>e\<^sub>r\<^sub>s\<^sub>o\<^sub>n9 .oclAsType(Galaxy)}"
+  apply(subst perm_\<sigma>\<^sub>1)
+  apply(simp only: state.make_def oid0_def oid1_def oid3_def oid4_def oid5_def oid8_def X\<^sub>P\<^sub>e\<^sub>r\<^sub>s\<^sub>o\<^sub>n5_def X\<^sub>P\<^sub>e\<^sub>r\<^sub>s\<^sub>o\<^sub>n9_def X\<^sub>P\<^sub>e\<^sub>r\<^sub>s\<^sub>o\<^sub>n5\<^sub>P\<^sub>e\<^sub>r\<^sub>s\<^sub>o\<^sub>n_def X\<^sub>P\<^sub>e\<^sub>r\<^sub>s\<^sub>o\<^sub>n9\<^sub>P\<^sub>e\<^sub>r\<^sub>s\<^sub>o\<^sub>n_def)
+  apply(subst state_update_vs_allInstances_generic_tc, simp, simp, simp add: OclAsType\<^sub>G\<^sub>a\<^sub>l\<^sub>a\<^sub>x\<^sub>y_\<AA>_def, simp, rule const_StrictRefEq\<^sub>S\<^sub>e\<^sub>t_including, simp, simp, simp, rule OclIncluding_cong, simp, simp)
+  apply(subst state_update_vs_allInstances_generic_tc, simp, simp, simp add: OclAsType\<^sub>G\<^sub>a\<^sub>l\<^sub>a\<^sub>x\<^sub>y_\<AA>_def, simp, rule const_StrictRefEq\<^sub>S\<^sub>e\<^sub>t_including, simp, simp, simp, rule OclIncluding_cong, simp, simp)
+  apply(subst state_update_vs_allInstances_generic_tc, simp, simp, simp add: OclAsType\<^sub>G\<^sub>a\<^sub>l\<^sub>a\<^sub>x\<^sub>y_\<AA>_def, simp, rule const_StrictRefEq\<^sub>S\<^sub>e\<^sub>t_including, simp, simp, simp, rule OclIncluding_cong, simp, simp)
+  apply(subst state_update_vs_allInstances_generic_tc, simp, simp, simp add: OclAsType\<^sub>G\<^sub>a\<^sub>l\<^sub>a\<^sub>x\<^sub>y_\<AA>_def, simp, rule const_StrictRefEq\<^sub>S\<^sub>e\<^sub>t_including, simp, simp, simp, rule OclIncluding_cong, simp, simp)
+  apply(subst state_update_vs_allInstances_generic_tc, simp, simp, simp add: OclAsType\<^sub>G\<^sub>a\<^sub>l\<^sub>a\<^sub>x\<^sub>y_\<AA>_def, simp, rule const_StrictRefEq\<^sub>S\<^sub>e\<^sub>t_including, simp, simp, simp, rule OclIncluding_cong, simp, simp)
+  apply(subst state_update_vs_allInstances_generic_tc, simp, simp, simp add: OclAsType\<^sub>G\<^sub>a\<^sub>l\<^sub>a\<^sub>x\<^sub>y_\<AA>_def, simp, rule const_StrictRefEq\<^sub>S\<^sub>e\<^sub>t_including, simp, simp, simp, rule OclIncluding_cong, simp, simp)
+  apply(rule state_update_vs_allInstances_generic_empty)
+by((simp add: OclAsType\<^sub>G\<^sub>a\<^sub>l\<^sub>a\<^sub>x\<^sub>y_\<AA>_def)+) 
+lemma \<sigma>\<^sub>1_OclAllInstances_at_post_exec_Galaxy : 
+shows "(st , \<sigma>\<^sub>1) \<Turnstile> (OclAllInstances_at_post (Galaxy)) \<doteq> Set{((\<lambda>_. \<lfloor>\<lfloor>(mkoid\<^sub>P\<^sub>e\<^sub>r\<^sub>s\<^sub>o\<^sub>n ((mk\<^sub>P\<^sub>e\<^sub>r\<^sub>s\<^sub>o\<^sub>n (oid0) (None) (None) (None))) (\<lfloor>1000\<rfloor>) (\<lfloor>oid1\<rfloor>))\<rfloor>\<rfloor>)::Person) .oclAsType(Galaxy) , ((\<lambda>_. \<lfloor>\<lfloor>(mkoid\<^sub>P\<^sub>e\<^sub>r\<^sub>s\<^sub>o\<^sub>n ((mk\<^sub>P\<^sub>e\<^sub>r\<^sub>s\<^sub>o\<^sub>n (oid1) (None) (None) (None))) (\<lfloor>1200\<rfloor>) (None))\<rfloor>\<rfloor>)::Person) .oclAsType(Galaxy) , ((\<lambda>_. \<lfloor>\<lfloor>(mkoid\<^sub>P\<^sub>e\<^sub>r\<^sub>s\<^sub>o\<^sub>n ((mk\<^sub>P\<^sub>e\<^sub>r\<^sub>s\<^sub>o\<^sub>n (oid3) (None) (None) (None))) (\<lfloor>2600\<rfloor>) (\<lfloor>oid4\<rfloor>))\<rfloor>\<rfloor>)::Person) .oclAsType(Galaxy) , X\<^sub>P\<^sub>e\<^sub>r\<^sub>s\<^sub>o\<^sub>n5 .oclAsType(Galaxy) , ((\<lambda>_. \<lfloor>\<lfloor>(mkoid\<^sub>P\<^sub>e\<^sub>r\<^sub>s\<^sub>o\<^sub>n ((mk\<^sub>P\<^sub>e\<^sub>r\<^sub>s\<^sub>o\<^sub>n (oid5) (None) (None) (None))) (\<lfloor>2300\<rfloor>) (\<lfloor>oid3\<rfloor>))\<rfloor>\<rfloor>)::Person) .oclAsType(Galaxy) , X\<^sub>P\<^sub>e\<^sub>r\<^sub>s\<^sub>o\<^sub>n9 .oclAsType(Galaxy)}"
+  unfolding OclAllInstances_at_post_def
+by(rule \<sigma>\<^sub>1_OclAllInstances_generic_exec_Galaxy, simp) 
+lemma \<sigma>\<^sub>1_OclAllInstances_at_pre_exec_Galaxy : 
+shows "(\<sigma>\<^sub>1 , st) \<Turnstile> (OclAllInstances_at_pre (Galaxy)) \<doteq> Set{((\<lambda>_. \<lfloor>\<lfloor>(mkoid\<^sub>P\<^sub>e\<^sub>r\<^sub>s\<^sub>o\<^sub>n ((mk\<^sub>P\<^sub>e\<^sub>r\<^sub>s\<^sub>o\<^sub>n (oid0) (None) (None) (None))) (\<lfloor>1000\<rfloor>) (\<lfloor>oid1\<rfloor>))\<rfloor>\<rfloor>)::Person) .oclAsType(Galaxy) , ((\<lambda>_. \<lfloor>\<lfloor>(mkoid\<^sub>P\<^sub>e\<^sub>r\<^sub>s\<^sub>o\<^sub>n ((mk\<^sub>P\<^sub>e\<^sub>r\<^sub>s\<^sub>o\<^sub>n (oid1) (None) (None) (None))) (\<lfloor>1200\<rfloor>) (None))\<rfloor>\<rfloor>)::Person) .oclAsType(Galaxy) , ((\<lambda>_. \<lfloor>\<lfloor>(mkoid\<^sub>P\<^sub>e\<^sub>r\<^sub>s\<^sub>o\<^sub>n ((mk\<^sub>P\<^sub>e\<^sub>r\<^sub>s\<^sub>o\<^sub>n (oid3) (None) (None) (None))) (\<lfloor>2600\<rfloor>) (\<lfloor>oid4\<rfloor>))\<rfloor>\<rfloor>)::Person) .oclAsType(Galaxy) , X\<^sub>P\<^sub>e\<^sub>r\<^sub>s\<^sub>o\<^sub>n5 .oclAsType(Galaxy) , ((\<lambda>_. \<lfloor>\<lfloor>(mkoid\<^sub>P\<^sub>e\<^sub>r\<^sub>s\<^sub>o\<^sub>n ((mk\<^sub>P\<^sub>e\<^sub>r\<^sub>s\<^sub>o\<^sub>n (oid5) (None) (None) (None))) (\<lfloor>2300\<rfloor>) (\<lfloor>oid3\<rfloor>))\<rfloor>\<rfloor>)::Person) .oclAsType(Galaxy) , X\<^sub>P\<^sub>e\<^sub>r\<^sub>s\<^sub>o\<^sub>n9 .oclAsType(Galaxy)}"
+  unfolding OclAllInstances_at_pre_def
+by(rule \<sigma>\<^sub>1_OclAllInstances_generic_exec_Galaxy, simp) 
+lemma \<sigma>\<^sub>1_OclAllInstances_generic_exec_OclAny : 
+assumes [simp]: "(\<And>a. (pre_post ((mk (a)))) = a)"
+shows "(mk (\<sigma>\<^sub>1)) \<Turnstile> (OclAllInstances_generic (pre_post) (OclAny)) \<doteq> Set{((\<lambda>_. \<lfloor>\<lfloor>(mkoid\<^sub>P\<^sub>e\<^sub>r\<^sub>s\<^sub>o\<^sub>n ((mk\<^sub>P\<^sub>e\<^sub>r\<^sub>s\<^sub>o\<^sub>n (oid0) (None) (None) (None))) (\<lfloor>1000\<rfloor>) (\<lfloor>oid1\<rfloor>))\<rfloor>\<rfloor>)::Person) .oclAsType(OclAny) , ((\<lambda>_. \<lfloor>\<lfloor>(mkoid\<^sub>P\<^sub>e\<^sub>r\<^sub>s\<^sub>o\<^sub>n ((mk\<^sub>P\<^sub>e\<^sub>r\<^sub>s\<^sub>o\<^sub>n (oid1) (None) (None) (None))) (\<lfloor>1200\<rfloor>) (None))\<rfloor>\<rfloor>)::Person) .oclAsType(OclAny) , ((\<lambda>_. \<lfloor>\<lfloor>(mkoid\<^sub>P\<^sub>e\<^sub>r\<^sub>s\<^sub>o\<^sub>n ((mk\<^sub>P\<^sub>e\<^sub>r\<^sub>s\<^sub>o\<^sub>n (oid3) (None) (None) (None))) (\<lfloor>2600\<rfloor>) (\<lfloor>oid4\<rfloor>))\<rfloor>\<rfloor>)::Person) .oclAsType(OclAny) , X\<^sub>P\<^sub>e\<^sub>r\<^sub>s\<^sub>o\<^sub>n5 .oclAsType(OclAny) , ((\<lambda>_. \<lfloor>\<lfloor>(mkoid\<^sub>P\<^sub>e\<^sub>r\<^sub>s\<^sub>o\<^sub>n ((mk\<^sub>P\<^sub>e\<^sub>r\<^sub>s\<^sub>o\<^sub>n (oid5) (None) (None) (None))) (\<lfloor>2300\<rfloor>) (\<lfloor>oid3\<rfloor>))\<rfloor>\<rfloor>)::Person) .oclAsType(OclAny) , X\<^sub>P\<^sub>e\<^sub>r\<^sub>s\<^sub>o\<^sub>n9 .oclAsType(OclAny)}"
+  apply(subst perm_\<sigma>\<^sub>1)
+  apply(simp only: state.make_def oid0_def oid1_def oid3_def oid4_def oid5_def oid8_def X\<^sub>P\<^sub>e\<^sub>r\<^sub>s\<^sub>o\<^sub>n5_def X\<^sub>P\<^sub>e\<^sub>r\<^sub>s\<^sub>o\<^sub>n9_def X\<^sub>P\<^sub>e\<^sub>r\<^sub>s\<^sub>o\<^sub>n5\<^sub>P\<^sub>e\<^sub>r\<^sub>s\<^sub>o\<^sub>n_def X\<^sub>P\<^sub>e\<^sub>r\<^sub>s\<^sub>o\<^sub>n9\<^sub>P\<^sub>e\<^sub>r\<^sub>s\<^sub>o\<^sub>n_def)
+  apply(subst state_update_vs_allInstances_generic_tc, simp, simp, simp add: OclAsType\<^sub>O\<^sub>c\<^sub>l\<^sub>A\<^sub>n\<^sub>y_\<AA>_def, simp, rule const_StrictRefEq\<^sub>S\<^sub>e\<^sub>t_including, simp, simp, simp, rule OclIncluding_cong, simp, simp)
+  apply(subst state_update_vs_allInstances_generic_tc, simp, simp, simp add: OclAsType\<^sub>O\<^sub>c\<^sub>l\<^sub>A\<^sub>n\<^sub>y_\<AA>_def, simp, rule const_StrictRefEq\<^sub>S\<^sub>e\<^sub>t_including, simp, simp, simp, rule OclIncluding_cong, simp, simp)
+  apply(subst state_update_vs_allInstances_generic_tc, simp, simp, simp add: OclAsType\<^sub>O\<^sub>c\<^sub>l\<^sub>A\<^sub>n\<^sub>y_\<AA>_def, simp, rule const_StrictRefEq\<^sub>S\<^sub>e\<^sub>t_including, simp, simp, simp, rule OclIncluding_cong, simp, simp)
+  apply(subst state_update_vs_allInstances_generic_tc, simp, simp, simp add: OclAsType\<^sub>O\<^sub>c\<^sub>l\<^sub>A\<^sub>n\<^sub>y_\<AA>_def, simp, rule const_StrictRefEq\<^sub>S\<^sub>e\<^sub>t_including, simp, simp, simp, rule OclIncluding_cong, simp, simp)
+  apply(subst state_update_vs_allInstances_generic_tc, simp, simp, simp add: OclAsType\<^sub>O\<^sub>c\<^sub>l\<^sub>A\<^sub>n\<^sub>y_\<AA>_def, simp, rule const_StrictRefEq\<^sub>S\<^sub>e\<^sub>t_including, simp, simp, simp, rule OclIncluding_cong, simp, simp)
+  apply(subst state_update_vs_allInstances_generic_tc, simp, simp, simp add: OclAsType\<^sub>O\<^sub>c\<^sub>l\<^sub>A\<^sub>n\<^sub>y_\<AA>_def, simp, rule const_StrictRefEq\<^sub>S\<^sub>e\<^sub>t_including, simp, simp, simp, rule OclIncluding_cong, simp, simp)
+  apply(rule state_update_vs_allInstances_generic_empty)
+by((simp add: OclAsType\<^sub>O\<^sub>c\<^sub>l\<^sub>A\<^sub>n\<^sub>y_\<AA>_def)+) 
+lemma \<sigma>\<^sub>1_OclAllInstances_at_post_exec_OclAny : 
+shows "(st , \<sigma>\<^sub>1) \<Turnstile> (OclAllInstances_at_post (OclAny)) \<doteq> Set{((\<lambda>_. \<lfloor>\<lfloor>(mkoid\<^sub>P\<^sub>e\<^sub>r\<^sub>s\<^sub>o\<^sub>n ((mk\<^sub>P\<^sub>e\<^sub>r\<^sub>s\<^sub>o\<^sub>n (oid0) (None) (None) (None))) (\<lfloor>1000\<rfloor>) (\<lfloor>oid1\<rfloor>))\<rfloor>\<rfloor>)::Person) .oclAsType(OclAny) , ((\<lambda>_. \<lfloor>\<lfloor>(mkoid\<^sub>P\<^sub>e\<^sub>r\<^sub>s\<^sub>o\<^sub>n ((mk\<^sub>P\<^sub>e\<^sub>r\<^sub>s\<^sub>o\<^sub>n (oid1) (None) (None) (None))) (\<lfloor>1200\<rfloor>) (None))\<rfloor>\<rfloor>)::Person) .oclAsType(OclAny) , ((\<lambda>_. \<lfloor>\<lfloor>(mkoid\<^sub>P\<^sub>e\<^sub>r\<^sub>s\<^sub>o\<^sub>n ((mk\<^sub>P\<^sub>e\<^sub>r\<^sub>s\<^sub>o\<^sub>n (oid3) (None) (None) (None))) (\<lfloor>2600\<rfloor>) (\<lfloor>oid4\<rfloor>))\<rfloor>\<rfloor>)::Person) .oclAsType(OclAny) , X\<^sub>P\<^sub>e\<^sub>r\<^sub>s\<^sub>o\<^sub>n5 .oclAsType(OclAny) , ((\<lambda>_. \<lfloor>\<lfloor>(mkoid\<^sub>P\<^sub>e\<^sub>r\<^sub>s\<^sub>o\<^sub>n ((mk\<^sub>P\<^sub>e\<^sub>r\<^sub>s\<^sub>o\<^sub>n (oid5) (None) (None) (None))) (\<lfloor>2300\<rfloor>) (\<lfloor>oid3\<rfloor>))\<rfloor>\<rfloor>)::Person) .oclAsType(OclAny) , X\<^sub>P\<^sub>e\<^sub>r\<^sub>s\<^sub>o\<^sub>n9 .oclAsType(OclAny)}"
+  unfolding OclAllInstances_at_post_def
+by(rule \<sigma>\<^sub>1_OclAllInstances_generic_exec_OclAny, simp) 
+lemma \<sigma>\<^sub>1_OclAllInstances_at_pre_exec_OclAny : 
+shows "(\<sigma>\<^sub>1 , st) \<Turnstile> (OclAllInstances_at_pre (OclAny)) \<doteq> Set{((\<lambda>_. \<lfloor>\<lfloor>(mkoid\<^sub>P\<^sub>e\<^sub>r\<^sub>s\<^sub>o\<^sub>n ((mk\<^sub>P\<^sub>e\<^sub>r\<^sub>s\<^sub>o\<^sub>n (oid0) (None) (None) (None))) (\<lfloor>1000\<rfloor>) (\<lfloor>oid1\<rfloor>))\<rfloor>\<rfloor>)::Person) .oclAsType(OclAny) , ((\<lambda>_. \<lfloor>\<lfloor>(mkoid\<^sub>P\<^sub>e\<^sub>r\<^sub>s\<^sub>o\<^sub>n ((mk\<^sub>P\<^sub>e\<^sub>r\<^sub>s\<^sub>o\<^sub>n (oid1) (None) (None) (None))) (\<lfloor>1200\<rfloor>) (None))\<rfloor>\<rfloor>)::Person) .oclAsType(OclAny) , ((\<lambda>_. \<lfloor>\<lfloor>(mkoid\<^sub>P\<^sub>e\<^sub>r\<^sub>s\<^sub>o\<^sub>n ((mk\<^sub>P\<^sub>e\<^sub>r\<^sub>s\<^sub>o\<^sub>n (oid3) (None) (None) (None))) (\<lfloor>2600\<rfloor>) (\<lfloor>oid4\<rfloor>))\<rfloor>\<rfloor>)::Person) .oclAsType(OclAny) , X\<^sub>P\<^sub>e\<^sub>r\<^sub>s\<^sub>o\<^sub>n5 .oclAsType(OclAny) , ((\<lambda>_. \<lfloor>\<lfloor>(mkoid\<^sub>P\<^sub>e\<^sub>r\<^sub>s\<^sub>o\<^sub>n ((mk\<^sub>P\<^sub>e\<^sub>r\<^sub>s\<^sub>o\<^sub>n (oid5) (None) (None) (None))) (\<lfloor>2300\<rfloor>) (\<lfloor>oid3\<rfloor>))\<rfloor>\<rfloor>)::Person) .oclAsType(OclAny) , X\<^sub>P\<^sub>e\<^sub>r\<^sub>s\<^sub>o\<^sub>n9 .oclAsType(OclAny)}"
+  unfolding OclAllInstances_at_pre_def
+by(rule \<sigma>\<^sub>1_OclAllInstances_generic_exec_OclAny, simp) 
+
+(* 133 ************************************ 799 + 1 *)
 definition "\<sigma>\<^sub>1' = (state.make ((Map.empty (oid0 \<mapsto> (in\<^sub>P\<^sub>e\<^sub>r\<^sub>s\<^sub>o\<^sub>n (X\<^sub>P\<^sub>e\<^sub>r\<^sub>s\<^sub>o\<^sub>n1\<^sub>P\<^sub>e\<^sub>r\<^sub>s\<^sub>o\<^sub>n))) (oid1 \<mapsto> (in\<^sub>P\<^sub>e\<^sub>r\<^sub>s\<^sub>o\<^sub>n (X\<^sub>P\<^sub>e\<^sub>r\<^sub>s\<^sub>o\<^sub>n2\<^sub>P\<^sub>e\<^sub>r\<^sub>s\<^sub>o\<^sub>n))) (oid2 \<mapsto> (in\<^sub>P\<^sub>e\<^sub>r\<^sub>s\<^sub>o\<^sub>n (X\<^sub>P\<^sub>e\<^sub>r\<^sub>s\<^sub>o\<^sub>n3\<^sub>P\<^sub>e\<^sub>r\<^sub>s\<^sub>o\<^sub>n))) (oid3 \<mapsto> (in\<^sub>P\<^sub>e\<^sub>r\<^sub>s\<^sub>o\<^sub>n (X\<^sub>P\<^sub>e\<^sub>r\<^sub>s\<^sub>o\<^sub>n4\<^sub>P\<^sub>e\<^sub>r\<^sub>s\<^sub>o\<^sub>n))) (oid5 \<mapsto> (in\<^sub>P\<^sub>e\<^sub>r\<^sub>s\<^sub>o\<^sub>n (X\<^sub>P\<^sub>e\<^sub>r\<^sub>s\<^sub>o\<^sub>n6\<^sub>P\<^sub>e\<^sub>r\<^sub>s\<^sub>o\<^sub>n))) (oid6 \<mapsto> (in\<^sub>O\<^sub>c\<^sub>l\<^sub>A\<^sub>n\<^sub>y (X\<^sub>P\<^sub>e\<^sub>r\<^sub>s\<^sub>o\<^sub>n7\<^sub>O\<^sub>c\<^sub>l\<^sub>A\<^sub>n\<^sub>y))) (oid7 \<mapsto> (in\<^sub>O\<^sub>c\<^sub>l\<^sub>A\<^sub>n\<^sub>y (X\<^sub>P\<^sub>e\<^sub>r\<^sub>s\<^sub>o\<^sub>n8\<^sub>O\<^sub>c\<^sub>l\<^sub>A\<^sub>n\<^sub>y))) (oid8 \<mapsto> (in\<^sub>P\<^sub>e\<^sub>r\<^sub>s\<^sub>o\<^sub>n (X\<^sub>P\<^sub>e\<^sub>r\<^sub>s\<^sub>o\<^sub>n9\<^sub>P\<^sub>e\<^sub>r\<^sub>s\<^sub>o\<^sub>n))))) (Map.empty) (Map.empty))"
 
-(* 123 ************************************ 727 + 1 *)
+(* 134 ************************************ 800 + 1 *)
+lemma dom_\<sigma>\<^sub>1' : "(dom ((heap (\<sigma>\<^sub>1')))) = {oid0 , oid1 , oid2 , oid3 , oid5 , oid6 , oid7 , oid8}"
+by(auto simp: \<sigma>\<^sub>1'_def)
+
+(* 135 ************************************ 801 + 1 *)
+lemmas [simp,code_unfold] = dom_\<sigma>\<^sub>1'
+
+(* 136 ************************************ 802 + 1 *)
+lemma perm_\<sigma>\<^sub>1' : "\<sigma>\<^sub>1' = (state.make ((Map.empty (oid8 \<mapsto> (in\<^sub>P\<^sub>e\<^sub>r\<^sub>s\<^sub>o\<^sub>n (X\<^sub>P\<^sub>e\<^sub>r\<^sub>s\<^sub>o\<^sub>n9\<^sub>P\<^sub>e\<^sub>r\<^sub>s\<^sub>o\<^sub>n))) (oid7 \<mapsto> (in\<^sub>O\<^sub>c\<^sub>l\<^sub>A\<^sub>n\<^sub>y (X\<^sub>P\<^sub>e\<^sub>r\<^sub>s\<^sub>o\<^sub>n8\<^sub>O\<^sub>c\<^sub>l\<^sub>A\<^sub>n\<^sub>y))) (oid6 \<mapsto> (in\<^sub>O\<^sub>c\<^sub>l\<^sub>A\<^sub>n\<^sub>y (X\<^sub>P\<^sub>e\<^sub>r\<^sub>s\<^sub>o\<^sub>n7\<^sub>O\<^sub>c\<^sub>l\<^sub>A\<^sub>n\<^sub>y))) (oid5 \<mapsto> (in\<^sub>P\<^sub>e\<^sub>r\<^sub>s\<^sub>o\<^sub>n (X\<^sub>P\<^sub>e\<^sub>r\<^sub>s\<^sub>o\<^sub>n6\<^sub>P\<^sub>e\<^sub>r\<^sub>s\<^sub>o\<^sub>n))) (oid3 \<mapsto> (in\<^sub>P\<^sub>e\<^sub>r\<^sub>s\<^sub>o\<^sub>n (X\<^sub>P\<^sub>e\<^sub>r\<^sub>s\<^sub>o\<^sub>n4\<^sub>P\<^sub>e\<^sub>r\<^sub>s\<^sub>o\<^sub>n))) (oid2 \<mapsto> (in\<^sub>P\<^sub>e\<^sub>r\<^sub>s\<^sub>o\<^sub>n (X\<^sub>P\<^sub>e\<^sub>r\<^sub>s\<^sub>o\<^sub>n3\<^sub>P\<^sub>e\<^sub>r\<^sub>s\<^sub>o\<^sub>n))) (oid1 \<mapsto> (in\<^sub>P\<^sub>e\<^sub>r\<^sub>s\<^sub>o\<^sub>n (X\<^sub>P\<^sub>e\<^sub>r\<^sub>s\<^sub>o\<^sub>n2\<^sub>P\<^sub>e\<^sub>r\<^sub>s\<^sub>o\<^sub>n))) (oid0 \<mapsto> (in\<^sub>P\<^sub>e\<^sub>r\<^sub>s\<^sub>o\<^sub>n (X\<^sub>P\<^sub>e\<^sub>r\<^sub>s\<^sub>o\<^sub>n1\<^sub>P\<^sub>e\<^sub>r\<^sub>s\<^sub>o\<^sub>n))))) ((assocs\<^sub>2 (\<sigma>\<^sub>1'))) ((assocs\<^sub>3 (\<sigma>\<^sub>1'))))"
+  apply(simp add: \<sigma>\<^sub>1'_def oid0_def oid1_def oid2_def oid3_def oid5_def oid6_def oid7_def oid8_def)
+  apply(subst (1) fun_upd_twist, simp)
+  apply(subst (2) fun_upd_twist, simp)
+  apply(subst (1) fun_upd_twist, simp)
+  apply(subst (3) fun_upd_twist, simp)
+  apply(subst (2) fun_upd_twist, simp)
+  apply(subst (1) fun_upd_twist, simp)
+  apply(subst (4) fun_upd_twist, simp)
+  apply(subst (3) fun_upd_twist, simp)
+  apply(subst (2) fun_upd_twist, simp)
+  apply(subst (1) fun_upd_twist, simp)
+  apply(subst (5) fun_upd_twist, simp)
+  apply(subst (4) fun_upd_twist, simp)
+  apply(subst (3) fun_upd_twist, simp)
+  apply(subst (2) fun_upd_twist, simp)
+  apply(subst (1) fun_upd_twist, simp)
+  apply(subst (6) fun_upd_twist, simp)
+  apply(subst (5) fun_upd_twist, simp)
+  apply(subst (4) fun_upd_twist, simp)
+  apply(subst (3) fun_upd_twist, simp)
+  apply(subst (2) fun_upd_twist, simp)
+  apply(subst (1) fun_upd_twist, simp)
+  apply(subst (7) fun_upd_twist, simp)
+  apply(subst (6) fun_upd_twist, simp)
+  apply(subst (5) fun_upd_twist, simp)
+  apply(subst (4) fun_upd_twist, simp)
+  apply(subst (3) fun_upd_twist, simp)
+  apply(subst (2) fun_upd_twist, simp)
+  apply(subst (1) fun_upd_twist, simp)
+by(simp)
+
+(* 137 ************************************ 803 + 12 *)
+lemma \<sigma>\<^sub>1'_OclAllInstances_generic_exec_Person : 
+assumes [simp]: "(\<And>a. (pre_post ((mk (a)))) = a)"
+shows "(mk (\<sigma>\<^sub>1')) \<Turnstile> (OclAllInstances_generic (pre_post) (Person)) \<doteq> Set{X\<^sub>P\<^sub>e\<^sub>r\<^sub>s\<^sub>o\<^sub>n1 , X\<^sub>P\<^sub>e\<^sub>r\<^sub>s\<^sub>o\<^sub>n2 , X\<^sub>P\<^sub>e\<^sub>r\<^sub>s\<^sub>o\<^sub>n3 , X\<^sub>P\<^sub>e\<^sub>r\<^sub>s\<^sub>o\<^sub>n4 , X\<^sub>P\<^sub>e\<^sub>r\<^sub>s\<^sub>o\<^sub>n6 , X\<^sub>P\<^sub>e\<^sub>r\<^sub>s\<^sub>o\<^sub>n7 .oclAsType(Person) , X\<^sub>P\<^sub>e\<^sub>r\<^sub>s\<^sub>o\<^sub>n9}"
+  apply(subst perm_\<sigma>\<^sub>1')
+  apply(simp only: state.make_def oid0_def oid1_def oid2_def oid3_def oid5_def oid6_def oid7_def oid8_def X\<^sub>P\<^sub>e\<^sub>r\<^sub>s\<^sub>o\<^sub>n1_def X\<^sub>P\<^sub>e\<^sub>r\<^sub>s\<^sub>o\<^sub>n2_def X\<^sub>P\<^sub>e\<^sub>r\<^sub>s\<^sub>o\<^sub>n3_def X\<^sub>P\<^sub>e\<^sub>r\<^sub>s\<^sub>o\<^sub>n4_def X\<^sub>P\<^sub>e\<^sub>r\<^sub>s\<^sub>o\<^sub>n6_def X\<^sub>P\<^sub>e\<^sub>r\<^sub>s\<^sub>o\<^sub>n7_def X\<^sub>P\<^sub>e\<^sub>r\<^sub>s\<^sub>o\<^sub>n9_def X\<^sub>P\<^sub>e\<^sub>r\<^sub>s\<^sub>o\<^sub>n7\<^sub>O\<^sub>c\<^sub>l\<^sub>A\<^sub>n\<^sub>y_def)
+  apply(subst state_update_vs_allInstances_generic_tc, simp, simp, simp add: OclAsType\<^sub>P\<^sub>e\<^sub>r\<^sub>s\<^sub>o\<^sub>n_\<AA>_def, simp, rule const_StrictRefEq\<^sub>S\<^sub>e\<^sub>t_including, simp, simp, simp, rule OclIncluding_cong, simp, simp)
+  apply(subst state_update_vs_allInstances_generic_tc, simp, simp, simp add: OclAsType\<^sub>P\<^sub>e\<^sub>r\<^sub>s\<^sub>o\<^sub>n_\<AA>_def, simp, rule const_StrictRefEq\<^sub>S\<^sub>e\<^sub>t_including, simp, simp, simp, rule OclIncluding_cong, simp, simp)
+  apply(subst state_update_vs_allInstances_generic_tc, simp, simp, simp add: OclAsType\<^sub>P\<^sub>e\<^sub>r\<^sub>s\<^sub>o\<^sub>n_\<AA>_def, simp, rule const_StrictRefEq\<^sub>S\<^sub>e\<^sub>t_including, simp, simp, simp, rule OclIncluding_cong, simp, simp)
+  apply(subst state_update_vs_allInstances_generic_tc, simp, simp, simp add: OclAsType\<^sub>P\<^sub>e\<^sub>r\<^sub>s\<^sub>o\<^sub>n_\<AA>_def, simp, rule const_StrictRefEq\<^sub>S\<^sub>e\<^sub>t_including, simp, simp, simp, rule OclIncluding_cong, simp, simp)
+  apply(subst state_update_vs_allInstances_generic_tc, simp, simp, simp add: OclAsType\<^sub>P\<^sub>e\<^sub>r\<^sub>s\<^sub>o\<^sub>n_\<AA>_def, simp, rule const_StrictRefEq\<^sub>S\<^sub>e\<^sub>t_including, simp, simp, simp, rule OclIncluding_cong, simp, simp)
+  apply(subst state_update_vs_allInstances_generic_tc, simp, simp, simp add: OclAsType\<^sub>P\<^sub>e\<^sub>r\<^sub>s\<^sub>o\<^sub>n_\<AA>_def, simp, rule const_StrictRefEq\<^sub>S\<^sub>e\<^sub>t_including, simp, simp, simp, rule OclIncluding_cong, simp, simp)
+  apply(subst state_update_vs_allInstances_generic_ntc, simp, simp, simp add: OclAsType\<^sub>P\<^sub>e\<^sub>r\<^sub>s\<^sub>o\<^sub>n_\<AA>_def X\<^sub>P\<^sub>e\<^sub>r\<^sub>s\<^sub>o\<^sub>n8\<^sub>O\<^sub>c\<^sub>l\<^sub>A\<^sub>n\<^sub>y_def, simp, rule const_StrictRefEq\<^sub>S\<^sub>e\<^sub>t_including, simp, simp, simp)
+  apply(subst state_update_vs_allInstances_generic_tc, simp, simp, simp add: OclAsType\<^sub>P\<^sub>e\<^sub>r\<^sub>s\<^sub>o\<^sub>n_\<AA>_def, simp, rule const_StrictRefEq\<^sub>S\<^sub>e\<^sub>t_including, simp, simp, simp, rule OclIncluding_cong, simp, simp)
+  apply(rule state_update_vs_allInstances_generic_empty)
+by((simp add: OclAsType\<^sub>P\<^sub>e\<^sub>r\<^sub>s\<^sub>o\<^sub>n_\<AA>_def)+) 
+lemma \<sigma>\<^sub>1'_OclAllInstances_at_post_exec_Person : 
+shows "(st , \<sigma>\<^sub>1') \<Turnstile> (OclAllInstances_at_post (Person)) \<doteq> Set{X\<^sub>P\<^sub>e\<^sub>r\<^sub>s\<^sub>o\<^sub>n1 , X\<^sub>P\<^sub>e\<^sub>r\<^sub>s\<^sub>o\<^sub>n2 , X\<^sub>P\<^sub>e\<^sub>r\<^sub>s\<^sub>o\<^sub>n3 , X\<^sub>P\<^sub>e\<^sub>r\<^sub>s\<^sub>o\<^sub>n4 , X\<^sub>P\<^sub>e\<^sub>r\<^sub>s\<^sub>o\<^sub>n6 , X\<^sub>P\<^sub>e\<^sub>r\<^sub>s\<^sub>o\<^sub>n7 .oclAsType(Person) , X\<^sub>P\<^sub>e\<^sub>r\<^sub>s\<^sub>o\<^sub>n9}"
+  unfolding OclAllInstances_at_post_def
+by(rule \<sigma>\<^sub>1'_OclAllInstances_generic_exec_Person, simp) 
+lemma \<sigma>\<^sub>1'_OclAllInstances_at_pre_exec_Person : 
+shows "(\<sigma>\<^sub>1' , st) \<Turnstile> (OclAllInstances_at_pre (Person)) \<doteq> Set{X\<^sub>P\<^sub>e\<^sub>r\<^sub>s\<^sub>o\<^sub>n1 , X\<^sub>P\<^sub>e\<^sub>r\<^sub>s\<^sub>o\<^sub>n2 , X\<^sub>P\<^sub>e\<^sub>r\<^sub>s\<^sub>o\<^sub>n3 , X\<^sub>P\<^sub>e\<^sub>r\<^sub>s\<^sub>o\<^sub>n4 , X\<^sub>P\<^sub>e\<^sub>r\<^sub>s\<^sub>o\<^sub>n6 , X\<^sub>P\<^sub>e\<^sub>r\<^sub>s\<^sub>o\<^sub>n7 .oclAsType(Person) , X\<^sub>P\<^sub>e\<^sub>r\<^sub>s\<^sub>o\<^sub>n9}"
+  unfolding OclAllInstances_at_pre_def
+by(rule \<sigma>\<^sub>1'_OclAllInstances_generic_exec_Person, simp) 
+lemma \<sigma>\<^sub>1'_OclAllInstances_generic_exec_Planet : 
+assumes [simp]: "(\<And>a. (pre_post ((mk (a)))) = a)"
+shows "(mk (\<sigma>\<^sub>1')) \<Turnstile> (OclAllInstances_generic (pre_post) (Planet)) \<doteq> Set{X\<^sub>P\<^sub>e\<^sub>r\<^sub>s\<^sub>o\<^sub>n1 .oclAsType(Planet) , X\<^sub>P\<^sub>e\<^sub>r\<^sub>s\<^sub>o\<^sub>n2 .oclAsType(Planet) , X\<^sub>P\<^sub>e\<^sub>r\<^sub>s\<^sub>o\<^sub>n3 .oclAsType(Planet) , X\<^sub>P\<^sub>e\<^sub>r\<^sub>s\<^sub>o\<^sub>n4 .oclAsType(Planet) , X\<^sub>P\<^sub>e\<^sub>r\<^sub>s\<^sub>o\<^sub>n6 .oclAsType(Planet) , X\<^sub>P\<^sub>e\<^sub>r\<^sub>s\<^sub>o\<^sub>n9 .oclAsType(Planet)}"
+  apply(subst perm_\<sigma>\<^sub>1')
+  apply(simp only: state.make_def oid0_def oid1_def oid2_def oid3_def oid5_def oid6_def oid7_def oid8_def X\<^sub>P\<^sub>e\<^sub>r\<^sub>s\<^sub>o\<^sub>n1_def X\<^sub>P\<^sub>e\<^sub>r\<^sub>s\<^sub>o\<^sub>n2_def X\<^sub>P\<^sub>e\<^sub>r\<^sub>s\<^sub>o\<^sub>n3_def X\<^sub>P\<^sub>e\<^sub>r\<^sub>s\<^sub>o\<^sub>n4_def X\<^sub>P\<^sub>e\<^sub>r\<^sub>s\<^sub>o\<^sub>n6_def X\<^sub>P\<^sub>e\<^sub>r\<^sub>s\<^sub>o\<^sub>n9_def X\<^sub>P\<^sub>e\<^sub>r\<^sub>s\<^sub>o\<^sub>n1\<^sub>P\<^sub>e\<^sub>r\<^sub>s\<^sub>o\<^sub>n_def X\<^sub>P\<^sub>e\<^sub>r\<^sub>s\<^sub>o\<^sub>n2\<^sub>P\<^sub>e\<^sub>r\<^sub>s\<^sub>o\<^sub>n_def X\<^sub>P\<^sub>e\<^sub>r\<^sub>s\<^sub>o\<^sub>n3\<^sub>P\<^sub>e\<^sub>r\<^sub>s\<^sub>o\<^sub>n_def X\<^sub>P\<^sub>e\<^sub>r\<^sub>s\<^sub>o\<^sub>n4\<^sub>P\<^sub>e\<^sub>r\<^sub>s\<^sub>o\<^sub>n_def X\<^sub>P\<^sub>e\<^sub>r\<^sub>s\<^sub>o\<^sub>n6\<^sub>P\<^sub>e\<^sub>r\<^sub>s\<^sub>o\<^sub>n_def X\<^sub>P\<^sub>e\<^sub>r\<^sub>s\<^sub>o\<^sub>n9\<^sub>P\<^sub>e\<^sub>r\<^sub>s\<^sub>o\<^sub>n_def)
+  apply(subst state_update_vs_allInstances_generic_tc, simp, simp, simp add: OclAsType\<^sub>P\<^sub>l\<^sub>a\<^sub>n\<^sub>e\<^sub>t_\<AA>_def, simp, rule const_StrictRefEq\<^sub>S\<^sub>e\<^sub>t_including, simp, simp, simp, rule OclIncluding_cong, simp, simp)
+  apply(subst state_update_vs_allInstances_generic_tc, simp, simp, simp add: OclAsType\<^sub>P\<^sub>l\<^sub>a\<^sub>n\<^sub>e\<^sub>t_\<AA>_def, simp, rule const_StrictRefEq\<^sub>S\<^sub>e\<^sub>t_including, simp, simp, simp, rule OclIncluding_cong, simp, simp)
+  apply(subst state_update_vs_allInstances_generic_tc, simp, simp, simp add: OclAsType\<^sub>P\<^sub>l\<^sub>a\<^sub>n\<^sub>e\<^sub>t_\<AA>_def, simp, rule const_StrictRefEq\<^sub>S\<^sub>e\<^sub>t_including, simp, simp, simp, rule OclIncluding_cong, simp, simp)
+  apply(subst state_update_vs_allInstances_generic_tc, simp, simp, simp add: OclAsType\<^sub>P\<^sub>l\<^sub>a\<^sub>n\<^sub>e\<^sub>t_\<AA>_def, simp, rule const_StrictRefEq\<^sub>S\<^sub>e\<^sub>t_including, simp, simp, simp, rule OclIncluding_cong, simp, simp)
+  apply(subst state_update_vs_allInstances_generic_tc, simp, simp, simp add: OclAsType\<^sub>P\<^sub>l\<^sub>a\<^sub>n\<^sub>e\<^sub>t_\<AA>_def, simp, rule const_StrictRefEq\<^sub>S\<^sub>e\<^sub>t_including, simp, simp, simp, rule OclIncluding_cong, simp, simp)
+  apply(subst state_update_vs_allInstances_generic_ntc, simp, simp, simp add: OclAsType\<^sub>P\<^sub>l\<^sub>a\<^sub>n\<^sub>e\<^sub>t_\<AA>_def X\<^sub>P\<^sub>e\<^sub>r\<^sub>s\<^sub>o\<^sub>n7\<^sub>O\<^sub>c\<^sub>l\<^sub>A\<^sub>n\<^sub>y_def, simp, rule const_StrictRefEq\<^sub>S\<^sub>e\<^sub>t_including, simp, simp, simp)
+  apply(subst state_update_vs_allInstances_generic_ntc, simp, simp, simp add: OclAsType\<^sub>P\<^sub>l\<^sub>a\<^sub>n\<^sub>e\<^sub>t_\<AA>_def X\<^sub>P\<^sub>e\<^sub>r\<^sub>s\<^sub>o\<^sub>n8\<^sub>O\<^sub>c\<^sub>l\<^sub>A\<^sub>n\<^sub>y_def, simp, rule const_StrictRefEq\<^sub>S\<^sub>e\<^sub>t_including, simp, simp, simp)
+  apply(subst state_update_vs_allInstances_generic_tc, simp, simp, simp add: OclAsType\<^sub>P\<^sub>l\<^sub>a\<^sub>n\<^sub>e\<^sub>t_\<AA>_def, simp, rule const_StrictRefEq\<^sub>S\<^sub>e\<^sub>t_including, simp, simp, simp, rule OclIncluding_cong, simp, simp)
+  apply(rule state_update_vs_allInstances_generic_empty)
+by((simp add: OclAsType\<^sub>P\<^sub>l\<^sub>a\<^sub>n\<^sub>e\<^sub>t_\<AA>_def)+) 
+lemma \<sigma>\<^sub>1'_OclAllInstances_at_post_exec_Planet : 
+shows "(st , \<sigma>\<^sub>1') \<Turnstile> (OclAllInstances_at_post (Planet)) \<doteq> Set{X\<^sub>P\<^sub>e\<^sub>r\<^sub>s\<^sub>o\<^sub>n1 .oclAsType(Planet) , X\<^sub>P\<^sub>e\<^sub>r\<^sub>s\<^sub>o\<^sub>n2 .oclAsType(Planet) , X\<^sub>P\<^sub>e\<^sub>r\<^sub>s\<^sub>o\<^sub>n3 .oclAsType(Planet) , X\<^sub>P\<^sub>e\<^sub>r\<^sub>s\<^sub>o\<^sub>n4 .oclAsType(Planet) , X\<^sub>P\<^sub>e\<^sub>r\<^sub>s\<^sub>o\<^sub>n6 .oclAsType(Planet) , X\<^sub>P\<^sub>e\<^sub>r\<^sub>s\<^sub>o\<^sub>n9 .oclAsType(Planet)}"
+  unfolding OclAllInstances_at_post_def
+by(rule \<sigma>\<^sub>1'_OclAllInstances_generic_exec_Planet, simp) 
+lemma \<sigma>\<^sub>1'_OclAllInstances_at_pre_exec_Planet : 
+shows "(\<sigma>\<^sub>1' , st) \<Turnstile> (OclAllInstances_at_pre (Planet)) \<doteq> Set{X\<^sub>P\<^sub>e\<^sub>r\<^sub>s\<^sub>o\<^sub>n1 .oclAsType(Planet) , X\<^sub>P\<^sub>e\<^sub>r\<^sub>s\<^sub>o\<^sub>n2 .oclAsType(Planet) , X\<^sub>P\<^sub>e\<^sub>r\<^sub>s\<^sub>o\<^sub>n3 .oclAsType(Planet) , X\<^sub>P\<^sub>e\<^sub>r\<^sub>s\<^sub>o\<^sub>n4 .oclAsType(Planet) , X\<^sub>P\<^sub>e\<^sub>r\<^sub>s\<^sub>o\<^sub>n6 .oclAsType(Planet) , X\<^sub>P\<^sub>e\<^sub>r\<^sub>s\<^sub>o\<^sub>n9 .oclAsType(Planet)}"
+  unfolding OclAllInstances_at_pre_def
+by(rule \<sigma>\<^sub>1'_OclAllInstances_generic_exec_Planet, simp) 
+lemma \<sigma>\<^sub>1'_OclAllInstances_generic_exec_Galaxy : 
+assumes [simp]: "(\<And>a. (pre_post ((mk (a)))) = a)"
+shows "(mk (\<sigma>\<^sub>1')) \<Turnstile> (OclAllInstances_generic (pre_post) (Galaxy)) \<doteq> Set{X\<^sub>P\<^sub>e\<^sub>r\<^sub>s\<^sub>o\<^sub>n1 .oclAsType(Galaxy) , X\<^sub>P\<^sub>e\<^sub>r\<^sub>s\<^sub>o\<^sub>n2 .oclAsType(Galaxy) , X\<^sub>P\<^sub>e\<^sub>r\<^sub>s\<^sub>o\<^sub>n3 .oclAsType(Galaxy) , X\<^sub>P\<^sub>e\<^sub>r\<^sub>s\<^sub>o\<^sub>n4 .oclAsType(Galaxy) , X\<^sub>P\<^sub>e\<^sub>r\<^sub>s\<^sub>o\<^sub>n6 .oclAsType(Galaxy) , X\<^sub>P\<^sub>e\<^sub>r\<^sub>s\<^sub>o\<^sub>n9 .oclAsType(Galaxy)}"
+  apply(subst perm_\<sigma>\<^sub>1')
+  apply(simp only: state.make_def oid0_def oid1_def oid2_def oid3_def oid5_def oid6_def oid7_def oid8_def X\<^sub>P\<^sub>e\<^sub>r\<^sub>s\<^sub>o\<^sub>n1_def X\<^sub>P\<^sub>e\<^sub>r\<^sub>s\<^sub>o\<^sub>n2_def X\<^sub>P\<^sub>e\<^sub>r\<^sub>s\<^sub>o\<^sub>n3_def X\<^sub>P\<^sub>e\<^sub>r\<^sub>s\<^sub>o\<^sub>n4_def X\<^sub>P\<^sub>e\<^sub>r\<^sub>s\<^sub>o\<^sub>n6_def X\<^sub>P\<^sub>e\<^sub>r\<^sub>s\<^sub>o\<^sub>n9_def X\<^sub>P\<^sub>e\<^sub>r\<^sub>s\<^sub>o\<^sub>n1\<^sub>P\<^sub>e\<^sub>r\<^sub>s\<^sub>o\<^sub>n_def X\<^sub>P\<^sub>e\<^sub>r\<^sub>s\<^sub>o\<^sub>n2\<^sub>P\<^sub>e\<^sub>r\<^sub>s\<^sub>o\<^sub>n_def X\<^sub>P\<^sub>e\<^sub>r\<^sub>s\<^sub>o\<^sub>n3\<^sub>P\<^sub>e\<^sub>r\<^sub>s\<^sub>o\<^sub>n_def X\<^sub>P\<^sub>e\<^sub>r\<^sub>s\<^sub>o\<^sub>n4\<^sub>P\<^sub>e\<^sub>r\<^sub>s\<^sub>o\<^sub>n_def X\<^sub>P\<^sub>e\<^sub>r\<^sub>s\<^sub>o\<^sub>n6\<^sub>P\<^sub>e\<^sub>r\<^sub>s\<^sub>o\<^sub>n_def X\<^sub>P\<^sub>e\<^sub>r\<^sub>s\<^sub>o\<^sub>n9\<^sub>P\<^sub>e\<^sub>r\<^sub>s\<^sub>o\<^sub>n_def)
+  apply(subst state_update_vs_allInstances_generic_tc, simp, simp, simp add: OclAsType\<^sub>G\<^sub>a\<^sub>l\<^sub>a\<^sub>x\<^sub>y_\<AA>_def, simp, rule const_StrictRefEq\<^sub>S\<^sub>e\<^sub>t_including, simp, simp, simp, rule OclIncluding_cong, simp, simp)
+  apply(subst state_update_vs_allInstances_generic_tc, simp, simp, simp add: OclAsType\<^sub>G\<^sub>a\<^sub>l\<^sub>a\<^sub>x\<^sub>y_\<AA>_def, simp, rule const_StrictRefEq\<^sub>S\<^sub>e\<^sub>t_including, simp, simp, simp, rule OclIncluding_cong, simp, simp)
+  apply(subst state_update_vs_allInstances_generic_tc, simp, simp, simp add: OclAsType\<^sub>G\<^sub>a\<^sub>l\<^sub>a\<^sub>x\<^sub>y_\<AA>_def, simp, rule const_StrictRefEq\<^sub>S\<^sub>e\<^sub>t_including, simp, simp, simp, rule OclIncluding_cong, simp, simp)
+  apply(subst state_update_vs_allInstances_generic_tc, simp, simp, simp add: OclAsType\<^sub>G\<^sub>a\<^sub>l\<^sub>a\<^sub>x\<^sub>y_\<AA>_def, simp, rule const_StrictRefEq\<^sub>S\<^sub>e\<^sub>t_including, simp, simp, simp, rule OclIncluding_cong, simp, simp)
+  apply(subst state_update_vs_allInstances_generic_tc, simp, simp, simp add: OclAsType\<^sub>G\<^sub>a\<^sub>l\<^sub>a\<^sub>x\<^sub>y_\<AA>_def, simp, rule const_StrictRefEq\<^sub>S\<^sub>e\<^sub>t_including, simp, simp, simp, rule OclIncluding_cong, simp, simp)
+  apply(subst state_update_vs_allInstances_generic_ntc, simp, simp, simp add: OclAsType\<^sub>G\<^sub>a\<^sub>l\<^sub>a\<^sub>x\<^sub>y_\<AA>_def X\<^sub>P\<^sub>e\<^sub>r\<^sub>s\<^sub>o\<^sub>n7\<^sub>O\<^sub>c\<^sub>l\<^sub>A\<^sub>n\<^sub>y_def, simp, rule const_StrictRefEq\<^sub>S\<^sub>e\<^sub>t_including, simp, simp, simp)
+  apply(subst state_update_vs_allInstances_generic_ntc, simp, simp, simp add: OclAsType\<^sub>G\<^sub>a\<^sub>l\<^sub>a\<^sub>x\<^sub>y_\<AA>_def X\<^sub>P\<^sub>e\<^sub>r\<^sub>s\<^sub>o\<^sub>n8\<^sub>O\<^sub>c\<^sub>l\<^sub>A\<^sub>n\<^sub>y_def, simp, rule const_StrictRefEq\<^sub>S\<^sub>e\<^sub>t_including, simp, simp, simp)
+  apply(subst state_update_vs_allInstances_generic_tc, simp, simp, simp add: OclAsType\<^sub>G\<^sub>a\<^sub>l\<^sub>a\<^sub>x\<^sub>y_\<AA>_def, simp, rule const_StrictRefEq\<^sub>S\<^sub>e\<^sub>t_including, simp, simp, simp, rule OclIncluding_cong, simp, simp)
+  apply(rule state_update_vs_allInstances_generic_empty)
+by((simp add: OclAsType\<^sub>G\<^sub>a\<^sub>l\<^sub>a\<^sub>x\<^sub>y_\<AA>_def)+) 
+lemma \<sigma>\<^sub>1'_OclAllInstances_at_post_exec_Galaxy : 
+shows "(st , \<sigma>\<^sub>1') \<Turnstile> (OclAllInstances_at_post (Galaxy)) \<doteq> Set{X\<^sub>P\<^sub>e\<^sub>r\<^sub>s\<^sub>o\<^sub>n1 .oclAsType(Galaxy) , X\<^sub>P\<^sub>e\<^sub>r\<^sub>s\<^sub>o\<^sub>n2 .oclAsType(Galaxy) , X\<^sub>P\<^sub>e\<^sub>r\<^sub>s\<^sub>o\<^sub>n3 .oclAsType(Galaxy) , X\<^sub>P\<^sub>e\<^sub>r\<^sub>s\<^sub>o\<^sub>n4 .oclAsType(Galaxy) , X\<^sub>P\<^sub>e\<^sub>r\<^sub>s\<^sub>o\<^sub>n6 .oclAsType(Galaxy) , X\<^sub>P\<^sub>e\<^sub>r\<^sub>s\<^sub>o\<^sub>n9 .oclAsType(Galaxy)}"
+  unfolding OclAllInstances_at_post_def
+by(rule \<sigma>\<^sub>1'_OclAllInstances_generic_exec_Galaxy, simp) 
+lemma \<sigma>\<^sub>1'_OclAllInstances_at_pre_exec_Galaxy : 
+shows "(\<sigma>\<^sub>1' , st) \<Turnstile> (OclAllInstances_at_pre (Galaxy)) \<doteq> Set{X\<^sub>P\<^sub>e\<^sub>r\<^sub>s\<^sub>o\<^sub>n1 .oclAsType(Galaxy) , X\<^sub>P\<^sub>e\<^sub>r\<^sub>s\<^sub>o\<^sub>n2 .oclAsType(Galaxy) , X\<^sub>P\<^sub>e\<^sub>r\<^sub>s\<^sub>o\<^sub>n3 .oclAsType(Galaxy) , X\<^sub>P\<^sub>e\<^sub>r\<^sub>s\<^sub>o\<^sub>n4 .oclAsType(Galaxy) , X\<^sub>P\<^sub>e\<^sub>r\<^sub>s\<^sub>o\<^sub>n6 .oclAsType(Galaxy) , X\<^sub>P\<^sub>e\<^sub>r\<^sub>s\<^sub>o\<^sub>n9 .oclAsType(Galaxy)}"
+  unfolding OclAllInstances_at_pre_def
+by(rule \<sigma>\<^sub>1'_OclAllInstances_generic_exec_Galaxy, simp) 
+lemma \<sigma>\<^sub>1'_OclAllInstances_generic_exec_OclAny : 
+assumes [simp]: "(\<And>a. (pre_post ((mk (a)))) = a)"
+shows "(mk (\<sigma>\<^sub>1')) \<Turnstile> (OclAllInstances_generic (pre_post) (OclAny)) \<doteq> Set{X\<^sub>P\<^sub>e\<^sub>r\<^sub>s\<^sub>o\<^sub>n1 .oclAsType(OclAny) , X\<^sub>P\<^sub>e\<^sub>r\<^sub>s\<^sub>o\<^sub>n2 .oclAsType(OclAny) , X\<^sub>P\<^sub>e\<^sub>r\<^sub>s\<^sub>o\<^sub>n3 .oclAsType(OclAny) , X\<^sub>P\<^sub>e\<^sub>r\<^sub>s\<^sub>o\<^sub>n4 .oclAsType(OclAny) , X\<^sub>P\<^sub>e\<^sub>r\<^sub>s\<^sub>o\<^sub>n6 .oclAsType(OclAny) , X\<^sub>P\<^sub>e\<^sub>r\<^sub>s\<^sub>o\<^sub>n7 , X\<^sub>P\<^sub>e\<^sub>r\<^sub>s\<^sub>o\<^sub>n8 , X\<^sub>P\<^sub>e\<^sub>r\<^sub>s\<^sub>o\<^sub>n9 .oclAsType(OclAny)}"
+  apply(subst perm_\<sigma>\<^sub>1')
+  apply(simp only: state.make_def oid0_def oid1_def oid2_def oid3_def oid5_def oid6_def oid7_def oid8_def X\<^sub>P\<^sub>e\<^sub>r\<^sub>s\<^sub>o\<^sub>n1_def X\<^sub>P\<^sub>e\<^sub>r\<^sub>s\<^sub>o\<^sub>n2_def X\<^sub>P\<^sub>e\<^sub>r\<^sub>s\<^sub>o\<^sub>n3_def X\<^sub>P\<^sub>e\<^sub>r\<^sub>s\<^sub>o\<^sub>n4_def X\<^sub>P\<^sub>e\<^sub>r\<^sub>s\<^sub>o\<^sub>n6_def X\<^sub>P\<^sub>e\<^sub>r\<^sub>s\<^sub>o\<^sub>n7_def X\<^sub>P\<^sub>e\<^sub>r\<^sub>s\<^sub>o\<^sub>n8_def X\<^sub>P\<^sub>e\<^sub>r\<^sub>s\<^sub>o\<^sub>n9_def X\<^sub>P\<^sub>e\<^sub>r\<^sub>s\<^sub>o\<^sub>n1\<^sub>P\<^sub>e\<^sub>r\<^sub>s\<^sub>o\<^sub>n_def X\<^sub>P\<^sub>e\<^sub>r\<^sub>s\<^sub>o\<^sub>n2\<^sub>P\<^sub>e\<^sub>r\<^sub>s\<^sub>o\<^sub>n_def X\<^sub>P\<^sub>e\<^sub>r\<^sub>s\<^sub>o\<^sub>n3\<^sub>P\<^sub>e\<^sub>r\<^sub>s\<^sub>o\<^sub>n_def X\<^sub>P\<^sub>e\<^sub>r\<^sub>s\<^sub>o\<^sub>n4\<^sub>P\<^sub>e\<^sub>r\<^sub>s\<^sub>o\<^sub>n_def X\<^sub>P\<^sub>e\<^sub>r\<^sub>s\<^sub>o\<^sub>n6\<^sub>P\<^sub>e\<^sub>r\<^sub>s\<^sub>o\<^sub>n_def X\<^sub>P\<^sub>e\<^sub>r\<^sub>s\<^sub>o\<^sub>n9\<^sub>P\<^sub>e\<^sub>r\<^sub>s\<^sub>o\<^sub>n_def)
+  apply(subst state_update_vs_allInstances_generic_tc, simp, simp, simp add: OclAsType\<^sub>O\<^sub>c\<^sub>l\<^sub>A\<^sub>n\<^sub>y_\<AA>_def, simp, rule const_StrictRefEq\<^sub>S\<^sub>e\<^sub>t_including, simp, simp, simp, rule OclIncluding_cong, simp, simp)
+  apply(subst state_update_vs_allInstances_generic_tc, simp, simp, simp add: OclAsType\<^sub>O\<^sub>c\<^sub>l\<^sub>A\<^sub>n\<^sub>y_\<AA>_def, simp, rule const_StrictRefEq\<^sub>S\<^sub>e\<^sub>t_including, simp, simp, simp, rule OclIncluding_cong, simp, simp)
+  apply(subst state_update_vs_allInstances_generic_tc, simp, simp, simp add: OclAsType\<^sub>O\<^sub>c\<^sub>l\<^sub>A\<^sub>n\<^sub>y_\<AA>_def, simp, rule const_StrictRefEq\<^sub>S\<^sub>e\<^sub>t_including, simp, simp, simp, rule OclIncluding_cong, simp, simp)
+  apply(subst state_update_vs_allInstances_generic_tc, simp, simp, simp add: OclAsType\<^sub>O\<^sub>c\<^sub>l\<^sub>A\<^sub>n\<^sub>y_\<AA>_def, simp, rule const_StrictRefEq\<^sub>S\<^sub>e\<^sub>t_including, simp, simp, simp, rule OclIncluding_cong, simp, simp)
+  apply(subst state_update_vs_allInstances_generic_tc, simp, simp, simp add: OclAsType\<^sub>O\<^sub>c\<^sub>l\<^sub>A\<^sub>n\<^sub>y_\<AA>_def, simp, rule const_StrictRefEq\<^sub>S\<^sub>e\<^sub>t_including, simp, simp, simp, rule OclIncluding_cong, simp, simp)
+  apply(subst state_update_vs_allInstances_generic_tc, simp, simp, simp add: OclAsType\<^sub>O\<^sub>c\<^sub>l\<^sub>A\<^sub>n\<^sub>y_\<AA>_def, simp, rule const_StrictRefEq\<^sub>S\<^sub>e\<^sub>t_including, simp, simp, simp, rule OclIncluding_cong, simp, simp)
+  apply(subst state_update_vs_allInstances_generic_tc, simp, simp, simp add: OclAsType\<^sub>O\<^sub>c\<^sub>l\<^sub>A\<^sub>n\<^sub>y_\<AA>_def, simp, rule const_StrictRefEq\<^sub>S\<^sub>e\<^sub>t_including, simp, simp, simp, rule OclIncluding_cong, simp, simp)
+  apply(subst state_update_vs_allInstances_generic_tc, simp, simp, simp add: OclAsType\<^sub>O\<^sub>c\<^sub>l\<^sub>A\<^sub>n\<^sub>y_\<AA>_def, simp, rule const_StrictRefEq\<^sub>S\<^sub>e\<^sub>t_including, simp, simp, simp, rule OclIncluding_cong, simp, simp)
+  apply(rule state_update_vs_allInstances_generic_empty)
+by((simp add: OclAsType\<^sub>O\<^sub>c\<^sub>l\<^sub>A\<^sub>n\<^sub>y_\<AA>_def)+) 
+lemma \<sigma>\<^sub>1'_OclAllInstances_at_post_exec_OclAny : 
+shows "(st , \<sigma>\<^sub>1') \<Turnstile> (OclAllInstances_at_post (OclAny)) \<doteq> Set{X\<^sub>P\<^sub>e\<^sub>r\<^sub>s\<^sub>o\<^sub>n1 .oclAsType(OclAny) , X\<^sub>P\<^sub>e\<^sub>r\<^sub>s\<^sub>o\<^sub>n2 .oclAsType(OclAny) , X\<^sub>P\<^sub>e\<^sub>r\<^sub>s\<^sub>o\<^sub>n3 .oclAsType(OclAny) , X\<^sub>P\<^sub>e\<^sub>r\<^sub>s\<^sub>o\<^sub>n4 .oclAsType(OclAny) , X\<^sub>P\<^sub>e\<^sub>r\<^sub>s\<^sub>o\<^sub>n6 .oclAsType(OclAny) , X\<^sub>P\<^sub>e\<^sub>r\<^sub>s\<^sub>o\<^sub>n7 , X\<^sub>P\<^sub>e\<^sub>r\<^sub>s\<^sub>o\<^sub>n8 , X\<^sub>P\<^sub>e\<^sub>r\<^sub>s\<^sub>o\<^sub>n9 .oclAsType(OclAny)}"
+  unfolding OclAllInstances_at_post_def
+by(rule \<sigma>\<^sub>1'_OclAllInstances_generic_exec_OclAny, simp) 
+lemma \<sigma>\<^sub>1'_OclAllInstances_at_pre_exec_OclAny : 
+shows "(\<sigma>\<^sub>1' , st) \<Turnstile> (OclAllInstances_at_pre (OclAny)) \<doteq> Set{X\<^sub>P\<^sub>e\<^sub>r\<^sub>s\<^sub>o\<^sub>n1 .oclAsType(OclAny) , X\<^sub>P\<^sub>e\<^sub>r\<^sub>s\<^sub>o\<^sub>n2 .oclAsType(OclAny) , X\<^sub>P\<^sub>e\<^sub>r\<^sub>s\<^sub>o\<^sub>n3 .oclAsType(OclAny) , X\<^sub>P\<^sub>e\<^sub>r\<^sub>s\<^sub>o\<^sub>n4 .oclAsType(OclAny) , X\<^sub>P\<^sub>e\<^sub>r\<^sub>s\<^sub>o\<^sub>n6 .oclAsType(OclAny) , X\<^sub>P\<^sub>e\<^sub>r\<^sub>s\<^sub>o\<^sub>n7 , X\<^sub>P\<^sub>e\<^sub>r\<^sub>s\<^sub>o\<^sub>n8 , X\<^sub>P\<^sub>e\<^sub>r\<^sub>s\<^sub>o\<^sub>n9 .oclAsType(OclAny)}"
+  unfolding OclAllInstances_at_pre_def
+by(rule \<sigma>\<^sub>1'_OclAllInstances_generic_exec_OclAny, simp) 
+
+(* 138 ************************************ 815 + 1 *)
 definition "\<sigma>\<^sub>0 = (state.make ((Map.empty )) (Map.empty) (Map.empty))"
+
+(* 139 ************************************ 816 + 1 *)
+lemma dom_\<sigma>\<^sub>0 : "(dom ((heap (\<sigma>\<^sub>0)))) = {}"
+by(auto simp: \<sigma>\<^sub>0_def)
+
+(* 140 ************************************ 817 + 1 *)
+lemmas [simp,code_unfold] = dom_\<sigma>\<^sub>0
+
+(* 141 ************************************ 818 + 1 *)
+lemma perm_\<sigma>\<^sub>0 : "\<sigma>\<^sub>0 = (state.make ((Map.empty )) ((assocs\<^sub>2 (\<sigma>\<^sub>0))) ((assocs\<^sub>3 (\<sigma>\<^sub>0))))"
+by(simp add: \<sigma>\<^sub>0_def)
+
+(* 142 ************************************ 819 + 12 *)
+lemma \<sigma>\<^sub>0_OclAllInstances_generic_exec_Person : 
+assumes [simp]: "(\<And>a. (pre_post ((mk (a)))) = a)"
+shows "(mk (\<sigma>\<^sub>0)) \<Turnstile> (OclAllInstances_generic (pre_post) (Person)) \<doteq> Set{}"
+  apply(subst perm_\<sigma>\<^sub>0)
+  apply(simp only: state.make_def)
+  apply(rule state_update_vs_allInstances_generic_empty)
+by(simp) 
+lemma \<sigma>\<^sub>0_OclAllInstances_at_post_exec_Person : 
+shows "(st , \<sigma>\<^sub>0) \<Turnstile> (OclAllInstances_at_post (Person)) \<doteq> Set{}"
+  unfolding OclAllInstances_at_post_def
+by(rule \<sigma>\<^sub>0_OclAllInstances_generic_exec_Person, simp) 
+lemma \<sigma>\<^sub>0_OclAllInstances_at_pre_exec_Person : 
+shows "(\<sigma>\<^sub>0 , st) \<Turnstile> (OclAllInstances_at_pre (Person)) \<doteq> Set{}"
+  unfolding OclAllInstances_at_pre_def
+by(rule \<sigma>\<^sub>0_OclAllInstances_generic_exec_Person, simp) 
+lemma \<sigma>\<^sub>0_OclAllInstances_generic_exec_Planet : 
+assumes [simp]: "(\<And>a. (pre_post ((mk (a)))) = a)"
+shows "(mk (\<sigma>\<^sub>0)) \<Turnstile> (OclAllInstances_generic (pre_post) (Planet)) \<doteq> Set{}"
+  apply(subst perm_\<sigma>\<^sub>0)
+  apply(simp only: state.make_def)
+  apply(rule state_update_vs_allInstances_generic_empty)
+by(simp) 
+lemma \<sigma>\<^sub>0_OclAllInstances_at_post_exec_Planet : 
+shows "(st , \<sigma>\<^sub>0) \<Turnstile> (OclAllInstances_at_post (Planet)) \<doteq> Set{}"
+  unfolding OclAllInstances_at_post_def
+by(rule \<sigma>\<^sub>0_OclAllInstances_generic_exec_Planet, simp) 
+lemma \<sigma>\<^sub>0_OclAllInstances_at_pre_exec_Planet : 
+shows "(\<sigma>\<^sub>0 , st) \<Turnstile> (OclAllInstances_at_pre (Planet)) \<doteq> Set{}"
+  unfolding OclAllInstances_at_pre_def
+by(rule \<sigma>\<^sub>0_OclAllInstances_generic_exec_Planet, simp) 
+lemma \<sigma>\<^sub>0_OclAllInstances_generic_exec_Galaxy : 
+assumes [simp]: "(\<And>a. (pre_post ((mk (a)))) = a)"
+shows "(mk (\<sigma>\<^sub>0)) \<Turnstile> (OclAllInstances_generic (pre_post) (Galaxy)) \<doteq> Set{}"
+  apply(subst perm_\<sigma>\<^sub>0)
+  apply(simp only: state.make_def)
+  apply(rule state_update_vs_allInstances_generic_empty)
+by(simp) 
+lemma \<sigma>\<^sub>0_OclAllInstances_at_post_exec_Galaxy : 
+shows "(st , \<sigma>\<^sub>0) \<Turnstile> (OclAllInstances_at_post (Galaxy)) \<doteq> Set{}"
+  unfolding OclAllInstances_at_post_def
+by(rule \<sigma>\<^sub>0_OclAllInstances_generic_exec_Galaxy, simp) 
+lemma \<sigma>\<^sub>0_OclAllInstances_at_pre_exec_Galaxy : 
+shows "(\<sigma>\<^sub>0 , st) \<Turnstile> (OclAllInstances_at_pre (Galaxy)) \<doteq> Set{}"
+  unfolding OclAllInstances_at_pre_def
+by(rule \<sigma>\<^sub>0_OclAllInstances_generic_exec_Galaxy, simp) 
+lemma \<sigma>\<^sub>0_OclAllInstances_generic_exec_OclAny : 
+assumes [simp]: "(\<And>a. (pre_post ((mk (a)))) = a)"
+shows "(mk (\<sigma>\<^sub>0)) \<Turnstile> (OclAllInstances_generic (pre_post) (OclAny)) \<doteq> Set{}"
+  apply(subst perm_\<sigma>\<^sub>0)
+  apply(simp only: state.make_def)
+  apply(rule state_update_vs_allInstances_generic_empty)
+by(simp) 
+lemma \<sigma>\<^sub>0_OclAllInstances_at_post_exec_OclAny : 
+shows "(st , \<sigma>\<^sub>0) \<Turnstile> (OclAllInstances_at_post (OclAny)) \<doteq> Set{}"
+  unfolding OclAllInstances_at_post_def
+by(rule \<sigma>\<^sub>0_OclAllInstances_generic_exec_OclAny, simp) 
+lemma \<sigma>\<^sub>0_OclAllInstances_at_pre_exec_OclAny : 
+shows "(\<sigma>\<^sub>0 , st) \<Turnstile> (OclAllInstances_at_pre (OclAny)) \<doteq> Set{}"
+  unfolding OclAllInstances_at_pre_def
+by(rule \<sigma>\<^sub>0_OclAllInstances_generic_exec_OclAny, simp) 
 
 end
